@prefix dcterms: <http://purl.org/dc/terms/> .
@prefix jsonld: <https://www.w3.org/TR/json-ld11/> .
@prefix ns1: <http://www.opengis.net/def/metamodel/ogc-na/> .
@prefix owl: <http://www.w3.org/2002/07/owl#> .
@prefix prof: <http://www.w3.org/ns/dx/prof/> .
@prefix profiles: <http://www.opengis.net/def/metamodel/profiles/> .
@prefix profrole: <http://www.w3.org/ns/dx/prof/role/> .
@prefix rdfs: <http://www.w3.org/2000/01/rdf-schema#> .
@prefix sh: <http://www.w3.org/ns/shacl#> .
@prefix skos: <http://www.w3.org/2004/02/skos/core#> .
@prefix xsd: <http://www.w3.org/2001/XMLSchema#> .

profiles:skos skos:narrower profiles:skos_shared .

<http://www.w3.org/2004/02/skos/core> skos:narrower profiles:skos_shared .

profiles:skos_shared a skos:Concept,
        prof:Profile ;
    rdfs:label "Shareable SKOS" ;
    ns1:status <http://www.opengis.net/def/status/valid> ;
    skos:broader profiles:skos,
        <http://www.w3.org/2004/02/skos/core> ;
    skos:definition """Provides a minimal profile for sharing of terms across multiple environments using SKOS. 
  
  The requirement here is that the source of each term can be unambiguosly identified without dereferencing the term successfully in an online environment and successfully navigating to metadata about the scheme that defines the term.
  
  """ ;
    skos:inScheme <http://www.opengis.net/def/metamodel/profiles> ;
    skos:prefLabel "Shareable SKOS" ;
    prof:hasResource [ a prof:ResourceDescriptor ;
            rdfs:label "Profile description as HTML" ;
            dcterms:conformsTo prof: ;
            dcterms:format "text/html" ;
            rdfs:comment "Artefact is self reference using canonical URI and content negotiation" ;
            prof:hasArtifact profiles:skos_shared ;
            prof:hasRole profrole:profile ],
        [ a prof:ResourceDescriptor ;
            rdfs:label "Profile constraints as SHACL" ;
            dcterms:conformsTo sh: ;
            dcterms:format "text/turtle" ;
            rdfs:comment "Artefact is self reference using canonical URI and content negotiation" ;
            prof:hasArtifact <http://defs-dev.opengis.net/ogc-na/definitions/profiles/resources/skos_shared_shacl.ttl>,
                profiles:skos_shared,
                <http://www.opengis.net/def/metamodel/profiles/skos_shared?_profile=shacl&_mediatype=text/turtle> ;
            prof:hasRole profrole:validation ],
        [ a prof:ResourceDescriptor ;
            rdfs:label "Profile Class Diagram" ;
            dcterms:format "image/png" ;
            rdfs:comment "Crude illustration of profile scope" ;
            prof:hasArtifact <http://defs-dev.opengis.net/ogc-na/definitions/profiles/resources/skos_shared_class_diagram.png> ],
        [ a prof:ResourceDescriptor ;
            rdfs:label "Validation example" ;
            dcterms:conformsTo sh: ;
            dcterms:format "text/turtle" ;
            rdfs:comment "Uses SHACL rules against a sample vocabulary with known issue" ;
            prof:hasArtifact <https://shacl-play.sparna.fr/play/validate?url=http://defs-dev.opengis.net/ogc-na/definitions/conceptschemes/auth.ttl&shapesUrl=http://defs-dev.opengis.net/ogc-na/definitions/profiles/resources/skos_shared_shacl.ttl>,
                <https://shacl-play.sparna.fr/play/validate?url=http://defs-dev.opengis.net/ogc-na/definitions/conceptschemes/entailed/auth.ttl&shapesUrl=http://defs-dev.opengis.net/ogc-na/definitions/profiles/resources/skos_shared_shacl.ttl> ;
            prof:hasRole profrole:example ],
        [ a prof:ResourceDescriptor ;
            rdfs:label "OWL view" ;
            dcterms:conformsTo owl: ;
            dcterms:format "text/turtle" ;
            rdfs:comment "OWL classes for profile" ;
            prof:hasArtifact <http://defs-dev.opengis.net/ogc-na/definitions/profiles/resources/skos_shared_owl.ttl> ;
            prof:hasRole profrole:profile ],
        [ a prof:ResourceDescriptor ;
            rdfs:label "JSON-LD Implementation Example - Viewer" ;
            dcterms:conformsTo jsonld: ;
            dcterms:format "application/json" ;
            rdfs:comment "JSON-LD playground permalink accessing sample resources" ;
            prof:hasArtifact <https://tinyurl.com/stfrmhh2> ;
            prof:hasRole profrole:example ],
        [ a prof:ResourceDescriptor ;
            rdfs:label "JSON-LD Implementation Example - Data" ;
            dcterms:conformsTo jsonld: ;
            dcterms:format "application/json" ;
            rdfs:comment "Data object" ;
            prof:hasArtifact <http://defs-dev.opengis.net/ogc-na/definitions/profiles/resources/skos_shared_example.json> ;
            prof:hasRole profrole:example ] ;
    prof:hasToken "skos_shared"^^xsd:token ;
    prof:isProfileOf profiles:skos,
        <http://www.w3.org/2004/02/skos/core> .

