<http://www.opengis.net/def/observation-collection-type/OGC/0/by-member-characteristics-semantics>
        a       <http://www.w3.org/2004/02/skos/core#ConceptScheme> ;
        <http://purl.org/dc/terms/created>  "2021-06-15" ;
        <http://www.w3.org/2000/01/rdf-schema#label>  "Collection type by the interpretation of its memberCharacteristics"@en ;
        <http://www.w3.org/2004/02/skos/core#definition>  "OMS 3.0 ObservationCollection classification scheme based on how the properties of its memberCharacteristics relate to the properties of the member Observations of the collection."@en ;
        <http://www.w3.org/2004/02/skos/core#inScheme>  <http://www.opengis.net/def/observation-collection-type> ;
        <http://www.w3.org/2004/02/skos/core#prefLabel>  "Collection type by the interpretation of its memberCharacteristics"@en .

<http://www.opengis.net/def/observation-collection-type/OGC/0/by-member-characteristics-semantics/>
        a       <http://www.w3.org/2004/02/skos/core#Collection> ;
        <http://purl.org/dc/terms/created>  "2021-06-09" ;
        <http://www.w3.org/2004/02/skos/core#member>  <http://www.opengis.net/def/observation-collection-type/OGC/0/by-member-characteristics-semantics/summarizing> ;
        <http://www.w3.org/2004/02/skos/core#member>  <http://www.opengis.net/def/observation-collection-type/OGC/0/by-member-characteristics-semantics/homogenous> ;
        <http://www.w3.org/2004/02/skos/core#prefLabel>  "Collection of OMS 3.0 ObservationCollection type by the semantics of its memberCharacteristics"@en .

<http://www.opengis.net/def/observation-collection-type/OGC/0/by-member-characteristics-semantics/summarizing>
        a       <http://www.w3.org/2004/02/skos/core#Concept> ;
        <http://purl.org/dc/terms/created>  "2021-06-09" ;
        <http://www.w3.org/2000/01/rdf-schema#label>  "Summarizing"@en ;
        <http://www.w3.org/2004/02/skos/core#altLabel>  "Summarizing ObservationCollection"@en ;
        <http://www.w3.org/2004/02/skos/core#definition>  "In a summarizing ObservationCollection, the properties provided though the memberCharacteristics provide the full range of the values of the corresponding Observation properties present in any of the collection members."@en ;
        <http://www.w3.org/2004/02/skos/core#inScheme>  <http://www.opengis.net/def/observation-collection-type/OGC/0/by-member-characteristics-semantics> ;
        <http://www.w3.org/2004/02/skos/core#prefLabel>  "Summarizing"@en .

<http://www.opengis.net/def/observation-collection-type/OGC/0/by-member-characteristics-semantics/homogenous>
        a       <http://www.w3.org/2004/02/skos/core#Concept> ;
        <http://purl.org/dc/terms/created>  "2021-06-09" ;
        <http://www.w3.org/2000/01/rdf-schema#label>  "Homogenous"@en ;
        <http://www.w3.org/2004/02/skos/core#altLabel>  "Homogenous ObservationCollection"@en ;
        <http://www.w3.org/2004/02/skos/core#definition>  "In a homogenous ObservationCollection the properties provided though the memberCharacteristics are identical to the corresponding Observation properties of each collection member."@en ;
        <http://www.w3.org/2004/02/skos/core#inScheme>  <http://www.opengis.net/def/observation-collection-type/OGC/0/by-member-characteristics-semantics> ;
        <http://www.w3.org/2004/02/skos/core#prefLabel>  "Homogenous"@en .
