@prefix dcterms: <http://purl.org/dc/terms/> .
@prefix ns1: <http://www.opengis.net/def/metamodel/ogc-na/> .
@prefix rdfs: <http://www.w3.org/2000/01/rdf-schema#> .
@prefix skos: <http://www.w3.org/2004/02/skos/core#> .

<http://www.opengis.net/def/observation-collection-type/> a skos:Collection ;
    dcterms:created "2021-06-09" ;
    skos:definition "Collection of ObservationCollection classification schemes"@en ;
    skos:member <http://www.opengis.net/def/observation-collection-type/OGC/0/by-member-characteristics-semantics> ;
    skos:prefLabel "Collection of ObservationCollection classification schemes"@en .

<http://www.opengis.net/def/observation-collection-type/OGC/0/by-member-characteristics-semantics/> a skos:Collection ;
    dcterms:created "2021-06-09" ;
    skos:definition "Collection of OMS 3.0 ObservationCollection type by the semantics of its memberCharacteristics"@en ;
    skos:member <http://www.opengis.net/def/observation-collection-type/OGC/0/by-member-characteristics-semantics/homogenous>,
        <http://www.opengis.net/def/observation-collection-type/OGC/0/by-member-characteristics-semantics/summarizing> ;
    skos:prefLabel "Collection of OMS 3.0 ObservationCollection type by the semantics of its memberCharacteristics"@en .

<http://www.opengis.net/def/observation-type/> a skos:Collection ;
    dcterms:created "2021-06-09" ;
    skos:definition "Collection of Observation classification schemes"@en ;
    skos:member <http://www.opengis.net/def/observation-type/OGC/0/by-result-type>,
        <http://www.opengis.net/def/ogc-omxml> ;
    skos:prefLabel "Collection of Observation classification schemes"@en .

<http://www.opengis.net/def/observation-type/OGC/0/by-result-type/> a skos:Collection ;
    dcterms:created "2021-06-09" ;
    skos:definition "Collection of ObservationTypeByResultType codelist member concepts"@en ;
    skos:member <http://www.opengis.net/def/observation-type/OGC/0/by-result-type/category-observation>,
        <http://www.opengis.net/def/observation-type/OGC/0/by-result-type/complex-observation>,
        <http://www.opengis.net/def/observation-type/OGC/0/by-result-type/count-observation>,
        <http://www.opengis.net/def/observation-type/OGC/0/by-result-type/discrete-coverage-observation>,
        <http://www.opengis.net/def/observation-type/OGC/0/by-result-type/discrete-point-coverage-observation>,
        <http://www.opengis.net/def/observation-type/OGC/0/by-result-type/geometry-observation>,
        <http://www.opengis.net/def/observation-type/OGC/0/by-result-type/measurement>,
        <http://www.opengis.net/def/observation-type/OGC/0/by-result-type/observation>,
        <http://www.opengis.net/def/observation-type/OGC/0/by-result-type/temporal-observation>,
        <http://www.opengis.net/def/observation-type/OGC/0/by-result-type/time-series-observation>,
        <http://www.opengis.net/def/observation-type/OGC/0/by-result-type/truth-observation> ;
    skos:prefLabel "Collection of ObservationTypeByResultType codelist member concepts"@en .

<http://www.opengis.net/def/sample-type/> a skos:Collection ;
    dcterms:created "2021-06-09" ;
    skos:definition "Collection of Sample classification schemes"@en ;
    skos:member <http://www.opengis.net/def/sample-type/OGC/0/by-geometry-type> ;
    skos:prefLabel "Collection of Sample classification schemes"@en .

<http://www.opengis.net/def/sample-type/OGC/0/by-geometry-type/> a skos:Collection ;
    dcterms:created "2021-06-09" ;
    skos:definition "Collection of SpatialSample by geometry type concepts"@en ;
    skos:member <http://www.opengis.net/def/sample-type/OGC/0/by-geometry-type/curve>,
        <http://www.opengis.net/def/sample-type/OGC/0/by-geometry-type/point>,
        <http://www.opengis.net/def/sample-type/OGC/0/by-geometry-type/solid>,
        <http://www.opengis.net/def/sample-type/OGC/0/by-geometry-type/surface> ;
    skos:prefLabel "Collection of SpatialSample by geometry type concepts"@en .

<http://www.opengis.net/def/sample-type/OGC/0/by-geometry-type/point/solid> a skos:Concept ;
    dcterms:created "2021-06-09" ;
    ns1:status <http://www.opengis.net/def/status/valid> ;
    skos:definition "SpatialSample with a Solid geometry as the value of its shape attribute."@en ;
    skos:exactMatch <http://www.opengis.net/def/ogc-om/SF_SamplingSolid>,
        <http://www.opengis.net/def/ogc-om/sf_sampling-solid>,
        <http://www.opengis.net/def/samplingFeatureType/OGC-OM/2.0/SF_SamplingSolid> ;
    skos:inScheme <http://www.opengis.net/def/sample-type/OGC/0/by-geometry-type> ;
    skos:prefLabel "Solid Sample"@en .

<http://www.opengis.net/def/observation-collection-type> a skos:ConceptScheme ;
    rdfs:label "ObservationCollection type"@en ;
    dcterms:created "2021-06-15" ;
    dcterms:source <http://www.opengis.net/def/entities/bodies/ogcna> ;
    skos:definition "Classification scheme for any kind of ObservationCollections"@en ;
    skos:prefLabel "ObservationCollection type"@en .

<http://www.opengis.net/def/observation-collection-type/OGC/0/by-member-characteristics-semantics/homogenous> a skos:Concept ;
    rdfs:label "Homogenous"@en ;
    dcterms:created "2021-06-09" ;
    ns1:status <http://www.opengis.net/def/status/valid> ;
    skos:altLabel "Homogenous ObservationCollection"@en ;
    skos:definition "In a homogenous ObservationCollection the properties provided though the memberCharacteristics are identical to the corresponding Observation properties of each collection member."@en ;
    skos:inScheme <http://www.opengis.net/def/observation-collection-type/OGC/0/by-member-characteristics-semantics> ;
    skos:prefLabel "Homogenous"@en .

<http://www.opengis.net/def/observation-collection-type/OGC/0/by-member-characteristics-semantics/summarizing> a skos:Concept ;
    rdfs:label "Summarizing"@en ;
    dcterms:created "2021-06-09" ;
    ns1:status <http://www.opengis.net/def/status/valid> ;
    skos:altLabel "Summarizing ObservationCollection"@en ;
    skos:definition "In a summarizing ObservationCollection, the properties provided though the memberCharacteristics provide the full range of the values of the corresponding Observation properties present in any of the collection members."@en ;
    skos:inScheme <http://www.opengis.net/def/observation-collection-type/OGC/0/by-member-characteristics-semantics> ;
    skos:prefLabel "Summarizing"@en .

<http://www.opengis.net/def/observation-type> a skos:ConceptScheme ;
    rdfs:label "Observation type"@en ;
    dcterms:created "2021-06-09" ;
    dcterms:source <http://www.opengis.net/def/entities/bodies/ogcna> ;
    skos:definition "Classification scheme for any kind of Observation classification schemes"@en ;
    skos:prefLabel "Observation type"@en .

<http://www.opengis.net/def/observation-type/OGC/0/by-result-type/category-observation> a skos:Concept ;
    dcterms:created "2021-06-09" ;
    ns1:status <http://www.opengis.net/def/status/valid> ;
    skos:definition "Observation whose result is a Scoped Name."@en ;
    skos:exactMatch <http://www.opengis.net/def/observation-type/ogc-om/2.0/om_category-observation>,
        <http://www.opengis.net/def/observationType/OGC-OM/2.0/OM_CategoryObservation>,
        <http://www.opengis.net/def/ogc-om/OM_CategoryObservation> ;
    skos:inScheme <http://www.opengis.net/def/observation-type/OGC/0/by-result-type> ;
    skos:prefLabel "Category Observation"@en .

<http://www.opengis.net/def/observation-type/OGC/0/by-result-type/complex-observation> a skos:Concept ;
    dcterms:created "2021-06-09" ;
    ns1:status <http://www.opengis.net/def/status/valid> ;
    skos:definition "Observation whose result is an Record in the ISO/IEC 11404 sense."@en ;
    skos:exactMatch <http://www.opengis.net/def/observation-type/ogc-om/2.0/om_complex-observation>,
        <http://www.opengis.net/def/observationType/OGC-OM/2.0/OM_ComplexObservation>,
        <http://www.opengis.net/def/ogc-om/OM_ComplexObservation> ;
    skos:inScheme <http://www.opengis.net/def/observation-type/OGC/0/by-result-type> ;
    skos:prefLabel "Complex Observation"@en .

<http://www.opengis.net/def/observation-type/OGC/0/by-result-type/count-observation> a skos:Concept ;
    dcterms:created "2021-06-09" ;
    ns1:status <http://www.opengis.net/def/status/valid> ;
    skos:definition "Observation whose result is a Integer."@en ;
    skos:exactMatch <http://www.opengis.net/def/observation-type/ogc-om/2.0/om_count-observation>,
        <http://www.opengis.net/def/observationType/OGC-OM/2.0/OM_CountObservation>,
        <http://www.opengis.net/def/ogc-om/OM_CountObservation> ;
    skos:inScheme <http://www.opengis.net/def/observation-type/OGC/0/by-result-type> ;
    skos:prefLabel "Count Observation"@en .

<http://www.opengis.net/def/observation-type/OGC/0/by-result-type/geometry-observation> a skos:Concept ;
    dcterms:created "2021-06-09" ;
    ns1:status <http://www.opengis.net/def/status/valid> ;
    skos:definition "Observation whose result is a Geometry."@en ;
    skos:exactMatch <http://www.opengis.net/def/observation-type/ogc-om/2.0/om_geometry-observation>,
        <http://www.opengis.net/def/observationType/OGC-OM/2.0/OM_GeometryObservation>,
        <http://www.opengis.net/def/ogc-om/OM_GeometryObservation> ;
    skos:inScheme <http://www.opengis.net/def/observation-type/OGC/0/by-result-type> ;
    skos:prefLabel "Geometry Observation"@en .

<http://www.opengis.net/def/observation-type/OGC/0/by-result-type/measurement> a skos:Concept ;
    dcterms:created "2021-06-09" ;
    ns1:status <http://www.opengis.net/def/status/valid> ;
    skos:definition "Observation whose result is a scaled number or Measure."@en ;
    skos:exactMatch <http://www.opengis.net/def/observation-type/ogc-om/2.0/om_measurement>,
        <http://www.opengis.net/def/observationType/OGC-OM/2.0/OM_Measurement>,
        <http://www.opengis.net/def/ogc-om/OM_Measurement> ;
    skos:inScheme <http://www.opengis.net/def/observation-type/OGC/0/by-result-type> ;
    skos:prefLabel "Measurement"@en .

<http://www.opengis.net/def/observation-type/OGC/0/by-result-type/observation> a skos:Concept ;
    dcterms:created "2021-06-09" ;
    ns1:status <http://www.opengis.net/def/status/valid> ;
    skos:definition "Observation whose result is of type Any"@en ;
    skos:exactMatch <http://www.opengis.net/def/observation-type/ogc-om/2.0/om_observation>,
        <http://www.opengis.net/def/observationType/OGC-OM/2.0/OM_Observation>,
        <http://www.opengis.net/def/ogc-om/OM_Observation> ;
    skos:inScheme <http://www.opengis.net/def/observation-type/OGC/0/by-result-type> ;
    skos:prefLabel "Observation"@en .

<http://www.opengis.net/def/observation-type/OGC/0/by-result-type/temporal-observation> a skos:Concept ;
    dcterms:created "2021-06-09" ;
    ns1:status <http://www.opengis.net/def/status/valid> ;
    skos:definition "Observation whose result is a TM_Object."@en ;
    skos:exactMatch <http://www.opengis.net/def/observation-type/ogc-om/2.0/om_temporal-observation>,
        <http://www.opengis.net/def/observationType/OGC-OM/2.0/OM_TemporalObservation>,
        <http://www.opengis.net/def/ogc-om/OM_TemporalObservation> ;
    skos:inScheme <http://www.opengis.net/def/observation-type/OGC/0/by-result-type> ;
    skos:prefLabel "Temporal Observation"@en .

<http://www.opengis.net/def/observation-type/OGC/0/by-result-type/time-series-observation> a skos:Concept ;
    dcterms:modified "2021-06-09" ;
    ns1:status <http://www.opengis.net/def/status/valid> ;
    skos:definition "Observation whose result is a a timeseries (a sequence of data values which are ordered in time) or a piece of a larger time series constrained by the phenomenonTime"@en ;
    skos:exactMatch <http://www.opengis.net/def/observation-type/ogc-om/2.0/om_discrete-time-series-observation>,
        <http://www.opengis.net/def/observationType/OGC-OM/2.0/OM_DiscreteTimeSeriesObservation>,
        <http://www.opengis.net/def/ogc-om/OM_TimeSeriesObservation> ;
    skos:inScheme <http://www.opengis.net/def/observation-type/OGC/0/by-result-type> ;
    skos:prefLabel "Time series Observation"@en .

<http://www.opengis.net/def/observation-type/OGC/0/by-result-type/truth-observation> a skos:Concept ;
    dcterms:created "2021-06-09" ;
    ns1:status <http://www.opengis.net/def/status/valid> ;
    skos:definition "Observation whose result is a truth value."@en ;
    skos:exactMatch <http://www.opengis.net/def/observation-type/ogc-om/2.0/om_truth-observation>,
        <http://www.opengis.net/def/observationType/OGC-OM/2.0/OM_TruthObservation>,
        <http://www.opengis.net/def/ogc-om/OM_TruthObservation> ;
    skos:inScheme <http://www.opengis.net/def/observation-type/OGC/0/by-result-type> ;
    skos:prefLabel "Truth Observation"@en .

<http://www.opengis.net/def/sample-type> a skos:ConceptScheme ;
    rdfs:label "Sample type"@en ;
    dcterms:created "2021-06-15" ;
    dcterms:source <http://www.opengis.net/def/entities/bodies/ogcna> ;
    skos:definition "Classification scheme for any kind of Sample classification schemes"@en ;
    skos:prefLabel "Sample type"@en .

<http://www.opengis.net/def/sample-type/OGC/0/by-geometry-type/curve> a skos:Concept ;
    dcterms:created "2021-06-09" ;
    ns1:status <http://www.opengis.net/def/status/valid> ;
    skos:definition "SpatialSample with a Curve geometry as the value of its shape attribute."@en ;
    skos:exactMatch <http://www.opengis.net/def/ogc-om/SF_SamplingCurve>,
        <http://www.opengis.net/def/ogc-om/sf_sampling-curve>,
        <http://www.opengis.net/def/samplingFeatureType/OGC-OM/2.0/SF_SamplingCurve> ;
    skos:inScheme <http://www.opengis.net/def/sample-type/OGC/0/by-geometry-type> ;
    skos:prefLabel "Curve Sample"@en .

<http://www.opengis.net/def/sample-type/OGC/0/by-geometry-type/point> a skos:Concept ;
    dcterms:created "2021-06-09" ;
    ns1:status <http://www.opengis.net/def/status/valid> ;
    skos:definition "SpatialSample with a Point geometry as the value of its shape attribute."@en ;
    skos:exactMatch <http://www.opengis.net/def/ogc-om/SF_SamplingPoint>,
        <http://www.opengis.net/def/ogc-om/sf_sampling-point>,
        <http://www.opengis.net/def/samplingFeatureType/OGC-OM/2.0/SF_SamplingPoint> ;
    skos:inScheme <http://www.opengis.net/def/sample-type/OGC/0/by-geometry-type> ;
    skos:prefLabel "Point Sample"@en .

<http://www.opengis.net/def/sample-type/OGC/0/by-geometry-type/surface> a skos:Concept ;
    dcterms:created "2021-06-09" ;
    ns1:status <http://www.opengis.net/def/status/valid> ;
    skos:definition "SpatialSample with a Surface geometry as the value of its shape attribute."@en ;
    skos:exactMatch <http://www.opengis.net/def/ogc-om/SF_SamplingSurface>,
        <http://www.opengis.net/def/ogc-om/sf_sampling-surface>,
        <http://www.opengis.net/def/samplingFeatureType/OGC-OM/2.0/SF_SamplingSurface> ;
    skos:inScheme <http://www.opengis.net/def/sample-type/OGC/0/by-geometry-type> ;
    skos:prefLabel "Surface Sample"@en .

<http://www.opengis.net/def/observation-type/OGC/0/by-result-type/discrete-coverage-observation> a skos:Concept ;
    dcterms:created "2021-06-09" ;
    ns1:status <http://www.opengis.net/def/status/valid> ;
    skos:definition "Observation whose result is a DiscreteCoverage in the ISO 19123 sense."@en ;
    skos:exactMatch <http://www.opengis.net/def/observation-type/ogc-om/2.0/om_discrete-coverage-observation>,
        <http://www.opengis.net/def/observationType/OGC-OM/2.0/OM_DiscreteCoverageObservation>,
        <http://www.opengis.net/def/ogc-om/OM_DiscreteCoverageObservation> ;
    skos:inScheme <http://www.opengis.net/def/observation-type/OGC/0/by-result-type> ;
    skos:narrower <http://www.opengis.net/def/observation-type/OGC/0/by-result-type/discrete-point-coverage-observation> ;
    skos:prefLabel "Discrete coverage Observation"@en .

<http://www.opengis.net/def/observation-type/OGC/0/by-result-type/discrete-point-coverage-observation> a skos:Concept ;
    dcterms:created "2021-06-09" ;
    ns1:status <http://www.opengis.net/def/status/valid> ;
    skos:broader <http://www.opengis.net/def/observation-type/OGC/0/by-result-type/discrete-coverage-observation> ;
    skos:definition "Observation whose result is a DiscretePointCoverage in the ISO 19123 sense."@en ;
    skos:exactMatch <http://www.opengis.net/def/observation-type/ogc-om/2.0/om_discrete-point-coverage-observation>,
        <http://www.opengis.net/def/observationType/OGC-OM/2.0/OM_DiscretePointCoverageObservation>,
        <http://www.opengis.net/def/ogc-om/OM_DiscretePointCoverageObservation> ;
    skos:inScheme <http://www.opengis.net/def/observation-type/OGC/0/by-result-type> ;
    skos:prefLabel "Discrete point poverage Observation"@en .

<http://www.opengis.net/def/observation-collection-type/OGC/0/by-member-characteristics-semantics> a skos:ConceptScheme ;
    rdfs:label "Collection type by the interpretation of its memberCharacteristics"@en ;
    dcterms:created "2021-06-15" ;
    dcterms:source <http://www.opengis.net/def/entities/bodies/ogcna> ;
    skos:definition "OMS 3.0 ObservationCollection classification scheme based on how the properties of its memberCharacteristics relate to the properties of the member Observations of the collection."@en ;
    skos:inScheme <http://www.opengis.net/def/observation-collection-type> ;
    skos:prefLabel "Collection type by the interpretation of its memberCharacteristics"@en .

<http://www.opengis.net/def/sample-type/OGC/0/by-geometry-type> a skos:ConceptScheme ;
    rdfs:label "SpatialSample by geometry type"@en ;
    dcterms:created "2021-06-09" ;
    dcterms:source <http://www.opengis.net/def/entities/bodies/ogcna> ;
    skos:definition "OMS 3.0 SpatialSample classification scheme based on the geometry type of its shape attribute"@en ;
    skos:inScheme <http://www.opengis.net/def/sample-type> ;
    skos:prefLabel "SpatialSample by geometry type"@en .

<http://www.opengis.net/def/entities/bodies/ogcna> a skos:Concept .

<http://www.opengis.net/def/observation-type/OGC/0/by-result-type> a skos:ConceptScheme ;
    rdfs:label "Observation by result type"@en ;
    dcterms:created "2021-06-09" ;
    dcterms:source <http://www.opengis.net/def/entities/bodies/ogcna> ;
    skos:definition "OMS 3.0 Observation classification scheme based on the type of its result property."@en ;
    skos:inScheme <http://www.opengis.net/def/observation-type> ;
    skos:prefLabel "Observation by result type"@en .

