<?xml version="1.0" encoding="UTF-8"?>
<rdf:RDF
   xmlns:adms="http://www.w3.org/ns/adms#"
   xmlns:dcat="http://www.w3.org/ns/dcat#"
   xmlns:dct="http://purl.org/dc/terms/"
   xmlns:na="http://www.opengis.net/def/metamodel/ogc-na/"
   xmlns:prov="http://www.w3.org/ns/prov#"
   xmlns:rdf="http://www.w3.org/1999/02/22-rdf-syntax-ns#"
   xmlns:reg="http://purl.org/linked-data/registry#"
   xmlns:skos="http://www.w3.org/2004/02/skos/core#"
   xmlns:spec="http://www.opengis.net/def/ont/modspec/"
   xmlns:specrel="http://www.opengis.net/def/ont/specrel/"
>
  <rdf:Description rdf:about="http://www.opengis.net/spec/landinfra/1.0/req/survey">
    <skos:inScheme rdf:resource="http://www.opengis.net/spec/landinfra/1.0"/>
    <skos:broader rdf:resource="http://www.opengis.net/spec/landinfra/1.0/conf/survey"/>
    <skos:broader rdf:resource="http://www.opengis.net/spec/landinfra/1.0/req/land-infra"/>
    <skos:narrower rdf:resource="http://www.opengis.net/spec/landinfra/1.0/req/survey-results"/>
    <skos:narrower rdf:resource="http://www.opengis.net/spec/landinfra/1.0/req/observations"/>
    <skos:narrower rdf:resource="http://www.opengis.net/spec/landinfra/1.0/req/survey-results/topic-20"/>
    <skos:narrower rdf:resource="http://www.opengis.net/spec/landinfra/1.0/req/equipment"/>
    <skos:narrower rdf:resource="http://www.opengis.net/spec/landinfra/1.0/req/survey-results/classes"/>
    <skos:narrower rdf:resource="http://www.opengis.net/spec/landinfra/1.0/req/survey/classes"/>
    <spec:normativeStatement rdf:resource="http://www.opengis.net/spec/landinfra/1.0/req/survey-results/classes"/>
    <spec:normativeStatement rdf:resource="http://www.opengis.net/spec/landinfra/1.0/req/survey-results/topic-20"/>
    <spec:normativeStatement rdf:resource="http://www.opengis.net/spec/landinfra/1.0/req/survey/classes"/>
    <rdf:type rdf:resource="http://www.opengis.net/def/ont/modspec/RequirementClass"/>
    <rdf:type rdf:resource="http://www.w3.org/2004/02/skos/core#Concept"/>
    <skos:prefLabel>Requirement Class: Survey</skos:prefLabel>
    <skos:definition>The Survey Requirements Class is the main survey class and provides a framework for information about observations, processes and their results collected during survey work. The content of this package is similar to the OGC Sensor Model Language (SensorML). The main reason not to use the SensorML standard for this topic is to allow the observation and processes structured in a compact way similar to the LandXML format. Due to the high number of classes the Survey Package was split into different parts, Equipment, Observations and SurveyResults.</skos:definition>
    <spec:dependency rdf:resource="http://www.opengis.net/spec/landinfra/1.0/req/land-infra"/>
  </rdf:Description>
  <rdf:Description rdf:about="http://www.opengis.net/spec/landinfra/1.0/req/observations">
    <skos:inScheme rdf:resource="http://www.opengis.net/spec/landinfra/1.0"/>
    <spec:normativeStatement rdf:resource="http://www.opengis.net/spec/landinfra/1.0/req/observations/classes"/>
    <skos:broader rdf:resource="http://www.opengis.net/spec/landinfra/1.0/conf/observations"/>
    <skos:broader rdf:resource="http://www.opengis.net/spec/landinfra/1.0/req/survey"/>
    <skos:prefLabel>Requirement Class: Observations</skos:prefLabel>
    <rdf:type rdf:resource="http://www.opengis.net/def/ont/modspec/RequirementClass"/>
    <rdf:type rdf:resource="http://www.w3.org/2004/02/skos/core#Concept"/>
    <spec:dependency rdf:resource="http://www.opengis.net/spec/landinfra/1.0/req/survey"/>
    <skos:definition>Observations Requirements class is the package containing all information about the raw observations and the measurements observed during survey work. The raw observations are needed to enable later reprocessing or reporting of resulting properties of the observed feature of interest.</skos:definition>
    <skos:narrower rdf:resource="http://www.opengis.net/spec/landinfra/1.0/req/observations/classes"/>
  </rdf:Description>
  <rdf:Description rdf:about="http://www.opengis.net/spec/landinfra/1.0/conf/road/alignment">
    <skos:prefLabel>Conformance Test: http://www.opengis.net/spec/landinfra/1.0/conf/road/alignment</skos:prefLabel>
    <skos:inScheme rdf:resource="http://www.opengis.net/spec/landinfra/1.0"/>
    <spec:method>Inspect the encoding to verify the above requirement.</spec:method>
    <spec:requirement rdf:resource="http://www.opengis.net/spec/landinfra/1.0/req/road/alignment"/>
    <skos:narrower rdf:resource="http://www.opengis.net/spec/landinfra/1.0/req/road/alignment"/>
    <skos:definition>Verify that if the encoding allows the linear element used for locating RoadElements to be an Alignment, then that encoding supports the Alignment Requirements Class.</skos:definition>
    <spec:testType rdf:resource="http://www.opengis.net/def/ont/modspec/Capabilities"/>
    <rdf:type rdf:resource="http://www.opengis.net/def/ont/modspec/ConformanceTest"/>
    <rdf:type rdf:resource="http://www.w3.org/2004/02/skos/core#Concept"/>
    <skos:broader rdf:resource="http://www.opengis.net/spec/landinfra/1.0/conf/road"/>
    <spec:purpose>Verify that if the encoding allows the linear element used for locating RoadElements to be an Alignment, then that encoding supports the Alignment Requirements Class.</spec:purpose>
  </rdf:Description>
  <rdf:Description rdf:about="http://www.opengis.net/spec/landinfra/1.0/req/project">
    <skos:definition>Facilities include collections of buildings and civil engineering works and their associated siteworks.  The Facilities Requirements Class includes the breakdown of facilities into discipline specific facility parts and introduces the notion of elements which make up these parts.  The Facilities Requirements Class only provides general support for facilities themselves, allowing subsequent Requirements Classes to focus on specific types of the parts that make up facilities, such as road and railway.  This Requirements Class is optional in order to allow for the condition where all of the LandInfra dataset information is not facility related, such as one containing only survey or land division information.</skos:definition>
    <skos:narrower rdf:resource="http://www.opengis.net/spec/landinfra/1.0/req/project/classes"/>
    <spec:dependency rdf:resource="http://www.opengis.net/spec/landinfra/1.0/req/facility"/>
    <rdf:type rdf:resource="http://www.w3.org/2004/02/skos/core#Concept"/>
    <rdf:type rdf:resource="http://www.opengis.net/def/ont/modspec/RequirementClass"/>
    <skos:broader rdf:resource="http://www.opengis.net/spec/landinfra/1.0/conf/project"/>
    <skos:broader rdf:resource="http://www.opengis.net/spec/landinfra/1.0/req/facility"/>
    <skos:prefLabel>Requirement Class: Project</skos:prefLabel>
    <skos:inScheme rdf:resource="http://www.opengis.net/spec/landinfra/1.0"/>
    <spec:normativeStatement rdf:resource="http://www.opengis.net/spec/landinfra/1.0/req/project/classes"/>
  </rdf:Description>
  <rdf:Description rdf:about="http://www.opengis.net/spec/landinfra/1.0/conf/condominium">
    <spec:dependency rdf:resource="http://www.opengis.net/spec/landinfra/1.0/conf/land-division"/>
    <skos:definition>A condominium denotes concurrent ownership of real property that has been divided into private and common portions.  The Condominium Requirements Class includes information about condominium units, buildings and schemes.</skos:definition>
    <skos:prefLabel>Conformance Class: Condominium</skos:prefLabel>
    <skos:narrower rdf:resource="http://www.opengis.net/spec/landinfra/1.0/req/condominium"/>
    <skos:narrower rdf:resource="http://www.opengis.net/spec/landinfra/1.0/conf/condominium/classes"/>
    <spec:requirementsTested rdf:resource="http://www.opengis.net/spec/landinfra/1.0/req/condominium"/>
    <rdf:type rdf:resource="http://www.w3.org/2004/02/skos/core#Concept"/>
    <rdf:type rdf:resource="http://www.opengis.net/def/ont/modspec/ConformanceClass"/>
    <skos:broader rdf:resource="http://www.opengis.net/spec/landinfra/1.0/conf/land-division"/>
    <skos:inScheme rdf:resource="http://www.opengis.net/spec/landinfra/1.0"/>
    <spec:conformanceTest rdf:resource="http://www.opengis.net/spec/landinfra/1.0/conf/condominium/classes"/>
  </rdf:Description>
  <rdf:Description rdf:about="http://www.opengis.net/spec/landinfra/1.0/conf/facility/subtypes">
    <spec:method>Inspect the encoding to verify the above requirement.</spec:method>
    <spec:purpose>Verify that the encoding specifies which of the FacilityPart subtypes shown in Figure 10 it supports.</spec:purpose>
    <skos:broader rdf:resource="http://www.opengis.net/spec/landinfra/1.0/conf/facility"/>
    <skos:narrower rdf:resource="http://www.opengis.net/spec/landinfra/1.0/req/facility/subtypes"/>
    <rdf:type rdf:resource="http://www.w3.org/2004/02/skos/core#Concept"/>
    <rdf:type rdf:resource="http://www.opengis.net/def/ont/modspec/ConformanceTest"/>
    <spec:testType rdf:resource="http://www.opengis.net/def/ont/modspec/Capabilities"/>
    <skos:definition>Verify that the encoding specifies which of the FacilityPart subtypes shown in Figure 10 it supports.</skos:definition>
    <spec:requirement rdf:resource="http://www.opengis.net/spec/landinfra/1.0/req/facility/subtypes"/>
    <skos:prefLabel>ConformanceTest: http://www.opengis.net/spec/landinfra/1.0/conf/facility/subtypes</skos:prefLabel>
    <skos:inScheme rdf:resource="http://www.opengis.net/spec/landinfra/1.0"/>
  </rdf:Description>
  <rdf:Description rdf:about="http://www.opengis.net/spec/landinfra/1.0/conf/land-infra">
    <skos:narrower rdf:resource="http://www.opengis.net/spec/landinfra/1.0/conf/land-infra/topic-19-core"/>
    <skos:narrower rdf:resource="http://www.opengis.net/spec/landinfra/1.0/conf/land-infra/crs"/>
    <skos:narrower rdf:resource="http://www.opengis.net/spec/landinfra/1.0/conf/land-infra/featureID"/>
    <skos:narrower rdf:resource="http://www.opengis.net/spec/landinfra/1.0/conf/land-infra/topic-19-extensions"/>
    <skos:narrower rdf:resource="http://www.opengis.net/spec/landinfra/1.0/conf/land-infra/19109"/>
    <skos:narrower rdf:resource="http://www.opengis.net/spec/landinfra/1.0/conf/land-infra/topic-1"/>
    <skos:narrower rdf:resource="http://www.opengis.net/spec/landinfra/1.0/conf/land-infra/subjects"/>
    <skos:narrower rdf:resource="http://www.opengis.net/spec/landinfra/1.0/conf/survey"/>
    <skos:narrower rdf:resource="http://www.opengis.net/spec/landinfra/1.0/conf/land-division"/>
    <skos:narrower rdf:resource="http://www.opengis.net/spec/landinfra/1.0/conf/land-infra/dataset"/>
    <skos:narrower rdf:resource="http://www.opengis.net/spec/landinfra/1.0/conf/facility"/>
    <skos:narrower rdf:resource="http://www.opengis.net/spec/landinfra/1.0/conf/land-feature"/>
    <skos:narrower rdf:resource="http://www.opengis.net/spec/landinfra/1.0/conf/land-infra/19103"/>
    <skos:narrower rdf:resource="http://www.opengis.net/spec/landinfra/1.0/conf/land-infra/classes"/>
    <skos:narrower rdf:resource="http://www.opengis.net/spec/landinfra/1.0/req/land-infra"/>
    <skos:prefLabel>Core Conformance Class: LandInfra</skos:prefLabel>
    <spec:conformanceTest rdf:resource="http://www.opengis.net/spec/landinfra/1.0/conf/land-infra/topic-19-core"/>
    <spec:conformanceTest rdf:resource="http://www.opengis.net/spec/landinfra/1.0/conf/land-infra/crs"/>
    <spec:conformanceTest rdf:resource="http://www.opengis.net/spec/landinfra/1.0/conf/land-infra/topic-19-extensions"/>
    <spec:conformanceTest rdf:resource="http://www.opengis.net/spec/landinfra/1.0/conf/land-infra/19109"/>
    <spec:conformanceTest rdf:resource="http://www.opengis.net/spec/landinfra/1.0/conf/land-infra/topic-1"/>
    <spec:conformanceTest rdf:resource="http://www.opengis.net/spec/landinfra/1.0/conf/land-infra/subjects"/>
    <spec:conformanceTest rdf:resource="http://www.opengis.net/spec/landinfra/1.0/conf/land-infra/dataset"/>
    <spec:conformanceTest rdf:resource="http://www.opengis.net/spec/landinfra/1.0/conf/land-infra/19103"/>
    <spec:conformanceTest rdf:resource="http://www.opengis.net/spec/landinfra/1.0/conf/land-infra/featureID"/>
    <spec:conformanceTest rdf:resource="http://www.opengis.net/spec/landinfra/1.0/conf/land-infra/classes"/>
    <rdf:type rdf:resource="http://www.opengis.net/def/ont/modspec/ConformanceClass"/>
    <rdf:type rdf:resource="http://www.w3.org/2004/02/skos/core#Concept"/>
    <skos:definition>LandInfra is the core Requirements Class and is the only mandatory Requirements Class.  This class contains information about the Land and Infrastructure dataset that can contain information about facilities, land features, land division, documents, survey marks, surveys, sets, and feature associations.  LandInfra also contains the definition of types common across other Requirements Classes, such as the Status CodeList.</skos:definition>
    <skos:inScheme rdf:resource="http://www.opengis.net/spec/landinfra/1.0"/>
    <skos:topConceptOf rdf:resource="http://www.opengis.net/spec/landinfra/1.0"/>
    <spec:requirementsTested rdf:resource="http://www.opengis.net/spec/landinfra/1.0/req/land-infra"/>
  </rdf:Description>
  <rdf:Description rdf:about="http://www.opengis.net/spec/landinfra/1.0/conf/land-infra/classes">
    <rdf:type rdf:resource="http://www.w3.org/2004/02/skos/core#Concept"/>
    <rdf:type rdf:resource="http://www.opengis.net/def/ont/modspec/ConformanceTest"/>
    <spec:testType rdf:resource="http://www.opengis.net/def/ont/modspec/Capabilities"/>
    <skos:prefLabel>Conformance Test: http://www.opengis.net/spec/landinfra/1.0/conf/land-infra/classes</skos:prefLabel>
    <spec:requirement rdf:resource="http://www.opengis.net/spec/landinfra/1.0/req/land-infra/classes"/>
    <skos:broader rdf:resource="http://www.opengis.net/spec/landinfra/1.0/conf/land-infra"/>
    <skos:narrower rdf:resource="http://www.opengis.net/spec/landinfra/1.0/req/land-infra/classes"/>
    <skos:inScheme rdf:resource="http://www.opengis.net/spec/landinfra/1.0"/>
    <spec:method>Inspect the encoding to verify the above requirement.</spec:method>
    <skos:definition>Verify that theencoding provides the LandInfra Requirements Class Classes shown in blue in Figure 2 in a manner consistent with the encoding.</skos:definition>
    <spec:purpose>Verify that theencoding provides the LandInfra Requirements Class Classes shown in blue in Figure 2 in a manner consistent with the encoding.</spec:purpose>
  </rdf:Description>
  <rdf:Description rdf:about="http://www.opengis.net/spec/landinfra/1.0">
    <skos:hasTopConcept rdf:resource="http://www.opengis.net/spec/landinfra/1.0/conf/land-infra"/>
    <skos:hasTopConcept rdf:resource="http://www.opengis.net/spec/landinfra/1.0/conf/alignment"/>
    <skos:hasTopConcept rdf:resource="http://www.opengis.net/spec/landinfra/1.0/conf/facility"/>
    <dct:source rdf:resource="http://www.opengis.net/def/docs/15-111r1"/>
    <skos:definition>A convenience hierarchy for navigating the elements of a specification using the SKOS model</skos:definition>
    <dct:modified rdf:datatype="http://www.w3.org/2001/XMLSchema#date">2016-12-20</dct:modified>
    <spec:status rdf:resource="http://www.opengis.net/def/status/experimental"/>
    <dct:created rdf:datatype="http://www.w3.org/2001/XMLSchema#date">2016-12-20</dct:created>
    <na:status rdf:resource="http://www.opengis.net/def/status/experimental"/>
    <skos:prefLabel>Specification elements for OGC 15-111r LandInfra</skos:prefLabel>
    <rdf:type rdf:resource="http://www.w3.org/2004/02/skos/core#ConceptScheme"/>
  </rdf:Description>
  <rdf:Description rdf:about="http://www.opengis.net/spec/landinfra/1.0/conf/road-cross-section/classes">
    <spec:method>Inspect the encoding to verify the above requirement.</spec:method>
    <spec:testType rdf:resource="http://www.opengis.net/def/ont/modspec/Capabilities"/>
    <rdf:type rdf:resource="http://www.opengis.net/def/ont/modspec/ConformanceTest"/>
    <rdf:type rdf:resource="http://www.w3.org/2004/02/skos/core#Concept"/>
    <skos:prefLabel>Conformance Test: http://www.opengis.net/spec/landinfra/1.0/conf/road-cross-section/classes</skos:prefLabel>
    <spec:requirement rdf:resource="http://www.opengis.net/spec/landinfra/1.0/req/road-cross-section/classes"/>
    <spec:purpose>Verify that the encoding provides the RoadCrossSection Requirements Class Classes shown in blue in Figure 25 in a manner consistent with the encoding.</spec:purpose>
    <skos:narrower rdf:resource="http://www.opengis.net/spec/landinfra/1.0/req/road-cross-section/classes"/>
    <skos:definition>Verify that the encoding provides the RoadCrossSection Requirements Class Classes shown in blue in Figure 25 in a manner consistent with the encoding.</skos:definition>
    <skos:broader rdf:resource="http://www.opengis.net/spec/landinfra/1.0/conf/road-cross-section"/>
    <skos:inScheme rdf:resource="http://www.opengis.net/spec/landinfra/1.0"/>
  </rdf:Description>
  <rdf:Description rdf:about="http://www.opengis.net/spec/landinfra/1.0/req/project/classes">
    <skos:broader rdf:resource="http://www.opengis.net/spec/landinfra/1.0/conf/project/classes"/>
    <skos:broader rdf:resource="http://www.opengis.net/spec/landinfra/1.0/req/project"/>
    <skos:prefLabel>Requirement: /req/project/classes</skos:prefLabel>
    <rdf:type rdf:resource="http://www.opengis.net/def/ont/modspec/Requirement"/>
    <rdf:type rdf:resource="http://www.w3.org/2004/02/skos/core#Concept"/>
    <skos:definition>The Project Requirements Class Classes shown in blue in Figure 13 shall be provided for by the encoding in a manner consistent with the encoding.</skos:definition>
    <skos:inScheme rdf:resource="http://www.opengis.net/spec/landinfra/1.0"/>
  </rdf:Description>
  <rdf:Description rdf:about="http://www.opengis.net/spec/landinfra/1.0/conf/survey/classes">
    <skos:definition>Verify that the encoding provides the Survey Requirements Class Classes shown in blue in Figure 41 in a manner consistent with the encoding.</skos:definition>
    <spec:method>Inspect the encoding to verify the above requirement.</spec:method>
    <spec:testType rdf:resource="http://www.opengis.net/def/ont/modspec/Capabilities"/>
    <skos:prefLabel>Conformance Test: http://www.opengis.net/spec/landinfra/1.0/conf/survey/classes</skos:prefLabel>
    <skos:narrower rdf:resource="http://www.opengis.net/spec/landinfra/1.0/req/survey/classes"/>
    <skos:broader rdf:resource="http://www.opengis.net/spec/landinfra/1.0/conf/survey"/>
    <rdf:type rdf:resource="http://www.opengis.net/def/ont/modspec/ConformanceTest"/>
    <rdf:type rdf:resource="http://www.w3.org/2004/02/skos/core#Concept"/>
    <spec:requirement rdf:resource="http://www.opengis.net/spec/landinfra/1.0/req/survey/classes"/>
    <spec:purpose>Verify that the encoding provides the Survey Requirements Class Classes shown in blue in Figure 41 in a manner consistent with the encoding.</spec:purpose>
    <skos:inScheme rdf:resource="http://www.opengis.net/spec/landinfra/1.0"/>
  </rdf:Description>
  <rdf:Description rdf:about="http://www.opengis.net/spec/landinfra/1.0/conf/condominium/classes">
    <skos:narrower rdf:resource="http://www.opengis.net/spec/landinfra/1.0/req/condominium/classes"/>
    <spec:method>Inspect the encoding to verify the above requirement.</spec:method>
    <rdf:type rdf:resource="http://www.w3.org/2004/02/skos/core#Concept"/>
    <rdf:type rdf:resource="http://www.opengis.net/def/ont/modspec/ConformanceTest"/>
    <skos:inScheme rdf:resource="http://www.opengis.net/spec/landinfra/1.0"/>
    <spec:testType rdf:resource="http://www.opengis.net/def/ont/modspec/Capabilities"/>
    <spec:requirement rdf:resource="http://www.opengis.net/spec/landinfra/1.0/req/condominium/classes"/>
    <skos:definition>Verify that the encoding provides the Condominium Requirements Class Classes shown in blue in Figure 68 in a manner consistent with the encoding.</skos:definition>
    <skos:broader rdf:resource="http://www.opengis.net/spec/landinfra/1.0/conf/condominium"/>
    <spec:purpose>Verify that the encoding provides the Condominium Requirements Class Classes shown in blue in Figure 68 in a manner consistent with the encoding.</spec:purpose>
    <skos:prefLabel>Conformance Test: http://www.opengis.net/spec/landinfra/1.0/conf/condominium/classes</skos:prefLabel>
  </rdf:Description>
  <rdf:Description rdf:about="http://www.opengis.net/spec/landinfra/1.0/conf/alignment">
    <spec:conformanceTest rdf:resource="http://www.opengis.net/spec/landinfra/1.0/conf/alignment/LR-interfaces"/>
    <spec:conformanceTest rdf:resource="http://www.opengis.net/spec/landinfra/1.0/conf/alignment/measures"/>
    <spec:conformanceTest rdf:resource="http://www.opengis.net/spec/landinfra/1.0/conf/alignment/classes"/>
    <spec:conformanceTest rdf:resource="http://www.opengis.net/spec/landinfra/1.0/conf/alignment/description"/>
    <spec:conformanceTest rdf:resource="http://www.opengis.net/spec/landinfra/1.0/conf/alignment/CRS"/>
    <skos:inScheme rdf:resource="http://www.opengis.net/spec/landinfra/1.0"/>
    <skos:narrower rdf:resource="http://www.opengis.net/spec/landinfra/1.0/conf/alignment/CRS"/>
    <skos:narrower rdf:resource="http://www.opengis.net/spec/landinfra/1.0/conf/alignment/LR-interfaces"/>
    <skos:narrower rdf:resource="http://www.opengis.net/spec/landinfra/1.0/conf/alignment/measures"/>
    <skos:narrower rdf:resource="http://www.opengis.net/spec/landinfra/1.0/req/alignment"/>
    <skos:narrower rdf:resource="http://www.opengis.net/spec/landinfra/1.0/conf/alignment/classes"/>
    <skos:narrower rdf:resource="http://www.opengis.net/spec/landinfra/1.0/conf/alignment/description"/>
    <spec:dependency rdf:resource="http://www.opengis.net/spec/landinfra/1.0/conf/facility"/>
    <skos:definition>An alignment is a positioning element which provides a Linear Referencing System for locating physical elements.  The Alignment Requirements Class specifies how an alignment is defined and used.</skos:definition>
    <spec:requirementsTested rdf:resource="http://www.opengis.net/spec/landinfra/1.0/req/alignment"/>
    <rdf:type rdf:resource="http://www.w3.org/2004/02/skos/core#Concept"/>
    <rdf:type rdf:resource="http://www.opengis.net/def/ont/modspec/ConformanceClass"/>
    <skos:prefLabel>Conformance Class: Alignment</skos:prefLabel>
    <skos:broader rdf:resource="http://www.opengis.net/spec/landinfra/1.0/conf/facility"/>
  </rdf:Description>
  <rdf:Description rdf:about="http://www.opengis.net/spec/landinfra/1.0/conf/road-cross-section/alignment">
    <rdf:type rdf:resource="http://www.w3.org/2004/02/skos/core#Concept"/>
    <rdf:type rdf:resource="http://www.opengis.net/def/ont/modspec/ConformanceTest"/>
    <spec:purpose>Verify that if the encoding allows the linear element used for locating CrossSections to be an Alignment, then that encoding supports the Alignment Requirements Class.</spec:purpose>
    <spec:requirement rdf:resource="http://www.opengis.net/spec/landinfra/1.0/req/road-cross-section/alignment"/>
    <skos:broader rdf:resource="http://www.opengis.net/spec/landinfra/1.0/conf/road-cross-section"/>
    <skos:definition>Verify that if the encoding allows the linear element used for locating CrossSections to be an Alignment, then that encoding supports the Alignment Requirements Class.</skos:definition>
    <spec:method>Inspect the encoding to verify the above requirement.</spec:method>
    <skos:inScheme rdf:resource="http://www.opengis.net/spec/landinfra/1.0"/>
    <spec:testType rdf:resource="http://www.opengis.net/def/ont/modspec/Capabilities"/>
    <skos:narrower rdf:resource="http://www.opengis.net/spec/landinfra/1.0/req/road-cross-section/alignment"/>
    <skos:prefLabel>Conformance Test: http://www.opengis.net/spec/landinfra/1.0/conf/road-cross-section/alignment</skos:prefLabel>
  </rdf:Description>
  <rdf:Description rdf:about="http://www.opengis.net/spec/landinfra/1.0/req/railway/alignment">
    <skos:broader rdf:resource="http://www.opengis.net/spec/landinfra/1.0/req/railway"/>
    <skos:broader rdf:resource="http://www.opengis.net/spec/landinfra/1.0/conf/railway/alignment"/>
    <skos:definition>If an encoding allows the linear element used for locating RailwayElements or CantEvents to be an Alignment, then that encoding shall support the Alignment Requirements Class.</skos:definition>
    <rdf:type rdf:resource="http://www.w3.org/2004/02/skos/core#Concept"/>
    <rdf:type rdf:resource="http://www.opengis.net/def/ont/modspec/Requirement"/>
    <skos:inScheme rdf:resource="http://www.opengis.net/spec/landinfra/1.0"/>
    <skos:prefLabel>Requirement: /req/railway/alignment</skos:prefLabel>
  </rdf:Description>
  <rdf:Description rdf:about="http://www.opengis.net/def/docs/15-111r1">
    <rdf:type rdf:resource="http://www.w3.org/2004/02/skos/core#Concept"/>
    <rdf:type rdf:resource="http://www.opengis.net/def/ont/modspec/Specification"/>
    <prov:wasAttributedTo rdf:resource="http://www.opengis.net/def/wg/landinfraswg"/>
    <dct:dateSubmitted rdf:datatype="http://www.w3.org/2001/XMLSchema#date">2016-05-16</dct:dateSubmitted>
    <dct:creator>Paul Scarponcini</dct:creator>
    <spec:class rdf:resource="http://www.opengis.net/spec/landinfra/1.0/conf/observations"/>
    <spec:class rdf:resource="http://www.opengis.net/spec/landinfra/1.0/conf/facility"/>
    <spec:class rdf:resource="http://www.opengis.net/spec/landinfra/1.0/conf/land-infra"/>
    <spec:class rdf:resource="http://www.opengis.net/spec/landinfra/1.0/conf/land-feature"/>
    <spec:class rdf:resource="http://www.opengis.net/spec/landinfra/1.0/conf/survey-results"/>
    <spec:class rdf:resource="http://www.opengis.net/spec/landinfra/1.0/conf/project"/>
    <spec:class rdf:resource="http://www.opengis.net/spec/landinfra/1.0/conf/road"/>
    <spec:class rdf:resource="http://www.opengis.net/spec/landinfra/1.0/conf/condominium"/>
    <spec:class rdf:resource="http://www.opengis.net/spec/landinfra/1.0/conf/alignment"/>
    <spec:class rdf:resource="http://www.opengis.net/spec/landinfra/1.0/conf/road-cross-section"/>
    <spec:class rdf:resource="http://www.opengis.net/spec/landinfra/1.0/conf/equipment"/>
    <spec:class rdf:resource="http://www.opengis.net/spec/landinfra/1.0/conf/survey"/>
    <spec:class rdf:resource="http://www.opengis.net/spec/landinfra/1.0/conf/railway"/>
    <spec:class rdf:resource="http://www.opengis.net/spec/landinfra/1.0/conf/land-division"/>
    <reg:status rdf:resource="http://purl.org/linked-data/registry#statusValid"/>
    <specrel:implementation rdf:resource="http://www.opengis.net/def/docs/16-105r2"/>
    <specrel:implementation rdf:resource="http://www.opengis.net/def/docs/16-101r2"/>
    <specrel:implementation rdf:resource="http://www.opengis.net/def/docs/16-000r1"/>
    <specrel:implementation rdf:resource="http://www.opengis.net/def/docs/16-102r2"/>
    <specrel:implementation rdf:resource="http://www.opengis.net/def/docs/16-107r2"/>
    <specrel:implementation rdf:resource="http://www.opengis.net/def/docs/16-103r2"/>
    <specrel:implementation rdf:resource="http://www.opengis.net/def/docs/16-100r2"/>
    <specrel:implementation rdf:resource="http://www.opengis.net/def/docs/16-104r2"/>
    <specrel:implementation rdf:resource="http://www.opengis.net/def/docs/16-106r2"/>
    <na:status rdf:resource="http://www.opengis.net/def/status/valid"/>
    <skos:prefLabel>OGC Land and Infrastructure Conceptual Model Standard (LandInfra)</skos:prefLabel>
    <dct:identifier>http://www.opengis.net/doc/is/landinfra/1.0</dct:identifier>
    <dcat:landingPage rdf:resource="http://docs.opengeospatial.org/is/15-111r1/15-111r1.html"/>
    <dct:dateAccepted rdf:datatype="http://www.w3.org/2001/XMLSchema#date">2016-08-02</dct:dateAccepted>
    <skos:inScheme rdf:resource="http://www.opengis.net/def/docs"/>
    <adms:version>1.0</adms:version>
    <na:doctype rdf:resource="http://www.opengis.net/def/doc-type/ip"/>
    <spec:date rdf:datatype="http://www.w3.org/2001/XMLSchema#date">2016-12-20</spec:date>
    <skos:definition>OGC Land and Infrastructure Conceptual Model Standard (LandInfra)</skos:definition>
    <skos:notation rdf:datatype="http://www.opengis.net/def/metamodel/ogc-na/doc_no">15-111r1</skos:notation>
    <spec:status rdf:resource="http://www.opengis.net/def/status/valid"/>
    <adms:last rdf:resource="http://www.opengis.net/def/docs/15-111r1"/>
    <spec:authority>Open Geospatial Consortium</spec:authority>
  </rdf:Description>
  <rdf:Description rdf:about="http://www.opengis.net/spec/landinfra/1.0/conf/survey-results">
    <spec:requirementsTested rdf:resource="http://www.opengis.net/spec/landinfra/1.0/req/survey-results"/>
    <spec:dependency rdf:resource="http://www.opengis.net/spec/landinfra/1.0/conf/survey"/>
    <skos:narrower rdf:resource="http://www.opengis.net/spec/landinfra/1.0/conf/survey-results/classes"/>
    <skos:narrower rdf:resource="http://www.opengis.net/spec/landinfra/1.0/conf/survey-results/topic-20"/>
    <skos:narrower rdf:resource="http://www.opengis.net/spec/landinfra/1.0/req/survey-results"/>
    <spec:conformanceTest rdf:resource="http://www.opengis.net/spec/landinfra/1.0/conf/survey-results/classes"/>
    <spec:conformanceTest rdf:resource="http://www.opengis.net/spec/landinfra/1.0/conf/survey-results/topic-20"/>
    <skos:prefLabel>Conformance Class: Survey Results</skos:prefLabel>
    <skos:definition>The SurveyResults Requirements Class contains the observed property of a feature of interest.  Using sampling features from the Observation &amp; Measurements (O&amp;M) standard, the dependencies between the observation acts and the results are realized.</skos:definition>
    <rdf:type rdf:resource="http://www.w3.org/2004/02/skos/core#Concept"/>
    <rdf:type rdf:resource="http://www.opengis.net/def/ont/modspec/ConformanceClass"/>
    <skos:inScheme rdf:resource="http://www.opengis.net/spec/landinfra/1.0"/>
    <skos:broader rdf:resource="http://www.opengis.net/spec/landinfra/1.0/conf/survey"/>
  </rdf:Description>
  <rdf:Description rdf:about="http://www.opengis.net/spec/landinfra/1.0/req/alignment">
    <skos:inScheme rdf:resource="http://www.opengis.net/spec/landinfra/1.0"/>
    <spec:dependency rdf:resource="http://www.opengis.net/spec/landinfra/1.0/req/facility"/>
    <rdf:type rdf:resource="http://www.w3.org/2004/02/skos/core#Concept"/>
    <rdf:type rdf:resource="http://www.opengis.net/def/ont/modspec/RequirementClass"/>
    <spec:normativeStatement rdf:resource="http://www.opengis.net/spec/landinfra/1.0/req/alignment/description"/>
    <spec:normativeStatement rdf:resource="http://www.opengis.net/spec/landinfra/1.0/req/alignment/classes"/>
    <spec:normativeStatement rdf:resource="http://www.opengis.net/spec/landinfra/1.0/req/alignment/CRS"/>
    <spec:normativeStatement rdf:resource="http://www.opengis.net/spec/landinfra/1.0/req/alignment/LR-interfaces"/>
    <spec:normativeStatement rdf:resource="http://www.opengis.net/spec/landinfra/1.0/req/alignment/measures"/>
    <skos:narrower rdf:resource="http://www.opengis.net/spec/landinfra/1.0/req/alignment/measures"/>
    <skos:narrower rdf:resource="http://www.opengis.net/spec/landinfra/1.0/req/alignment/CRS"/>
    <skos:narrower rdf:resource="http://www.opengis.net/spec/landinfra/1.0/req/alignment/LR-interfaces"/>
    <skos:narrower rdf:resource="http://www.opengis.net/spec/landinfra/1.0/req/alignment/description"/>
    <skos:narrower rdf:resource="http://www.opengis.net/spec/landinfra/1.0/req/alignment/classes"/>
    <skos:broader rdf:resource="http://www.opengis.net/spec/landinfra/1.0/req/facility"/>
    <skos:broader rdf:resource="http://www.opengis.net/spec/landinfra/1.0/conf/alignment"/>
    <skos:prefLabel>Requirement Class: Alignment</skos:prefLabel>
    <skos:definition>An alignment is a positioning element which provides a Linear Referencing System for locating physical elements.  The Alignment Requirements Class specifies how an alignment is defined and used.</skos:definition>
  </rdf:Description>
  <rdf:Description rdf:about="http://www.opengis.net/spec/landinfra/1.0/req/road-cross-section/alignment">
    <skos:prefLabel>Requirement: /req/road-cross-section/alignment</skos:prefLabel>
    <skos:definition>If an encoding allows the linear element used for locating CrossSections to be an Alignment, then that encoding shall support the Alignment Requirements Class.</skos:definition>
    <skos:broader rdf:resource="http://www.opengis.net/spec/landinfra/1.0/req/road-cross-section"/>
    <skos:broader rdf:resource="http://www.opengis.net/spec/landinfra/1.0/req/road"/>
    <skos:broader rdf:resource="http://www.opengis.net/spec/landinfra/1.0/conf/road-cross-section/alignment"/>
    <skos:inScheme rdf:resource="http://www.opengis.net/spec/landinfra/1.0"/>
    <rdf:type rdf:resource="http://www.opengis.net/def/ont/modspec/Requirement"/>
    <rdf:type rdf:resource="http://www.w3.org/2004/02/skos/core#Concept"/>
  </rdf:Description>
  <rdf:Description rdf:about="http://www.opengis.net/spec/landinfra/1.0/req/survey-results">
    <skos:broader rdf:resource="http://www.opengis.net/spec/landinfra/1.0/req/survey"/>
    <skos:broader rdf:resource="http://www.opengis.net/spec/landinfra/1.0/conf/survey-results"/>
    <skos:narrower rdf:resource="http://www.opengis.net/spec/landinfra/1.0/req/survey-results/classes"/>
    <skos:narrower rdf:resource="http://www.opengis.net/spec/landinfra/1.0/req/survey-results/topic-20"/>
    <spec:normativeStatement rdf:resource="http://www.opengis.net/spec/landinfra/1.0/req/survey-results/topic-20"/>
    <spec:normativeStatement rdf:resource="http://www.opengis.net/spec/landinfra/1.0/req/survey-results/classes"/>
    <skos:prefLabel>Requirement Class: SurveyResult</skos:prefLabel>
    <skos:inScheme rdf:resource="http://www.opengis.net/spec/landinfra/1.0"/>
    <rdf:type rdf:resource="http://www.opengis.net/def/ont/modspec/RequirementClass"/>
    <rdf:type rdf:resource="http://www.w3.org/2004/02/skos/core#Concept"/>
    <spec:dependency rdf:resource="http://www.opengis.net/spec/landinfra/1.0/req/survey"/>
    <skos:definition>The SurveyResults Requirements Class contains the observed property of a feature of interest.  Using sampling features from the Observation &amp; Measurements (O&amp;M) standard, the dependencies between the observation acts and the results are realized.</skos:definition>
  </rdf:Description>
  <rdf:Description rdf:about="http://www.opengis.net/spec/landinfra/1.0/">
    <dct:source rdf:resource="http://www.opengis.net/def/docs/15-111r1"/>
    <skos:definition>LandInfra conceptual model collection of Conformance Classes</skos:definition>
    <rdf:type rdf:resource="http://www.w3.org/2004/02/skos/core#Collection"/>
  </rdf:Description>
  <rdf:Description rdf:about="http://www.opengis.net/spec/landinfra/1.0/conf/land-infra/19103">
    <spec:method>Inspect the encoding to verify the above requirement.</spec:method>
    <spec:testType rdf:resource="http://www.opengis.net/def/ont/modspec/Capabilities"/>
    <rdf:type rdf:resource="http://www.opengis.net/def/ont/modspec/ConformanceTest"/>
    <rdf:type rdf:resource="http://www.w3.org/2004/02/skos/core#Concept"/>
    <skos:broader rdf:resource="http://www.opengis.net/spec/landinfra/1.0/conf/land-infra"/>
    <skos:prefLabel>Conformance Test: http://www.opengis.net/spec/landinfra/1.0/conf/land-infra/19103</skos:prefLabel>
    <spec:purpose>Verify that the encoding provides the core data types specified in ISO 19103 Clause 7 and shown in pink in Figure 5 that are appropriate to the supported subject area(s).</spec:purpose>
    <skos:definition>Verify that the encoding provides the core data types specified in ISO 19103 Clause 7 and shown in pink in Figure 5 that are appropriate to the supported subject area(s).</skos:definition>
    <spec:requirement rdf:resource="http://www.opengis.net/spec/landinfra/1.0/req/land-infra/19103"/>
    <skos:narrower rdf:resource="http://www.opengis.net/spec/landinfra/1.0/req/land-infra/19103"/>
    <skos:inScheme rdf:resource="http://www.opengis.net/spec/landinfra/1.0"/>
  </rdf:Description>
  <rdf:Description rdf:about="http://www.opengis.net/spec/landinfra/1.0/conf/equipment/observation-correction">
    <skos:broader rdf:resource="http://www.opengis.net/spec/landinfra/1.0/conf/equipment"/>
    <spec:testType rdf:resource="http://www.opengis.net/def/ont/modspec/Capabilities"/>
    <spec:requirement rdf:resource="http://www.opengis.net/spec/landinfra/1.0/req/equipment/observation-correction"/>
    <skos:narrower rdf:resource="http://www.opengis.net/spec/landinfra/1.0/req/equipment/observation-correction"/>
    <spec:purpose>Verify that the encoding provides the ObservationCorrection Classes in blue in Figure 51 in a manner consistent with the encoding.  The encoding shall decide which correction types it will support and define appropriate requirements classes accordingly.</spec:purpose>
    <skos:inScheme rdf:resource="http://www.opengis.net/spec/landinfra/1.0"/>
    <rdf:type rdf:resource="http://www.w3.org/2004/02/skos/core#Concept"/>
    <rdf:type rdf:resource="http://www.opengis.net/def/ont/modspec/ConformanceTest"/>
    <skos:prefLabel>Conformance Test: http://www.opengis.net/spec/landinfra/1.0/conf/equipment/observation-correction</skos:prefLabel>
    <spec:method>Inspect the encoding to verify the above requirement.</spec:method>
    <skos:definition>Verify that the encoding provides the ObservationCorrection Classes in blue in Figure 51 in a manner consistent with the encoding.  The encoding shall decide which correction types it will support and define appropriate requirements classes accordingly.</skos:definition>
  </rdf:Description>
  <rdf:Description rdf:about="http://www.opengis.net/spec/landinfra/1.0/conf/land-division">
    <skos:prefLabel>Conformance Class: LandDivision</skos:prefLabel>
    <skos:broader rdf:resource="http://www.opengis.net/spec/landinfra/1.0/conf/land-infra"/>
    <skos:inScheme rdf:resource="http://www.opengis.net/spec/landinfra/1.0"/>
    <skos:narrower rdf:resource="http://www.opengis.net/spec/landinfra/1.0/req/land-division"/>
    <skos:narrower rdf:resource="http://www.opengis.net/spec/landinfra/1.0/conf/land-division/classes"/>
    <skos:narrower rdf:resource="http://www.opengis.net/spec/landinfra/1.0/conf/condominium"/>
    <spec:requirementsTested rdf:resource="http://www.opengis.net/spec/landinfra/1.0/req/land-division"/>
    <spec:conformanceTest rdf:resource="http://www.opengis.net/spec/landinfra/1.0/conf/land-division/classes"/>
    <skos:definition>Land can be divided up into land divisions.  These can either be public (political, judicial, or executive) or private in nature.  The former are administrative divisions and the latter are interests in land.  Both of these are specified in the LandDivision Requirements Class, though condominium interests in land are specified in a separate, Condominium Requirements Class.</skos:definition>
    <rdf:type rdf:resource="http://www.w3.org/2004/02/skos/core#Concept"/>
    <rdf:type rdf:resource="http://www.opengis.net/def/ont/modspec/ConformanceClass"/>
    <spec:dependency rdf:resource="http://www.opengis.net/spec/landinfra/1.0/conf/land-infra"/>
  </rdf:Description>
  <rdf:Description rdf:about="http://www.opengis.net/spec/landinfra/1.0/conf/observations">
    <rdf:type rdf:resource="http://www.w3.org/2004/02/skos/core#Concept"/>
    <rdf:type rdf:resource="http://www.opengis.net/def/ont/modspec/ConformanceClass"/>
    <spec:requirementsTested rdf:resource="http://www.opengis.net/spec/landinfra/1.0/req/observations"/>
    <skos:definition>Observations Requirements class is the package containing all information about the raw observations and the measurements observed during survey work. The raw observations are needed to enable later reprocessing or reporting of resulting properties of the observed feature of interest.</skos:definition>
    <skos:inScheme rdf:resource="http://www.opengis.net/spec/landinfra/1.0"/>
    <skos:prefLabel>Conformance Class: Observations</skos:prefLabel>
    <skos:broader rdf:resource="http://www.opengis.net/spec/landinfra/1.0/conf/survey"/>
    <skos:narrower rdf:resource="http://www.opengis.net/spec/landinfra/1.0/req/observations"/>
    <skos:narrower rdf:resource="http://www.opengis.net/spec/landinfra/1.0/conf/observations/classes"/>
    <spec:dependency rdf:resource="http://www.opengis.net/spec/landinfra/1.0/conf/survey"/>
    <spec:conformanceTest rdf:resource="http://www.opengis.net/spec/landinfra/1.0/conf/observations/classes"/>
  </rdf:Description>
  <rdf:Description rdf:about="http://www.opengis.net/spec/landinfra/1.0/req/land-infra/classes">
    <rdf:type rdf:resource="http://www.w3.org/2004/02/skos/core#Concept"/>
    <rdf:type rdf:resource="http://www.opengis.net/def/ont/modspec/Requirement"/>
    <skos:broader rdf:resource="http://www.opengis.net/spec/landinfra/1.0/conf/land-infra/classes"/>
    <skos:broader rdf:resource="http://www.opengis.net/spec/landinfra/1.0/req/land-infra"/>
    <skos:inScheme rdf:resource="http://www.opengis.net/spec/landinfra/1.0"/>
    <skos:prefLabel>Requirement: /req/land-infra/classes</skos:prefLabel>
    <skos:definition>The LandInfra Requirements Class Classes shown in blue in Figure 2 shall be provided by the encoding in a manner consistent with the encoding.</skos:definition>
  </rdf:Description>
  <rdf:Description rdf:about="http://www.opengis.net/spec/landinfra/1.0/conf/land-infra/subjects">
    <skos:inScheme rdf:resource="http://www.opengis.net/spec/landinfra/1.0"/>
    <spec:requirement rdf:resource="http://www.opengis.net/spec/landinfra/1.0/req/land-infra/subjects"/>
    <spec:testType rdf:resource="http://www.opengis.net/def/ont/modspec/Capabilities"/>
    <skos:narrower rdf:resource="http://www.opengis.net/spec/landinfra/1.0/req/land-infra/subjects"/>
    <skos:definition>Verify that the encoding specifies which of the LandInfra subjects it supports.</skos:definition>
    <rdf:type rdf:resource="http://www.w3.org/2004/02/skos/core#Concept"/>
    <rdf:type rdf:resource="http://www.opengis.net/def/ont/modspec/ConformanceTest"/>
    <skos:broader rdf:resource="http://www.opengis.net/spec/landinfra/1.0/conf/land-infra"/>
    <spec:purpose>Verify that the encoding specifies which of the LandInfra subjects it supports.</spec:purpose>
    <skos:prefLabel>Conformance Test: http://www.opengis.net/spec/landinfra/1.0/conf/land-infra/subjects</skos:prefLabel>
    <spec:method>Inspect the encoding to verify the above requirement.</spec:method>
  </rdf:Description>
  <rdf:Description rdf:about="http://www.opengis.net/spec/landinfra/1.0/req/alignment/LR-interfaces">
    <skos:prefLabel>Requirement: /req/alignment/LR-interfaces</skos:prefLabel>
    <rdf:type rdf:resource="http://www.opengis.net/def/ont/modspec/Requirement"/>
    <rdf:type rdf:resource="http://www.w3.org/2004/02/skos/core#Concept"/>
    <skos:broader rdf:resource="http://www.opengis.net/spec/landinfra/1.0/conf/alignment/LR-interfaces"/>
    <skos:broader rdf:resource="http://www.opengis.net/spec/landinfra/1.0/req/alignment"/>
    <skos:inScheme rdf:resource="http://www.opengis.net/spec/landinfra/1.0"/>
    <skos:definition>An encoding shall implement the OGC Abstract Specification Topic 19 ILinearElement and ISpatial interfaces in a manner consistent with the encoding.</skos:definition>
  </rdf:Description>
  <rdf:Description rdf:about="http://www.opengis.net/spec/landinfra/1.0/req/land-infra/featureID">
    <skos:broader rdf:resource="http://www.opengis.net/spec/landinfra/1.0/conf/land-infra/featureID"/>
    <skos:broader rdf:resource="http://www.opengis.net/spec/landinfra/1.0/req/land-infra"/>
    <skos:inScheme rdf:resource="http://www.opengis.net/spec/landinfra/1.0"/>
    <rdf:type rdf:resource="http://www.opengis.net/def/ont/modspec/Requirement"/>
    <rdf:type rdf:resource="http://www.w3.org/2004/02/skos/core#Concept"/>
    <skos:definition>An encoding shall specify if it supports ID at the feature level, ID at the Feature sub-type level, or both.</skos:definition>
    <skos:prefLabel>Requirement: /req/land-infra/featureID</skos:prefLabel>
  </rdf:Description>
  <rdf:Description rdf:about="http://www.opengis.net/spec/landinfra/1.0/conf/survey">
    <skos:inScheme rdf:resource="http://www.opengis.net/spec/landinfra/1.0"/>
    <rdf:type rdf:resource="http://www.opengis.net/def/ont/modspec/ConformanceClass"/>
    <rdf:type rdf:resource="http://www.w3.org/2004/02/skos/core#Concept"/>
    <skos:definition>The Survey Requirements Class is the main survey class and provides a framework for information about observations, processes and their results collected during survey work. The content of this package is similar to the OGC Sensor Model Language (SensorML). The main reason not to use the SensorML standard for this topic is to allow the observation and processes structured in a compact way similar to the LandXML format. Due to the high number of classes the Survey Package was split into different parts, Equipment, Observations and SurveyResults.</skos:definition>
    <skos:narrower rdf:resource="http://www.opengis.net/spec/landinfra/1.0/conf/survey/classes"/>
    <skos:narrower rdf:resource="http://www.opengis.net/spec/landinfra/1.0/conf/observations"/>
    <skos:narrower rdf:resource="http://www.opengis.net/spec/landinfra/1.0/req/survey"/>
    <skos:narrower rdf:resource="http://www.opengis.net/spec/landinfra/1.0/conf/survey-results"/>
    <spec:requirementsTested rdf:resource="http://www.opengis.net/spec/landinfra/1.0/req/survey"/>
    <spec:dependency rdf:resource="http://www.opengis.net/spec/landinfra/1.0/conf/land-infra"/>
    <skos:prefLabel>Conformance Class: Survey</skos:prefLabel>
    <spec:conformanceTest rdf:resource="http://www.opengis.net/spec/landinfra/1.0/conf/survey/classes"/>
    <skos:broader rdf:resource="http://www.opengis.net/spec/landinfra/1.0/conf/land-infra"/>
  </rdf:Description>
  <rdf:Description rdf:about="http://www.opengis.net/spec/landinfra/1.0/conf/equipment">
    <skos:narrower rdf:resource="http://www.opengis.net/spec/landinfra/1.0/conf/equipment/observation-correction"/>
    <skos:narrower rdf:resource="http://www.opengis.net/spec/landinfra/1.0/req/equipment"/>
    <skos:narrower rdf:resource="http://www.opengis.net/spec/landinfra/1.0/conf/equipment/classes"/>
    <spec:conformanceTest rdf:resource="http://www.opengis.net/spec/landinfra/1.0/conf/equipment/observation-correction"/>
    <spec:conformanceTest rdf:resource="http://www.opengis.net/spec/landinfra/1.0/conf/equipment/classes"/>
    <skos:prefLabel>Conformance Class: Equipment</skos:prefLabel>
    <skos:definition>In the Equipment Requirements class all information about the processes and the sensors is available that had been used for the determination of an observation.</skos:definition>
    <rdf:type rdf:resource="http://www.w3.org/2004/02/skos/core#Concept"/>
    <rdf:type rdf:resource="http://www.opengis.net/def/ont/modspec/ConformanceClass"/>
    <skos:inScheme rdf:resource="http://www.opengis.net/spec/landinfra/1.0"/>
    <spec:requirementsTested rdf:resource="http://www.opengis.net/spec/landinfra/1.0/req/equipment"/>
    <skos:dependency rdf:resource="http://www.opengis.net/spec/landinfra/1.0/conf/survey"/>
  </rdf:Description>
  <rdf:Description rdf:about="http://www.opengis.net/spec/landinfra/1.0/req/land-feature">
    <skos:inScheme rdf:resource="http://www.opengis.net/spec/landinfra/1.0"/>
    <rdf:type rdf:resource="http://www.opengis.net/def/ont/modspec/RequirementClass"/>
    <rdf:type rdf:resource="http://www.w3.org/2004/02/skos/core#Concept"/>
    <skos:narrower rdf:resource="http://www.opengis.net/spec/landinfra/1.0/req/land-feature/classes"/>
    <skos:narrower rdf:resource="http://www.opengis.net/spec/landinfra/1.0/req/land-feature/alignment"/>
    <skos:broader rdf:resource="http://www.opengis.net/spec/landinfra/1.0/req/land-infra"/>
    <skos:broader rdf:resource="http://www.opengis.net/spec/landinfra/1.0/conf/land-feature"/>
    <skos:prefLabel>Requirement Class: LandFeature</skos:prefLabel>
    <spec:normativeStatement rdf:resource="http://www.opengis.net/spec/landinfra/1.0/req/land-feature/classes"/>
    <spec:normativeStatement rdf:resource="http://www.opengis.net/spec/landinfra/1.0/req/land-feature/alignment"/>
    <skos:definition>Features of the land, such as naturally occurring water features and vegetation are specified in the LandFeature Requirements Class as land features.  Also included are models of the land surface and subsurface layers.  Improvements to the land such as the construction of an embankment or the planting of landscape material are considered to be part of Site Facilities in the Facility Requirements Class.</skos:definition>
    <spec:dependency rdf:resource="http://www.opengis.net/spec/landinfra/1.0/req/land-infra"/>
  </rdf:Description>
  <rdf:Description rdf:about="http://www.opengis.net/spec/landinfra/1.0/req/land-division">
    <skos:narrower rdf:resource="http://www.opengis.net/spec/landinfra/1.0/req/condominium"/>
    <skos:narrower rdf:resource="http://www.opengis.net/spec/landinfra/1.0/req/land-division/classes"/>
    <skos:definition>Land can be divided up into land divisions.  These can either be public (political, judicial, or executive) or private in nature.  The former are administrative divisions and the latter are interests in land.  Both of these are specified in the LandDivision Requirements Class, though condominium interests in land are specified in a separate, Condominium Requirements Class.</skos:definition>
    <spec:dependency rdf:resource="http://www.opengis.net/spec/landinfra/1.0/req/land-infra"/>
    <skos:broader rdf:resource="http://www.opengis.net/spec/landinfra/1.0/conf/land-division"/>
    <skos:broader rdf:resource="http://www.opengis.net/spec/landinfra/1.0/req/land-infra"/>
    <skos:prefLabel>Requirement Class: LandVision</skos:prefLabel>
    <spec:normativeStatement rdf:resource="http://www.opengis.net/spec/landinfra/1.0/req/land-division/classes"/>
    <rdf:type rdf:resource="http://www.opengis.net/def/ont/modspec/RequirementClass"/>
    <rdf:type rdf:resource="http://www.w3.org/2004/02/skos/core#Concept"/>
    <skos:inScheme rdf:resource="http://www.opengis.net/spec/landinfra/1.0"/>
  </rdf:Description>
  <rdf:Description rdf:about="http://www.opengis.net/spec/landinfra/1.0/conf/railway/alignment">
    <skos:prefLabel>Conformance Test: http://www.opengis.net/spec/landinfra/1.0/conf/railway/alignment</skos:prefLabel>
    <skos:inScheme rdf:resource="http://www.opengis.net/spec/landinfra/1.0"/>
    <spec:requirement rdf:resource="http://www.opengis.net/spec/landinfra/1.0/req/railway/alignment"/>
    <skos:broader rdf:resource="http://www.opengis.net/spec/landinfra/1.0/conf/railway"/>
    <spec:purpose>Verify that if the encoding allows the linear element used for locating RailwayElements or CantEvents to be an Alignment, then that encoding supports the Alignment Requirements Class.</spec:purpose>
    <rdf:type rdf:resource="http://www.w3.org/2004/02/skos/core#Concept"/>
    <rdf:type rdf:resource="http://www.opengis.net/def/ont/modspec/ConformanceTest"/>
    <spec:method>Inspect the encoding to verify the above requirement.</spec:method>
    <skos:narrower rdf:resource="http://www.opengis.net/spec/landinfra/1.0/req/railway/alignment"/>
    <skos:definition>Verify that if the encoding allows the linear element used for locating RailwayElements or CantEvents to be an Alignment, then that encoding supports the Alignment Requirements Class.</skos:definition>
    <spec:testType rdf:resource="http://www.opengis.net/def/ont/modspec/Capabilities"/>
  </rdf:Description>
  <rdf:Description rdf:about="http://www.opengis.net/spec/landinfra/1.0/req/condominium">
    <skos:broader rdf:resource="http://www.opengis.net/spec/landinfra/1.0/req/land-division"/>
    <skos:broader rdf:resource="http://www.opengis.net/spec/landinfra/1.0/conf/condominium"/>
    <rdf:type rdf:resource="http://www.opengis.net/def/ont/modspec/RequirementClass"/>
    <rdf:type rdf:resource="http://www.w3.org/2004/02/skos/core#Concept"/>
    <skos:prefLabel>Requirement Class: Condominium</skos:prefLabel>
    <skos:definition>A condominium denotes concurrent ownership of real property that has been divided into private and common portions.  The Condominium Requirements Class includes information about condominium units, buildings and schemes.</skos:definition>
    <skos:narrower rdf:resource="http://www.opengis.net/spec/landinfra/1.0/req/condominium/classes"/>
    <spec:normativeStatement rdf:resource="http://www.opengis.net/spec/landinfra/1.0/req/condominium/classes"/>
    <skos:inScheme rdf:resource="http://www.opengis.net/spec/landinfra/1.0"/>
    <spec:dependency rdf:resource="http://www.opengis.net/spec/landinfra/1.0/req/land-division"/>
  </rdf:Description>
  <rdf:Description rdf:about="http://www.opengis.net/spec/landinfra/1.0/conf/observations/classes">
    <skos:inScheme rdf:resource="http://www.opengis.net/spec/landinfra/1.0"/>
    <spec:method>Inspect the encoding to verify the above requirement.</spec:method>
    <spec:testType rdf:resource="http://www.opengis.net/def/ont/modspec/Capabilities"/>
    <skos:broader rdf:resource="http://www.opengis.net/spec/landinfra/1.0/conf/observations"/>
    <skos:narrower rdf:resource="http://www.opengis.net/spec/landinfra/1.0/req/observations/classes"/>
    <skos:prefLabel>Conformance Test: http://www.opengis.net/spec/landinfra/1.0/conf/observations/classes</skos:prefLabel>
    <skos:definition>Verify that the encoding provides the Observation Requirements Class Classes shown in blue in Figure 43 in a manner consistent with the encoding.  An encoding shall decide which SurveyObservation types it will support and define appropriate requirements classes accordingly. This then would include any dependent types (example SatelliteSystemType has only to be supported if the encoding will support GNSS Observations).</skos:definition>
    <spec:purpose>Verify that the encoding provides the Observation Requirements Class Classes shown in blue in Figure 43 in a manner consistent with the encoding.  An encoding shall decide which SurveyObservation types it will support and define appropriate requirements classes accordingly. This then would include any dependent types (example SatelliteSystemType has only to be supported if the encoding will support GNSS Observations).</spec:purpose>
    <rdf:type rdf:resource="http://www.w3.org/2004/02/skos/core#Concept"/>
    <rdf:type rdf:resource="http://www.opengis.net/def/ont/modspec/ConformanceTest"/>
    <spec:requirement rdf:resource="http://www.opengis.net/spec/landinfra/1.0/req/observations/classes"/>
  </rdf:Description>
  <rdf:Description rdf:about="http://www.opengis.net/spec/landinfra/1.0/req/survey-results/topic-20">
    <skos:inScheme rdf:resource="http://www.opengis.net/spec/landinfra/1.0"/>
    <skos:broader rdf:resource="http://www.opengis.net/spec/landinfra/1.0/req/survey-results"/>
    <skos:broader rdf:resource="http://www.opengis.net/spec/landinfra/1.0/req/survey"/>
    <skos:broader rdf:resource="http://www.opengis.net/spec/landinfra/1.0/conf/survey-results/topic-20"/>
    <rdf:type rdf:resource="http://www.opengis.net/def/ont/modspec/Requirement"/>
    <rdf:type rdf:resource="http://www.w3.org/2004/02/skos/core#Concept"/>
    <skos:definition>If a Land and Infrastructure encoding supports survey results subjects, then the encoding shall support the SF_SamplingFeature and related Classes specified in the OGC Abstract Specification Topic 20, Observation and Measurements shown in Figure 54 that are appropriate to the supported subject area(s).</skos:definition>
    <skos:prefLabel>Requirement: /req/survey-results/topic-20</skos:prefLabel>
  </rdf:Description>
  <rdf:Description rdf:about="http://www.opengis.net/spec/landinfra/1.0/req/survey-results/classes">
    <rdf:type rdf:resource="http://www.opengis.net/def/ont/modspec/Requirement"/>
    <rdf:type rdf:resource="http://www.w3.org/2004/02/skos/core#Concept"/>
    <skos:definition>The SurveyResults Requirements Class Classes shown in blue in Figure 52 shall be provided for by the encoding in a manner consistent with the encoding. An encoding shall decide which SurveyResult types it will support and define appropriate requirements classes accordingly.</skos:definition>
    <skos:broader rdf:resource="http://www.opengis.net/spec/landinfra/1.0/conf/survey-results/classes"/>
    <skos:broader rdf:resource="http://www.opengis.net/spec/landinfra/1.0/req/survey"/>
    <skos:broader rdf:resource="http://www.opengis.net/spec/landinfra/1.0/req/survey-results"/>
    <skos:prefLabel>Requirement: /req/survey-results/classes</skos:prefLabel>
    <skos:inScheme rdf:resource="http://www.opengis.net/spec/landinfra/1.0"/>
  </rdf:Description>
  <rdf:Description rdf:about="http://www.opengis.net/spec/landinfra/1.0/conf/land-feature/classes">
    <rdf:type rdf:resource="http://www.w3.org/2004/02/skos/core#Concept"/>
    <rdf:type rdf:resource="http://www.opengis.net/def/ont/modspec/ConformanceTest"/>
    <skos:narrower rdf:resource="http://www.opengis.net/spec/landinfra/1.0/req/land-feature/classes"/>
    <skos:inScheme rdf:resource="http://www.opengis.net/spec/landinfra/1.0"/>
    <spec:purpose>Verify that the encoding provides the LandFeature Requirements Class Classes shown in blue in Figure 55 in a manner consistent with the encoding.</spec:purpose>
    <spec:method>Inspect the encoding to verify the above requirement.</spec:method>
    <spec:testType rdf:resource="http://www.opengis.net/def/ont/modspec/Capabilities"/>
    <skos:prefLabel>ConformanceTest: http://www.opengis.net/spec/landinfra/1.0/conf/land-feature/classes</skos:prefLabel>
    <skos:definition>Verify that the encoding provides the LandFeature Requirements Class Classes shown in blue in Figure 55 in a manner consistent with the encoding.</skos:definition>
    <spec:requirement rdf:resource="http://www.opengis.net/spec/landinfra/1.0/req/land-feature/classes"/>
    <skos:broader rdf:resource="http://www.opengis.net/spec/landinfra/1.0/conf/land-feature"/>
  </rdf:Description>
  <rdf:Description rdf:about="http://www.opengis.net/spec/landinfra/1.0/req/alignment/CRS">
    <rdf:type rdf:resource="http://www.opengis.net/def/ont/modspec/Requirement"/>
    <rdf:type rdf:resource="http://www.w3.org/2004/02/skos/core#Concept"/>
    <dct:description>All geometry/locations for Alignment2DHorSegments and Alignment2DVertSegments shall be specified using the Alignment2DHorizontal.crs which shall be a Cartesian local engineering reference system.</dct:description>
    <skos:broader rdf:resource="http://www.opengis.net/spec/landinfra/1.0/conf/alignment/CRS"/>
    <skos:broader rdf:resource="http://www.opengis.net/spec/landinfra/1.0/req/alignment"/>
    <skos:prefLabel>Requirement: /req/alignment/CRS</skos:prefLabel>
    <skos:inScheme rdf:resource="http://www.opengis.net/spec/landinfra/1.0"/>
    <skos:definition>All geometry/locations for Alignment2DHorSegments and Alignment2DVertSegments shall be specified using the Alignment2DHorizontal.crs which shall be a Cartesian local engineering reference system.</skos:definition>
  </rdf:Description>
  <rdf:Description rdf:about="http://www.opengis.net/spec/landinfra/1.0/conf/project/classes">
    <rdf:type rdf:resource="http://www.opengis.net/def/ont/modspec/ConformanceTest"/>
    <rdf:type rdf:resource="http://www.w3.org/2004/02/skos/core#Concept"/>
    <skos:broader rdf:resource="http://www.opengis.net/spec/landinfra/1.0/conf/project"/>
    <skos:inScheme rdf:resource="http://www.opengis.net/spec/landinfra/1.0"/>
    <spec:method>Inspect the encoding to verify the above requirement.</spec:method>
    <spec:purpose>Verify that the encoding provides the Project Requirements Class Classes shown in blue in Figure 13 in a manner consistent with the encoding.</spec:purpose>
    <skos:prefLabel>Conformance Test: http://www.opengis.net/spec/landinfra/1.0/conf/project/classes</skos:prefLabel>
    <skos:narrower rdf:resource="http://www.opengis.net/spec/landinfra/1.0/req/project/classes"/>
    <skos:definition>Verify that the encoding provides the Project Requirements Class Classes shown in blue in Figure 13 in a manner consistent with the encoding.</skos:definition>
    <spec:requirement rdf:resource="http://www.opengis.net/spec/landinfra/1.0/req/project/classes"/>
    <spec:testType rdf:resource="http://www.opengis.net/def/ont/modspec/Capabilities"/>
  </rdf:Description>
  <rdf:Description rdf:about="http://www.opengis.net/spec/landinfra/1.0/req/facility/subtypes">
    <skos:definition>A Land and Infrastructure encoding shall specify which of the FacilityPart subtypes shown in Figure 10 it supports.</skos:definition>
    <skos:broader rdf:resource="http://www.opengis.net/spec/landinfra/1.0/req/facility"/>
    <skos:broader rdf:resource="http://www.opengis.net/spec/landinfra/1.0/conf/facility/subtypes"/>
    <rdf:type rdf:resource="http://www.opengis.net/def/ont/modspec/Requirement"/>
    <rdf:type rdf:resource="http://www.w3.org/2004/02/skos/core#Concept"/>
    <skos:prefLabel>Requirement: /req/facility/subtypes</skos:prefLabel>
    <skos:inScheme rdf:resource="http://www.opengis.net/spec/landinfra/1.0"/>
  </rdf:Description>
  <rdf:Description rdf:about="http://www.opengis.net/spec/landinfra/1.0/conf/survey-results/classes">
    <skos:inScheme rdf:resource="http://www.opengis.net/spec/landinfra/1.0"/>
    <spec:purpose>Verify that the encoding provides the SurveyResults Requirements Class Classes shown in blue in Figure 52 in a manner consistent with the encoding.  An encoding shall decide which SurveyResult types it will support and define appropriate requirements classes accordingly.</spec:purpose>
    <spec:method>Inspect the encoding to verify the above requirement.</spec:method>
    <spec:requirement rdf:resource="http://www.opengis.net/spec/landinfra/1.0/req/survey-results/classes"/>
    <spec:testType rdf:resource="http://www.opengis.net/def/ont/modspec/Capabilities"/>
    <skos:definition>Verify that the encoding provides the SurveyResults Requirements Class Classes shown in blue in Figure 52 in a manner consistent with the encoding.  An encoding shall decide which SurveyResult types it will support and define appropriate requirements classes accordingly.</skos:definition>
    <skos:narrower rdf:resource="http://www.opengis.net/spec/landinfra/1.0/req/survey-results/classes"/>
    <skos:broader rdf:resource="http://www.opengis.net/spec/landinfra/1.0/conf/survey-results"/>
    <skos:prefLabel>Conformance Test: http://www.opengis.net/spec/landinfra/1.0/conf/survey-results/classes</skos:prefLabel>
    <rdf:type rdf:resource="http://www.w3.org/2004/02/skos/core#Concept"/>
    <rdf:type rdf:resource="http://www.opengis.net/def/ont/modspec/ConformanceTest"/>
  </rdf:Description>
  <rdf:Description rdf:about="http://www.opengis.net/spec/landinfra/1.0/req/land-infra/crs">
    <rdf:type rdf:resource="http://www.w3.org/2004/02/skos/core#Concept"/>
    <rdf:type rdf:resource="http://www.opengis.net/def/ont/modspec/Requirement"/>
    <skos:broader rdf:resource="http://www.opengis.net/spec/landinfra/1.0/req/land-infra"/>
    <skos:broader rdf:resource="http://www.opengis.net/spec/landinfra/1.0/conf/land-infra/crs"/>
    <skos:prefLabel>Requirement: /req/land-infra/crs</skos:prefLabel>
    <skos:inScheme rdf:resource="http://www.opengis.net/spec/landinfra/1.0"/>
    <skos:definition>An encoding shall support coordinate reference systems in accordance with OGC Abstract Specification Topic 2, Spatial Referencing by Coordinates.</skos:definition>
  </rdf:Description>
  <rdf:Description rdf:about="http://www.opengis.net/spec/landinfra/1.0/req/survey/classes">
    <rdf:type rdf:resource="http://www.w3.org/2004/02/skos/core#Concept"/>
    <rdf:type rdf:resource="http://www.opengis.net/def/ont/modspec/Requirement"/>
    <skos:prefLabel>Requirement: /req/survey/classes</skos:prefLabel>
    <skos:inScheme rdf:resource="http://www.opengis.net/spec/landinfra/1.0"/>
    <skos:definition>The Survey Requirements Class Classes shown in blue in Figure 41 shall be provided for by the encoding in a manner consistent with the encoding.</skos:definition>
    <skos:broader rdf:resource="http://www.opengis.net/spec/landinfra/1.0/conf/survey/classes"/>
    <skos:broader rdf:resource="http://www.opengis.net/spec/landinfra/1.0/req/survey"/>
  </rdf:Description>
  <rdf:Description rdf:about="http://www.opengis.net/spec/landinfra/1.0/conf/railway/classes">
    <spec:method>Inspect the encoding to verify the above requirement.</spec:method>
    <skos:broader rdf:resource="http://www.opengis.net/spec/landinfra/1.0/conf/railway"/>
    <spec:testType rdf:resource="http://www.opengis.net/def/ont/modspec/Capabilities"/>
    <skos:narrower rdf:resource="http://www.opengis.net/spec/landinfra/1.0/req/railway/classes"/>
    <rdf:type rdf:resource="http://www.opengis.net/def/ont/modspec/ConformanceTest"/>
    <rdf:type rdf:resource="http://www.w3.org/2004/02/skos/core#Concept"/>
    <spec:requirement rdf:resource="http://www.opengis.net/spec/landinfra/1.0/req/railway/classes"/>
    <spec:purpose>Verify that the encoding provides the Railway Requirements Class Classes shown in blue in Figure 36 in a manner consistent with the encoding.</spec:purpose>
    <skos:prefLabel>Conformance Test: http://www.opengis.net/spec/landinfra/1.0/conf/railway/classes</skos:prefLabel>
    <skos:definition>Verify that the encoding provides the Railway Requirements Class Classes shown in blue in Figure 36 in a manner consistent with the encoding.</skos:definition>
    <skos:inScheme rdf:resource="http://www.opengis.net/spec/landinfra/1.0"/>
  </rdf:Description>
  <rdf:Description rdf:about="http://www.opengis.net/spec/landinfra/1.0/conf/land-infra/featureID">
    <spec:requirement rdf:resource="http://www.opengis.net/spec/landinfra/1.0/req/land-infra/featureID"/>
    <skos:definition>Verify that the encoding specifies whether it supports ID at the feature level, ID at the Feature sub-type level, or both.</skos:definition>
    <rdf:type rdf:resource="http://www.w3.org/2004/02/skos/core#Concept"/>
    <rdf:type rdf:resource="http://www.opengis.net/def/ont/modspec/ConformanceTest"/>
    <skos:narrower rdf:resource="http://www.opengis.net/spec/landinfra/1.0/req/land-infra/featureID"/>
    <skos:broader rdf:resource="http://www.opengis.net/spec/landinfra/1.0/conf/land-infra"/>
    <spec:purpose>Verify that the encoding specifies whether it supports ID at the feature level, ID at the Feature sub-type level, or both.</spec:purpose>
    <skos:inScheme rdf:resource="http://www.opengis.net/spec/landinfra/1.0"/>
    <spec:method>Inspect the encoding to verify the above requirement.</spec:method>
    <spec:testType rdf:resource="http://www.opengis.net/def/ont/modspec/Capabilities"/>
    <skos:prefLabel>Conformance Test: http://www.opengis.net/spec/landinfra/1.0/conf/land-infra/featureID</skos:prefLabel>
  </rdf:Description>
  <rdf:Description rdf:about="http://www.opengis.net/spec/landinfra/1.0/conf/land-infra/crs">
    <skos:definition>Verify that the encoding requirement for coordinate reference systems is consistent with OGC Abstract Specification Topic 2.</skos:definition>
    <spec:testType rdf:resource="http://www.opengis.net/def/ont/modspec/Capabilities"/>
    <spec:purpose>Verify that the encoding requirement for coordinate reference systems is consistent with OGC Abstract Specification Topic 2.</spec:purpose>
    <rdf:type rdf:resource="http://www.opengis.net/def/ont/modspec/ConformanceTest"/>
    <rdf:type rdf:resource="http://www.w3.org/2004/02/skos/core#Concept"/>
    <skos:broader rdf:resource="http://www.opengis.net/spec/landinfra/1.0/conf/land-infra"/>
    <spec:requirement rdf:resource="http://www.opengis.net/spec/landinfra/1.0/req/land-infra/crs"/>
    <skos:narrower rdf:resource="http://www.opengis.net/spec/landinfra/1.0/req/land-infra/crs"/>
    <skos:inScheme rdf:resource="http://www.opengis.net/spec/landinfra/1.0"/>
    <skos:prefLabel>Conformance Test: http://www.opengis.net/spec/landinfra/1.0/conf/land-infra/crs</skos:prefLabel>
    <spec:method>Inspect the encoding to verify the above requirement.</spec:method>
  </rdf:Description>
  <rdf:Description rdf:about="http://www.opengis.net/spec/landinfra/1.0/conf/land-infra/topic-19-core">
    <skos:broader rdf:resource="http://www.opengis.net/spec/landinfra/1.0/conf/land-infra"/>
    <skos:definition>Verify that, if the encoding supports linearly referenced locations, then the encoding provides the PositionExpression and related Classes specified in the OGC Abstract Specification Topic 19, core Linear Referencing (LR) Package shown in pink in Figure 7 that are appropriate to the supported subject area(s).</skos:definition>
    <spec:method>Inspect the encoding to verify the above requirement.</spec:method>
    <rdf:type rdf:resource="http://www.w3.org/2004/02/skos/core#Concept"/>
    <rdf:type rdf:resource="http://www.opengis.net/def/ont/modspec/ConformanceTest"/>
    <skos:narrower rdf:resource="http://www.opengis.net/spec/landinfra/1.0/req/land-infra/topic-19-core"/>
    <skos:prefLabel>Conformance Test: http://www.opengis.net/spec/landinfra/1.0/conf/land-infra/topic-19-core</skos:prefLabel>
    <spec:purpose>Verify that, if the encoding supports linearly referenced locations, then the encoding provides the PositionExpression and related Classes specified in the OGC Abstract Specification Topic 19, core Linear Referencing (LR) Package shown in pink in Figure 7 that are appropriate to the supported subject area(s).</spec:purpose>
    <skos:inScheme rdf:resource="http://www.opengis.net/spec/landinfra/1.0"/>
    <spec:testType rdf:resource="http://www.opengis.net/def/ont/modspec/Capabilities"/>
    <spec:requirement rdf:resource="http://www.opengis.net/spec/landinfra/1.0/req/land-infra/topic-19-core"/>
  </rdf:Description>
  <rdf:Description rdf:about="http://www.opengis.net/spec/landinfra/1.0/req/condominium/classes">
    <skos:prefLabel>Requirement: /req/condominium/classes</skos:prefLabel>
    <skos:broader rdf:resource="http://www.opengis.net/spec/landinfra/1.0/conf/condominium/classes"/>
    <skos:broader rdf:resource="http://www.opengis.net/spec/landinfra/1.0/req/condominium"/>
    <skos:definition>The Condominium Requirements Class Classes shown in blue in Figure 68 shall be provided for by the encoding in a manner consistent with the encoding.</skos:definition>
    <rdf:type rdf:resource="http://www.opengis.net/def/ont/modspec/Requirement"/>
    <rdf:type rdf:resource="http://www.w3.org/2004/02/skos/core#Concept"/>
    <skos:inScheme rdf:resource="http://www.opengis.net/spec/landinfra/1.0"/>
  </rdf:Description>
  <rdf:Description rdf:about="http://www.opengis.net/spec/landinfra/1.0/conf/land-division/classes">
    <rdf:type rdf:resource="http://www.w3.org/2004/02/skos/core#Concept"/>
    <rdf:type rdf:resource="http://www.opengis.net/def/ont/modspec/ConformanceTest"/>
    <skos:definition>Verify that the encoding provides the LandDivision Requirements Class Classes shown in blue in Figure 60 in a manner consistent with the encoding.</skos:definition>
    <spec:requirement rdf:resource="http://www.opengis.net/spec/landinfra/1.0/req/land-division/classes"/>
    <spec:purpose>Verify that the encoding provides the LandDivision Requirements Class Classes shown in blue in Figure 60 in a manner consistent with the encoding.</spec:purpose>
    <skos:inScheme rdf:resource="http://www.opengis.net/spec/landinfra/1.0"/>
    <skos:narrower rdf:resource="http://www.opengis.net/spec/landinfra/1.0/req/land-division/classes"/>
    <spec:method>Inspect the encoding to verify the above requirement.</spec:method>
    <skos:broader rdf:resource="http://www.opengis.net/spec/landinfra/1.0/conf/land-division"/>
    <spec:testType rdf:resource="http://www.opengis.net/def/ont/modspec/Capabilities"/>
    <skos:prefLabel>ConformanceTest: http://www.opengis.net/spec/landinfra/1.0/conf/land-division/classes</skos:prefLabel>
  </rdf:Description>
  <rdf:Description rdf:about="http://www.opengis.net/spec/landinfra/1.0/req/road/alignment">
    <skos:inScheme rdf:resource="http://www.opengis.net/spec/landinfra/1.0"/>
    <rdf:type rdf:resource="http://www.opengis.net/def/ont/modspec/Requirement"/>
    <rdf:type rdf:resource="http://www.w3.org/2004/02/skos/core#Concept"/>
    <skos:definition>If an encoding allows the linear element used for locating RoadElements to be an Alignment, then that encoding shall support the Alignment Requirements Class.</skos:definition>
    <skos:broader rdf:resource="http://www.opengis.net/spec/landinfra/1.0/req/road"/>
    <skos:broader rdf:resource="http://www.opengis.net/spec/landinfra/1.0/conf/road/alignment"/>
    <skos:prefLabel>Requirement: /req/road/alignment</skos:prefLabel>
  </rdf:Description>
  <rdf:Description rdf:about="http://www.opengis.net/spec/landinfra/1.0/conf/alignment/measures">
    <skos:prefLabel>Conformance Test: http://www.opengis.net/spec/landinfra/1.0/conf/alignment/measures</skos:prefLabel>
    <spec:requirement rdf:resource="http://www.opengis.net/spec/landinfra/1.0/req/alignment/measures"/>
    <rdf:type rdf:resource="http://www.w3.org/2004/02/skos/core#Concept"/>
    <rdf:type rdf:resource="http://www.opengis.net/def/ont/modspec/ConformanceTest"/>
    <spec:purpose>If an encoding uses Alignment as a linear element, verify that it specifies that:
1) If an Alignment2DHorizontal.2DLinestringRepresentation or an Alignment3D.3DLinestringRepresentation is specified as a linear element, then distanceAlong shall be measured along the LineString and offsetLateralDistance and offsetVerticalDistance values shall be measured normal to the LineString from this DistanceAlong point.
2) If an Alignment2DHorizontal.segment list of Alignment2DHorSegments is used as a linear element, then distanceAlong and offsetLateralDistance values shall be measured in the horizontal plane, ignoring any vertical displacement of the Alignment.  OffsetVerticalDistance values shall be absolute from the horizontal plane unless an Alignment2DVertical is specified as a VerticalOffsetReferent so as to take into consideration vertical displacement of the Alignment, if present.</spec:purpose>
    <skos:narrower rdf:resource="http://www.opengis.net/spec/landinfra/1.0/req/alignment/measures"/>
    <skos:broader rdf:resource="http://www.opengis.net/spec/landinfra/1.0/conf/alignment"/>
    <skos:inScheme rdf:resource="http://www.opengis.net/spec/landinfra/1.0"/>
    <spec:method>Inspect the encoding to verify the above requirement.</spec:method>
    <skos:definition>If an encoding uses Alignment as a linear element, verify that it specifies that:
1) If an Alignment2DHorizontal.2DLinestringRepresentation or an Alignment3D.3DLinestringRepresentation is specified as a linear element, then distanceAlong shall be measured along the LineString and offsetLateralDistance and offsetVerticalDistance values shall be measured normal to the LineString from this DistanceAlong point.
2) If an Alignment2DHorizontal.segment list of Alignment2DHorSegments is used as a linear element, then distanceAlong and offsetLateralDistance values shall be measured in the horizontal plane, ignoring any vertical displacement of the Alignment.  OffsetVerticalDistance values shall be absolute from the horizontal plane unless an Alignment2DVertical is specified as a VerticalOffsetReferent so as to take into consideration vertical displacement of the Alignment, if present.</skos:definition>
    <spec:testType rdf:resource="http://www.opengis.net/def/ont/modspec/Capabilities"/>
  </rdf:Description>
  <rdf:Description rdf:about="http://www.opengis.net/spec/landinfra/1.0/req/alignment/classes">
    <skos:prefLabel>Requirement: /req/alignment/classes</skos:prefLabel>
    <rdf:type rdf:resource="http://www.opengis.net/def/ont/modspec/Requirement"/>
    <rdf:type rdf:resource="http://www.w3.org/2004/02/skos/core#Concept"/>
    <skos:broader rdf:resource="http://www.opengis.net/spec/landinfra/1.0/req/alignment"/>
    <skos:broader rdf:resource="http://www.opengis.net/spec/landinfra/1.0/conf/alignment/classes"/>
    <skos:definition>An encoding shall implement the OGC Abstract Specification Topic 19 ILinearElement and ISpatial interfaces in a manner consistent with the encoding.</skos:definition>
    <skos:inScheme rdf:resource="http://www.opengis.net/spec/landinfra/1.0"/>
  </rdf:Description>
  <rdf:Description rdf:about="http://www.opengis.net/spec/landinfra/1.0/req/land-infra/topic-1">
    <skos:prefLabel>Requirement: /req/land-infra/topic-1</skos:prefLabel>
    <skos:broader rdf:resource="http://www.opengis.net/spec/landinfra/1.0/conf/land-infra/topic-1"/>
    <skos:broader rdf:resource="http://www.opengis.net/spec/landinfra/1.0/req/land-infra"/>
    <skos:inScheme rdf:resource="http://www.opengis.net/spec/landinfra/1.0"/>
    <rdf:type rdf:resource="http://www.opengis.net/def/ont/modspec/Requirement"/>
    <rdf:type rdf:resource="http://www.w3.org/2004/02/skos/core#Concept"/>
    <skos:definition>A Land and Infrastructure encoding shall support the geometry types specified in the OGC Abstract Specification Topic 1, Feature Geometry as shown in pink and the SimpleTriangle, TIN, and PolyfaceMesh extensions shown in beige in Figure 6, that are appropriate to the supported subject area(s). Additional geometry types, not found in Topic 1, but required by a specific requirements class, are specified in that requirements class. If a Land and Infrastructure encoding supports linearly referenced locations, then the encoding shall support the PositionExpression and related Classes specified in the OGC Abstract Specification Topic 19, core Linear Referencing (LR) Package shown in pink in Figure 7 that are appropriate to the supported subject area(s). If a Land and Infrastructure encoding supports linearly referenced locations, then the encoding shall specify which of the OGC Abstract Specification Topic 19, Linear Referencing extension packages it supports and shall therefore support the appropriate Classes shown in Figure 7 and Figure 8 for those packages that are appropriate to the supported subject area(s).</skos:definition>
  </rdf:Description>
  <rdf:Description rdf:about="http://www.opengis.net/spec/landinfra/1.0/req/road-cross-section">
    <skos:broader rdf:resource="http://www.opengis.net/spec/landinfra/1.0/req/road"/>
    <skos:broader rdf:resource="http://www.opengis.net/spec/landinfra/1.0/conf/road-cross-section"/>
    <spec:normativeStatement rdf:resource="http://www.opengis.net/spec/landinfra/1.0/req/road-cross-section/classes"/>
    <spec:normativeStatement rdf:resource="http://www.opengis.net/spec/landinfra/1.0/req/road-cross-section/alignment"/>
    <rdf:type rdf:resource="http://www.opengis.net/def/ont/modspec/RequirementClass"/>
    <rdf:type rdf:resource="http://www.w3.org/2004/02/skos/core#Concept"/>
    <skos:inScheme rdf:resource="http://www.opengis.net/spec/landinfra/1.0"/>
    <skos:prefLabel>Requirement Class: RoadCrossSection</skos:prefLabel>
    <spec:dependency rdf:resource="http://www.opengis.net/spec/landinfra/1.0/req/road"/>
    <skos:definition>The RoadCrossSection Requirements Class extends the Road Requirements Class by adding the 2D CrossSection alternative way of representing a design, as well as collections of these.</skos:definition>
    <skos:narrower rdf:resource="http://www.opengis.net/spec/landinfra/1.0/req/road-cross-section/alignment"/>
    <skos:narrower rdf:resource="http://www.opengis.net/spec/landinfra/1.0/req/road-cross-section/classes"/>
  </rdf:Description>
  <rdf:Description rdf:about="http://www.opengis.net/spec/landinfra/1.0/conf/facility">
    <spec:requirementsTested rdf:resource="http://www.opengis.net/spec/landinfra/1.0/req/facility"/>
    <skos:narrower rdf:resource="http://www.opengis.net/spec/landinfra/1.0/conf/railway"/>
    <skos:narrower rdf:resource="http://www.opengis.net/spec/landinfra/1.0/conf/facility/classes"/>
    <skos:narrower rdf:resource="http://www.opengis.net/spec/landinfra/1.0/conf/project"/>
    <skos:narrower rdf:resource="http://www.opengis.net/spec/landinfra/1.0/conf/road"/>
    <skos:narrower rdf:resource="http://www.opengis.net/spec/landinfra/1.0/req/facility"/>
    <skos:narrower rdf:resource="http://www.opengis.net/spec/landinfra/1.0/conf/alignment"/>
    <skos:narrower rdf:resource="http://www.opengis.net/spec/landinfra/1.0/conf/facility/subtypes"/>
    <skos:broader rdf:resource="http://www.opengis.net/spec/landinfra/1.0/conf/land-infra"/>
    <skos:prefLabel>Conformance Class: Facility</skos:prefLabel>
    <skos:definition>Facilities include collections of buildings and civil engineering works and their associated siteworks.  The Facilities Requirements Class includes the breakdown of facilities into discipline specific facility parts and introduces the notion of elements which make up these parts.  The Facilities Requirements Class only provides general support for facilities themselves, allowing subsequent Requirements Classes to focus on specific types of the parts that make up facilities, such as road and railway.  This Requirements Class is optional in order to allow for the condition where all of the LandInfra dataset information is not facility related, such as one containing only survey or land division information.</skos:definition>
    <rdf:type rdf:resource="http://www.w3.org/2004/02/skos/core#Concept"/>
    <rdf:type rdf:resource="http://www.opengis.net/def/ont/modspec/ConformanceClass"/>
    <spec:conformanceTest rdf:resource="http://www.opengis.net/spec/landinfra/1.0/conf/facility/subtypes"/>
    <spec:conformanceTest rdf:resource="http://www.opengis.net/spec/landinfra/1.0/conf/facility/classes"/>
    <spec:dependency rdf:resource="http://www.opengis.net/spec/landinfra/1.0/conf/land-infra"/>
    <skos:inScheme rdf:resource="http://www.opengis.net/spec/landinfra/1.0"/>
  </rdf:Description>
  <rdf:Description rdf:about="http://www.opengis.net/spec/landinfra/1.0/conf/land-feature">
    <spec:conformanceTest rdf:resource="http://www.opengis.net/spec/landinfra/1.0/conf/land-feature/alignment"/>
    <spec:conformanceTest rdf:resource="http://www.opengis.net/spec/landinfra/1.0/conf/land-feature/classes"/>
    <rdf:type rdf:resource="http://www.w3.org/2004/02/skos/core#Concept"/>
    <rdf:type rdf:resource="http://www.opengis.net/def/ont/modspec/ConformanceClass"/>
    <skos:prefLabel>Conformance Class: LandFeature</skos:prefLabel>
    <skos:inScheme rdf:resource="http://www.opengis.net/spec/landinfra/1.0"/>
    <spec:requirementsTested rdf:resource="http://www.opengis.net/spec/landinfra/1.0/req/land-feature"/>
    <spec:dependency rdf:resource="http://www.opengis.net/spec/landinfra/1.0/conf/land-infra"/>
    <skos:narrower rdf:resource="http://www.opengis.net/spec/landinfra/1.0/conf/land-feature/alignment"/>
    <skos:narrower rdf:resource="http://www.opengis.net/spec/landinfra/1.0/req/land-feature"/>
    <skos:narrower rdf:resource="http://www.opengis.net/spec/landinfra/1.0/conf/land-feature/classes"/>
    <skos:definition>Features of the land, such as naturally occurring water features and vegetation are specified in the LandFeature Requirements Class as land features.  Also included are models of the land surface and subsurface layers.  Improvements to the land such as the construction of an embankment or the planting of landscape material are considered to be part of Site Facilities in the Facility Requirements Class.</skos:definition>
    <skos:broader rdf:resource="http://www.opengis.net/spec/landinfra/1.0/conf/land-infra"/>
  </rdf:Description>
  <rdf:Description rdf:about="http://www.opengis.net/spec/landinfra/1.0/req/land-division/classes">
    <rdf:type rdf:resource="http://www.w3.org/2004/02/skos/core#Concept"/>
    <rdf:type rdf:resource="http://www.opengis.net/def/ont/modspec/Requirement"/>
    <skos:definition>The LandDivision Requirements Class Classes shown in blue in Figure 60 shall be provided for by the encoding in a manner consistent with the encoding.</skos:definition>
    <skos:prefLabel>Requirement: /req/land-division/classes</skos:prefLabel>
    <skos:inScheme rdf:resource="http://www.opengis.net/spec/landinfra/1.0"/>
    <skos:broader rdf:resource="http://www.opengis.net/spec/landinfra/1.0/req/land-division"/>
    <skos:broader rdf:resource="http://www.opengis.net/spec/landinfra/1.0/conf/land-division/classes"/>
  </rdf:Description>
  <rdf:Description rdf:about="http://www.opengis.net/spec/landinfra/1.0/req/land-infra/topic-19-extensions">
    <skos:broader rdf:resource="http://www.opengis.net/spec/landinfra/1.0/conf/land-infra/topic-19-extensions"/>
    <skos:broader rdf:resource="http://www.opengis.net/spec/landinfra/1.0/req/land-infra"/>
    <skos:definition>If a Land and Infrastructure encoding supports linearly referenced locations, then the encoding shall specify which of the OGC Abstract Specification Topic 19, Linear Referencing extension packages it supports and shall therefore support the appropriate Classes shown in Figure 7 and Figure 8 for those packages that are appropriate to the supported subject area(s).</skos:definition>
    <skos:inScheme rdf:resource="http://www.opengis.net/spec/landinfra/1.0"/>
    <rdf:type rdf:resource="http://www.w3.org/2004/02/skos/core#Concept"/>
    <rdf:type rdf:resource="http://www.opengis.net/def/ont/modspec/Requirement"/>
    <skos:prefLabel>Requirement: /req/land-infra/topic-19-extensions</skos:prefLabel>
  </rdf:Description>
  <rdf:Description rdf:about="http://www.opengis.net/spec/landinfra/1.0/conf/land-infra/topic-1">
    <skos:definition>Verify that the encoding provides the geometry types specified in the OGC Abstract Specification Topic 1, Feature Geometry as shown in pink and the SimpleTriangle, TIN, and PolyfaceMesh extensions shown in beige in Figure 6, that are appropriate to the supported subject area(s).
  Verify that the encoding provides the additional geometry types not found in Topic 1, but required by a specific supported requirements class, are specified in that requirements class.</skos:definition>
    <spec:method>Inspect the encoding to verify the above requirement.</spec:method>
    <spec:testType rdf:resource="http://www.opengis.net/def/ont/modspec/Capabilities"/>
    <spec:purpose>Verify that the encoding provides the geometry types specified in the OGC Abstract Specification Topic 1, Feature Geometry as shown in pink and the SimpleTriangle, TIN, and PolyfaceMesh extensions shown in beige in Figure 6, that are appropriate to the supported subject area(s).
  Verify that the encoding provides the additional geometry types not found in Topic 1, but required by a specific supported requirements class, are specified in that requirements class.</spec:purpose>
    <spec:requirement rdf:resource="http://www.opengis.net/spec/landinfra/1.0/req/land-infra/topic-1"/>
    <skos:prefLabel>Conformance Test: http://www.opengis.net/spec/landinfra/1.0/conf/land-infra/topic-1</skos:prefLabel>
    <skos:inScheme rdf:resource="http://www.opengis.net/spec/landinfra/1.0"/>
    <rdf:type rdf:resource="http://www.w3.org/2004/02/skos/core#Concept"/>
    <rdf:type rdf:resource="http://www.opengis.net/def/ont/modspec/ConformanceTest"/>
    <skos:narrower rdf:resource="http://www.opengis.net/spec/landinfra/1.0/req/land-infra/topic-1"/>
    <skos:broader rdf:resource="http://www.opengis.net/spec/landinfra/1.0/conf/land-infra"/>
  </rdf:Description>
  <rdf:Description rdf:about="http://www.opengis.net/spec/landinfra/1.0/req/railway/classes">
    <skos:definition>The Railway Requirements Class Classes shown in blue in Figure 36 shall be provided for by the encoding in a manner consistent with the encoding.</skos:definition>
    <skos:broader rdf:resource="http://www.opengis.net/spec/landinfra/1.0/req/railway"/>
    <skos:broader rdf:resource="http://www.opengis.net/spec/landinfra/1.0/conf/railway/classes"/>
    <skos:prefLabel>Requirement: /req/railway/classes</skos:prefLabel>
    <skos:inScheme rdf:resource="http://www.opengis.net/spec/landinfra/1.0"/>
    <rdf:type rdf:resource="http://www.opengis.net/def/ont/modspec/Requirement"/>
    <rdf:type rdf:resource="http://www.w3.org/2004/02/skos/core#Concept"/>
  </rdf:Description>
  <rdf:Description rdf:about="http://www.opengis.net/spec/landinfra/1.0/req/equipment/observation-correction">
    <skos:prefLabel>Requirement: /req/equipment/observation-correction</skos:prefLabel>
    <skos:definition>The ObservationCorrection Classes in blue in Figure 51 shall be provided for by the encoding in a manner consistent with the encoding. The encoding shall decide which correction types it will support and define appropriate requirements classes accordingly.</skos:definition>
    <skos:broader rdf:resource="http://www.opengis.net/spec/landinfra/1.0/req/equipment"/>
    <skos:broader rdf:resource="http://www.opengis.net/spec/landinfra/1.0/conf/equipment/observation-correction"/>
    <skos:inScheme rdf:resource="http://www.opengis.net/spec/landinfra/1.0"/>
    <rdf:type rdf:resource="http://www.opengis.net/def/ont/modspec/Requirement"/>
    <rdf:type rdf:resource="http://www.w3.org/2004/02/skos/core#Concept"/>
  </rdf:Description>
  <rdf:Description rdf:about="http://www.opengis.net/spec/landinfra/1.0/req/road/classes">
    <skos:definition>The Road Requirements Class Classes shown in blue in Figure 21 shall be provided for by the encoding in a manner consistent with the encoding.</skos:definition>
    <skos:inScheme rdf:resource="http://www.opengis.net/spec/landinfra/1.0"/>
    <skos:prefLabel>Requirement: /req/road/classes</skos:prefLabel>
    <rdf:type rdf:resource="http://www.opengis.net/def/ont/modspec/Requirement"/>
    <rdf:type rdf:resource="http://www.w3.org/2004/02/skos/core#Concept"/>
    <skos:broader rdf:resource="http://www.opengis.net/spec/landinfra/1.0/conf/road/classes"/>
    <skos:broader rdf:resource="http://www.opengis.net/spec/landinfra/1.0/req/road"/>
  </rdf:Description>
  <rdf:Description rdf:about="http://www.opengis.net/spec/landinfra/1.0/conf/road/classes">
    <skos:narrower rdf:resource="http://www.opengis.net/spec/landinfra/1.0/req/road/classes"/>
    <skos:prefLabel>Conformance Test: http://www.opengis.net/spec/landinfra/1.0/conf/road/classes</skos:prefLabel>
    <skos:definition>Verify that the encoding provides the Road Requirements Class Classes shown in blue in Figure 21 in a manner consistent with the encoding.</skos:definition>
    <skos:broader rdf:resource="http://www.opengis.net/spec/landinfra/1.0/conf/road"/>
    <spec:method>Inspect the encoding to verify the above requirement.</spec:method>
    <rdf:type rdf:resource="http://www.w3.org/2004/02/skos/core#Concept"/>
    <rdf:type rdf:resource="http://www.opengis.net/def/ont/modspec/ConformanceTest"/>
    <spec:requirement rdf:resource="http://www.opengis.net/spec/landinfra/1.0/req/road/classes"/>
    <spec:purpose>Verify that the encoding provides the Road Requirements Class Classes shown in blue in Figure 21 in a manner consistent with the encoding.</spec:purpose>
    <skos:inScheme rdf:resource="http://www.opengis.net/spec/landinfra/1.0"/>
    <spec:testType rdf:resource="http://www.opengis.net/def/ont/modspec/Capabilities"/>
  </rdf:Description>
  <rdf:Description rdf:about="http://www.opengis.net/spec/landinfra/1.0/req/facility">
    <spec:dependency rdf:resource="http://www.opengis.net/spec/landinfra/1.0/req/land-infra"/>
    <skos:narrower rdf:resource="http://www.opengis.net/spec/landinfra/1.0/req/facility/classes"/>
    <skos:narrower rdf:resource="http://www.opengis.net/spec/landinfra/1.0/req/railway"/>
    <skos:narrower rdf:resource="http://www.opengis.net/spec/landinfra/1.0/req/project"/>
    <skos:narrower rdf:resource="http://www.opengis.net/spec/landinfra/1.0/req/facility/subtypes"/>
    <skos:narrower rdf:resource="http://www.opengis.net/spec/landinfra/1.0/req/alignment"/>
    <skos:narrower rdf:resource="http://www.opengis.net/spec/landinfra/1.0/req/road"/>
    <skos:inScheme rdf:resource="http://www.opengis.net/spec/landinfra/1.0"/>
    <rdf:type rdf:resource="http://www.opengis.net/def/ont/modspec/RequirementClass"/>
    <rdf:type rdf:resource="http://www.w3.org/2004/02/skos/core#Concept"/>
    <spec:normativeStatement rdf:resource="http://www.opengis.net/spec/landinfra/1.0/req/facility/classes"/>
    <spec:normativeStatement rdf:resource="http://www.opengis.net/spec/landinfra/1.0/req/facility/subtypes"/>
    <skos:broader rdf:resource="http://www.opengis.net/spec/landinfra/1.0/conf/facility"/>
    <skos:broader rdf:resource="http://www.opengis.net/spec/landinfra/1.0/req/land-infra"/>
    <skos:definition>Facilities include collections of buildings and civil engineering works and their associated siteworks.  The Facilities Requirements Class includes the breakdown of facilities into discipline specific facility parts and introduces the notion of elements which make up these parts.  The Facilities Requirements Class only provides general support for facilities themselves, allowing subsequent Requirements Classes to focus on specific types of the parts that make up facilities, such as road and railway.  This Requirements Class is optional in order to allow for the condition where all of the LandInfra dataset information is not facility related, such as one containing only survey or land division information.</skos:definition>
    <skos:prefLabel>Requirement Class: Facility</skos:prefLabel>
  </rdf:Description>
  <rdf:Description rdf:about="http://www.opengis.net/spec/landinfra/1.0/conf/road-cross-section">
    <spec:requirementsTested rdf:resource="http://www.opengis.net/spec/landinfra/1.0/req/road-cross-section"/>
    <skos:broader rdf:resource="http://www.opengis.net/spec/landinfra/1.0/conf/road"/>
    <skos:narrower rdf:resource="http://www.opengis.net/spec/landinfra/1.0/conf/road-cross-section/classes"/>
    <skos:narrower rdf:resource="http://www.opengis.net/spec/landinfra/1.0/req/road-cross-section"/>
    <skos:narrower rdf:resource="http://www.opengis.net/spec/landinfra/1.0/conf/road-cross-section/alignment"/>
    <skos:definition>The RoadCrossSection Requirements Class extends the Road Requirements Class by adding the 2D CrossSection alternative way of representing a design, as well as collections of these.</skos:definition>
    <spec:conformanceTest rdf:resource="http://www.opengis.net/spec/landinfra/1.0/conf/road-cross-section/classes"/>
    <spec:conformanceTest rdf:resource="http://www.opengis.net/spec/landinfra/1.0/conf/road-cross-section/alignment"/>
    <rdf:type rdf:resource="http://www.w3.org/2004/02/skos/core#Concept"/>
    <rdf:type rdf:resource="http://www.opengis.net/def/ont/modspec/ConformanceClass"/>
    <skos:inScheme rdf:resource="http://www.opengis.net/spec/landinfra/1.0"/>
    <spec:dependency rdf:resource="http://www.opengis.net/spec/landinfra/1.0/conf/road"/>
    <skos:prefLabel>Conformance Class: RoadCrossSection</skos:prefLabel>
  </rdf:Description>
  <rdf:Description rdf:about="http://www.opengis.net/spec/landinfra/1.0/req/equipment">
    <spec:normativeStatement rdf:resource="http://www.opengis.net/spec/landinfra/1.0/req/equipment/observation-correction"/>
    <spec:normativeStatement rdf:resource="http://www.opengis.net/spec/landinfra/1.0/req/equipment/classes"/>
    <spec:dependency rdf:resource="http://www.opengis.net/spec/landinfra/1.0/req/survey"/>
    <skos:narrower rdf:resource="http://www.opengis.net/spec/landinfra/1.0/req/equipment/classes"/>
    <skos:narrower rdf:resource="http://www.opengis.net/spec/landinfra/1.0/req/equipment/observation-correction"/>
    <skos:definition>In the Equipment Requirements class all information about the processes and the sensors is available that had been used for the determination of an observation.</skos:definition>
    <rdf:type rdf:resource="http://www.w3.org/2004/02/skos/core#Concept"/>
    <rdf:type rdf:resource="http://www.opengis.net/def/ont/modspec/RequirementClass"/>
    <skos:broader rdf:resource="http://www.opengis.net/spec/landinfra/1.0/req/survey"/>
    <skos:broader rdf:resource="http://www.opengis.net/spec/landinfra/1.0/conf/equipment"/>
    <skos:prefLabel>Requirement Class: Equipment</skos:prefLabel>
    <skos:inScheme rdf:resource="http://www.opengis.net/spec/landinfra/1.0"/>
  </rdf:Description>
  <rdf:Description rdf:about="http://www.opengis.net/spec/landinfra/1.0/conf/road">
    <skos:inScheme rdf:resource="http://www.opengis.net/spec/landinfra/1.0"/>
    <skos:definition>The Road Requirements Class supports those use cases in which a designer wishes to exchange the output of the design with someone who is likely to use it for purposes other than completing the road design.  Consequently, the Road Requirements Class includes several alternative ways for representing a design such as with 3D RoadElements, 3D StringLines (aka profile views, longitudinal breaklines, long sections), and 3D surfaces and layers, as well as collections of these.</skos:definition>
    <skos:narrower rdf:resource="http://www.opengis.net/spec/landinfra/1.0/conf/road/alignment"/>
    <skos:narrower rdf:resource="http://www.opengis.net/spec/landinfra/1.0/conf/road/classes"/>
    <skos:narrower rdf:resource="http://www.opengis.net/spec/landinfra/1.0/req/road"/>
    <skos:narrower rdf:resource="http://www.opengis.net/spec/landinfra/1.0/conf/road-cross-section"/>
    <skos:broader rdf:resource="http://www.opengis.net/spec/landinfra/1.0/conf/facility"/>
    <spec:conformanceTest rdf:resource="http://www.opengis.net/spec/landinfra/1.0/conf/road/alignment"/>
    <spec:conformanceTest rdf:resource="http://www.opengis.net/spec/landinfra/1.0/conf/road/classes"/>
    <rdf:type rdf:resource="http://www.w3.org/2004/02/skos/core#Concept"/>
    <rdf:type rdf:resource="http://www.opengis.net/def/ont/modspec/ConformanceClass"/>
    <skos:prefLabel>Conformance Class: Road</skos:prefLabel>
    <spec:requirementsTested rdf:resource="http://www.opengis.net/spec/landinfra/1.0/req/road"/>
    <spec:dependency rdf:resource="http://www.opengis.net/spec/landinfra/1.0/conf/facility"/>
  </rdf:Description>
  <rdf:Description rdf:about="http://www.opengis.net/spec/landinfra/1.0/conf/land-infra/topic-19-extensions">
    <rdf:type rdf:resource="http://www.opengis.net/def/ont/modspec/ConformanceTest"/>
    <rdf:type rdf:resource="http://www.w3.org/2004/02/skos/core#Concept"/>
    <skos:narrower rdf:resource="http://www.opengis.net/spec/landinfra/1.0/req/land-infra/topic-19-extensions"/>
    <skos:definition>Verify that, if the encoding supports linearly referenced locations, then the encoding specifies which of the OGC Abstract Specification Topic 19, Linear Referencing extension packages it supports and therefore supports the appropriate Classes shown in Figure 7 and Figure 8 for those packages that are appropriate to the supported subject area(s).</skos:definition>
    <spec:method>Inspect the encoding to verify the above requirement.</spec:method>
    <skos:inScheme rdf:resource="http://www.opengis.net/spec/landinfra/1.0"/>
    <spec:testType rdf:resource="http://www.opengis.net/def/ont/modspec/Capabilities"/>
    <spec:requirement rdf:resource="http://www.opengis.net/spec/landinfra/1.0/req/land-infra/topic-19-extensions"/>
    <skos:broader rdf:resource="http://www.opengis.net/spec/landinfra/1.0/conf/land-infra"/>
    <spec:purpose>Verify that, if the encoding supports linearly referenced locations, then the encoding specifies which of the OGC Abstract Specification Topic 19, Linear Referencing extension packages it supports and therefore supports the appropriate Classes shown in Figure 7 and Figure 8 for those packages that are appropriate to the supported subject area(s).</spec:purpose>
    <skos:prefLabel>Conformance Test: http://www.opengis.net/spec/landinfra/1.0/conf/land-infra/topic-19-extensions</skos:prefLabel>
  </rdf:Description>
  <rdf:Description rdf:about="http://www.opengis.net/spec/landinfra/1.0/conf/land-infra/dataset">
    <rdf:type rdf:resource="http://www.w3.org/2004/02/skos/core#Concept"/>
    <rdf:type rdf:resource="http://www.opengis.net/def/ont/modspec/ConformanceTest"/>
    <skos:broader rdf:resource="http://www.opengis.net/spec/landinfra/1.0/conf/land-infra"/>
    <skos:inScheme rdf:resource="http://www.opengis.net/spec/landinfra/1.0"/>
    <skos:prefLabel>Conformance Test: http://www.opengis.net/spec/landinfra/1.0/conf/land-infra/dataset</skos:prefLabel>
    <spec:method>Inspect the encoding to verify the above requirement.</spec:method>
    <skos:definition>Verify that the encoding specifies a LandInfra dataset in a format appropriate for that encoding.</skos:definition>
    <spec:requirement rdf:resource="http://www.opengis.net/spec/landinfra/1.0/req/land-infra/dataset"/>
    <spec:testType rdf:resource="http://www.opengis.net/def/ont/modspec/Capabilities"/>
    <spec:purpose>Verify that the encoding specifies a LandInfra dataset in a format appropriate for that encoding.</spec:purpose>
    <skos:narrower rdf:resource="http://www.opengis.net/spec/landinfra/1.0/req/land-infra/dataset"/>
  </rdf:Description>
  <rdf:Description rdf:about="http://www.opengis.net/spec/landinfra/1.0/req/land-feature/classes">
    <skos:definition>The LandFeature Requirements Class Classes shown in blue in Figure 55 shall be provided for by the encoding in a manner consistent with the encoding.</skos:definition>
    <skos:inScheme rdf:resource="http://www.opengis.net/spec/landinfra/1.0"/>
    <skos:broader rdf:resource="http://www.opengis.net/spec/landinfra/1.0/conf/land-feature/classes"/>
    <skos:broader rdf:resource="http://www.opengis.net/spec/landinfra/1.0/req/land-feature"/>
    <rdf:type rdf:resource="http://www.opengis.net/def/ont/modspec/Requirement"/>
    <rdf:type rdf:resource="http://www.w3.org/2004/02/skos/core#Concept"/>
    <skos:prefLabel>Requirement: /req/land-feature/classes</skos:prefLabel>
  </rdf:Description>
  <rdf:Description rdf:about="http://www.opengis.net/spec/landinfra/1.0/conf/survey-results/topic-20">
    <skos:definition>Verify that, if the encoding supports survey results subjects, then the encoding shall support the SF_SamplingFeature and related Classes specified in the OGC Abstract Specification Topic 20, Observation and Measurements shown in Figure 54 that are appropriate to the supported subject area(s).</skos:definition>
    <rdf:type rdf:resource="http://www.w3.org/2004/02/skos/core#Concept"/>
    <rdf:type rdf:resource="http://www.opengis.net/def/ont/modspec/ConformanceTest"/>
    <skos:prefLabel>Conformance Test: http://www.opengis.net/spec/landinfra/1.0/conf/survey-results/topic-20</skos:prefLabel>
    <spec:purpose>Verify that, if the encoding supports survey results subjects, then the encoding shall support the SF_SamplingFeature and related Classes specified in the OGC Abstract Specification Topic 20, Observation and Measurements shown in Figure 54 that are appropriate to the supported subject area(s).</spec:purpose>
    <skos:inScheme rdf:resource="http://www.opengis.net/spec/landinfra/1.0"/>
    <spec:requirement rdf:resource="http://www.opengis.net/spec/landinfra/1.0/req/survey-results/topic-20"/>
    <spec:method>Inspect the encoding to verify the above requirement.</spec:method>
    <skos:narrower rdf:resource="http://www.opengis.net/spec/landinfra/1.0/req/survey-results/topic-20"/>
    <spec:testType rdf:resource="http://www.opengis.net/def/ont/modspec/Capabilities"/>
    <skos:broader rdf:resource="http://www.opengis.net/spec/landinfra/1.0/conf/survey-results"/>
  </rdf:Description>
  <rdf:Description rdf:about="http://www.opengis.net/spec/landinfra/1.0/req/railway">
    <spec:normativeStatement rdf:resource="http://www.opengis.net/spec/landinfra/1.0/req/railway/classes"/>
    <spec:normativeStatement rdf:resource="http://www.opengis.net/spec/landinfra/1.0/req/railway/cant"/>
    <spec:normativeStatement rdf:resource="http://www.opengis.net/spec/landinfra/1.0/req/railway/alignment"/>
    <skos:prefLabel>Requirement Class: Railway</skos:prefLabel>
    <rdf:type rdf:resource="http://www.w3.org/2004/02/skos/core#Concept"/>
    <rdf:type rdf:resource="http://www.opengis.net/def/ont/modspec/RequirementClass"/>
    <skos:narrower rdf:resource="http://www.opengis.net/spec/landinfra/1.0/req/railway/cant"/>
    <skos:narrower rdf:resource="http://www.opengis.net/spec/landinfra/1.0/req/railway/alignment"/>
    <skos:narrower rdf:resource="http://www.opengis.net/spec/landinfra/1.0/req/railway/classes"/>
    <skos:broader rdf:resource="http://www.opengis.net/spec/landinfra/1.0/req/facility"/>
    <skos:broader rdf:resource="http://www.opengis.net/spec/landinfra/1.0/conf/railway"/>
    <skos:definition>The Railway Requirements Class supports those use cases where a designer wishes to exchange the output of the railway design with someone who is likely to use if for purposes other than further design. Consequently, the Railway Requirements Class covers design output such as 3D railway elements and track geometry including superelevation (cant).</skos:definition>
    <skos:inScheme rdf:resource="http://www.opengis.net/spec/landinfra/1.0"/>
    <spec:dependency rdf:resource="http://www.opengis.net/spec/landinfra/1.0/req/facility"/>
  </rdf:Description>
  <rdf:Description rdf:about="http://www.opengis.net/spec/docs/15-111r1-anno">
    <rdf:type rdf:resource="http://www.w3.org/2002/07/owl#Ontology"/>
  </rdf:Description>
  <rdf:Description rdf:about="http://www.opengis.net/spec/landinfra/1.0/conf/facility/classes">
    <skos:inScheme rdf:resource="http://www.opengis.net/spec/landinfra/1.0"/>
    <spec:method>Inspect the encoding to verify the above requirement.</spec:method>
    <skos:prefLabel>Conformance Test: http://www.opengis.net/spec/landinfra/1.0/conf/facility/classes</skos:prefLabel>
    <skos:narrower rdf:resource="http://www.opengis.net/spec/landinfra/1.0/req/facility/classes"/>
    <spec:testType rdf:resource="http://www.opengis.net/def/ont/modspec/Capabilities"/>
    <spec:requirement rdf:resource="http://www.opengis.net/spec/landinfra/1.0/req/facility/classes"/>
    <skos:broader rdf:resource="http://www.opengis.net/spec/landinfra/1.0/conf/facility"/>
    <rdf:type rdf:resource="http://www.w3.org/2004/02/skos/core#Concept"/>
    <rdf:type rdf:resource="http://www.opengis.net/def/ont/modspec/ConformanceTest"/>
    <spec:purpose>Verify that the encoding provides the Facility Requirements class Classes shown in blue in Figure 10 in a manner consistent with the encoding.</spec:purpose>
    <skos:definition>Verify that the encoding provides the Facility Requirements class Classes shown in blue in Figure 10 in a manner consistent with the encoding.</skos:definition>
  </rdf:Description>
  <rdf:Description rdf:about="http://www.opengis.net/spec/landinfra/1.0/conf/project">
    <skos:prefLabel>Conformance Class: Project</skos:prefLabel>
    <skos:narrower rdf:resource="http://www.opengis.net/spec/landinfra/1.0/req/project"/>
    <skos:narrower rdf:resource="http://www.opengis.net/spec/landinfra/1.0/conf/project/classes"/>
    <skos:inScheme rdf:resource="http://www.opengis.net/spec/landinfra/1.0"/>
    <spec:dependency rdf:resource="http://www.opengis.net/spec/landinfra/1.0/conf/facility"/>
    <skos:definition>A project is an activity related to the improvement of a facility, including design and/or construction.  This class may be for the creation, modification, or elimination of the entire facility or a part of the facility.  The Project Requirements Class includes information about projects and their decomposition into project parts.  In order to allow for the condition where none of the LandInfra dataset information is project related, this Requirements Class is optional.</skos:definition>
    <spec:requirementsTested rdf:resource="http://www.opengis.net/spec/landinfra/1.0/req/project"/>
    <rdf:type rdf:resource="http://www.w3.org/2004/02/skos/core#Concept"/>
    <rdf:type rdf:resource="http://www.opengis.net/def/ont/modspec/ConformanceClass"/>
    <spec:conformanceTest rdf:resource="http://www.opengis.net/spec/landinfra/1.0/conf/project/classes"/>
    <skos:broader rdf:resource="http://www.opengis.net/spec/landinfra/1.0/conf/facility"/>
  </rdf:Description>
  <rdf:Description rdf:about="http://www.opengis.net/spec/landinfra/1.0/conf/alignment/CRS">
    <spec:method>Inspect the encoding to verify the above requirement.</spec:method>
    <rdf:type rdf:resource="http://www.w3.org/2004/02/skos/core#Concept"/>
    <rdf:type rdf:resource="http://www.opengis.net/def/ont/modspec/ConformanceTest"/>
    <skos:inScheme rdf:resource="http://www.opengis.net/spec/landinfra/1.0"/>
    <spec:purpose>Verify that an encoding requires that all geometry/locations for Alignment2DHorSegments and Alignment2DVertSegments be specified using the Alignment2DHorizontal.crs which shall be a Cartesian local engineering reference system.</spec:purpose>
    <spec:testType rdf:resource="http://www.opengis.net/def/ont/modspec/Capabilities"/>
    <skos:prefLabel>Conformance Test: http://www.opengis.net/spec/landinfra/1.0/conf/alignment/CRS</skos:prefLabel>
    <skos:narrower rdf:resource="http://www.opengis.net/spec/landinfra/1.0/req/alignment/CRS"/>
    <skos:definition>Verify that an encoding requires that all geometry/locations for Alignment2DHorSegments and Alignment2DVertSegments be specified using the Alignment2DHorizontal.crs which shall be a Cartesian local engineering reference system.</skos:definition>
    <spec:requirement rdf:resource="http://www.opengis.net/spec/landinfra/1.0/req/alignment/CRS"/>
    <skos:broader rdf:resource="http://www.opengis.net/spec/landinfra/1.0/conf/alignment"/>
  </rdf:Description>
  <rdf:Description rdf:about="http://www.opengis.net/spec/landinfra/1.0/conf/land-feature/alignment">
    <skos:broader rdf:resource="http://www.opengis.net/spec/landinfra/1.0/conf/land-feature"/>
    <skos:definition>If an encoding allows the linear element used for a LandLayer to be an Alignment, then verify that the encoding supports the Alignment Requirements class.</skos:definition>
    <rdf:type rdf:resource="http://www.w3.org/2004/02/skos/core#Concept"/>
    <rdf:type rdf:resource="http://www.opengis.net/def/ont/modspec/ConformanceTest"/>
    <skos:prefLabel>Conformance Test: http://www.opengis.net/spec/landinfra/1.0/conf/land-feature/alignment</skos:prefLabel>
    <skos:narrower rdf:resource="http://www.opengis.net/spec/landinfra/1.0/req/land-feature/alignment"/>
    <spec:purpose>If an encoding allows the linear element used for a LandLayer to be an Alignment, then verify that the encoding supports the Alignment Requirements class.</spec:purpose>
    <spec:method>Inspect the encoding to verify the above requirement.</spec:method>
    <skos:inScheme rdf:resource="http://www.opengis.net/spec/landinfra/1.0"/>
    <spec:testType rdf:resource="http://www.opengis.net/def/ont/modspec/Capabilities"/>
    <spec:requirement rdf:resource="http://www.opengis.net/spec/landinfra/1.0/req/land-feature/alignment"/>
  </rdf:Description>
  <rdf:Description rdf:about="http://www.opengis.net/spec/landinfra/1.0/req/alignment/measures">
    <skos:broader rdf:resource="http://www.opengis.net/spec/landinfra/1.0/conf/alignment/measures"/>
    <skos:broader rdf:resource="http://www.opengis.net/spec/landinfra/1.0/req/alignment"/>
    <skos:inScheme rdf:resource="http://www.opengis.net/spec/landinfra/1.0"/>
    <rdf:type rdf:resource="http://www.opengis.net/def/ont/modspec/Requirement"/>
    <rdf:type rdf:resource="http://www.w3.org/2004/02/skos/core#Concept"/>
    <skos:definition>If an Alignment2DHorizontal.2DLinestringRepresentation or an Alignment3D.3DLinestringRepresentation is specified as a linear element, then distanceAlong shall be measured along the LineString and offsetLateralDistance and offsetVerticalDistance values shall be measured normal to the LineString from this DistanceAlong point. If an Alignment2DHorizontal.segment list of Alignment2DHorSegments is used as a linear element, then distanceAlong and offsetLateralDistance values shall be measured in the horizontal plane, ignoring any vertical displacement of the Alignment. OffsetVerticalDistance values shall be absolute from the horizontal plane unless an Alignment2DVertical is specified as a VerticalOffsetReferent so as to take into consideration vertical displacement of the Alignment, if present.</skos:definition>
    <skos:prefLabel>Requirement: /req/alignment/measures</skos:prefLabel>
  </rdf:Description>
  <rdf:Description rdf:about="http://www.opengis.net/spec/landinfra/1.0/conf/alignment/LR-interfaces">
    <skos:inScheme rdf:resource="http://www.opengis.net/spec/landinfra/1.0"/>
    <skos:narrower rdf:resource="http://www.opengis.net/spec/landinfra/1.0/req/alignment/LR-interfaces"/>
    <spec:purpose>Verify that the encoding implements the OGC Abstract Specification Topic 19 ILinearElement and ISpatial interfaces in a manner consistent with the encoding.</spec:purpose>
    <skos:definition>Verify that the encoding implements the OGC Abstract Specification Topic 19 ILinearElement and ISpatial interfaces in a manner consistent with the encoding.</skos:definition>
    <spec:requirement rdf:resource="http://www.opengis.net/spec/landinfra/1.0/req/alignment/LR-interfaces"/>
    <skos:broader rdf:resource="http://www.opengis.net/spec/landinfra/1.0/conf/alignment"/>
    <spec:method>Inspect the encoding to verify the above requirement.</spec:method>
    <rdf:type rdf:resource="http://www.w3.org/2004/02/skos/core#Concept"/>
    <rdf:type rdf:resource="http://www.opengis.net/def/ont/modspec/ConformanceTest"/>
    <spec:testType rdf:resource="http://www.opengis.net/def/ont/modspec/Capabilities"/>
    <skos:prefLabel>Conformance Test: http://www.opengis.net/spec/landinfra/1.0/conf/alignment/LR-interfaces</skos:prefLabel>
  </rdf:Description>
  <rdf:Description rdf:about="http://www.opengis.net/spec/landinfra/1.0/conf/railway/cant">
    <skos:narrower rdf:resource="http://www.opengis.net/spec/landinfra/1.0/req/railway/cant"/>
    <skos:prefLabel>Conformance Test: http://www.opengis.net/spec/landinfra/1.0/conf/railway/cant</skos:prefLabel>
    <spec:method>Inspect the encoding to verify the above requirement.</spec:method>
    <rdf:type rdf:resource="http://www.w3.org/2004/02/skos/core#Concept"/>
    <rdf:type rdf:resource="http://www.opengis.net/def/ont/modspec/ConformanceTest"/>
    <skos:definition>Verify that the encoding specifies as a requirement that each CantSpecification shall cover the entire linear element the CantSpecification is located along from the linear element’s start to its end, and that the CantSpecification shall include CantEvents at the start and end of the linear element and wherever else there is a cant break along the linear element.</skos:definition>
    <spec:testType rdf:resource="http://www.opengis.net/def/ont/modspec/Capabilities"/>
    <spec:requirement rdf:resource="http://www.opengis.net/spec/landinfra/1.0/req/railway/cant"/>
    <skos:inScheme rdf:resource="http://www.opengis.net/spec/landinfra/1.0"/>
    <skos:broader rdf:resource="http://www.opengis.net/spec/landinfra/1.0/conf/railway"/>
    <spec:purpose>Verify that the encoding specifies as a requirement that each CantSpecification shall cover the entire linear element the CantSpecification is located along from the linear element’s start to its end, and that the CantSpecification shall include CantEvents at the start and end of the linear element and wherever else there is a cant break along the linear element.</spec:purpose>
  </rdf:Description>
  <rdf:Description rdf:about="http://www.opengis.net/spec/landinfra/1.0/conf/land-infra/19109">
    <spec:method>Inspect the encoding to verify the above requirement.</spec:method>
    <skos:prefLabel>Conformance Test: http://www.opengis.net/spec/landinfra/1.0/conf/land-infra/19109</skos:prefLabel>
    <rdf:type rdf:resource="http://www.w3.org/2004/02/skos/core#Concept"/>
    <rdf:type rdf:resource="http://www.opengis.net/def/ont/modspec/ConformanceTest"/>
    <spec:requirement rdf:resource="http://www.opengis.net/spec/landinfra/1.0/req/land-infra/19109"/>
    <spec:testType rdf:resource="http://www.opengis.net/def/ont/modspec/Capabilities"/>
    <skos:inScheme rdf:resource="http://www.opengis.net/spec/landinfra/1.0"/>
    <skos:definition>Verify that Features shall be supported by a Land and Infrastructure encoding in accordance with the uml:feature requirement in ISO 19109:2015 Clause 8.2.6 and shown in Figure 9, as follows:   Each instance of FeatureType shall be implemented by the encoding’s equivalent of a UML Class having a generalization association with AnyFeature and with a stereotype of &lt;&lt;FeatureType&gt;&gt;.</skos:definition>
    <skos:broader rdf:resource="http://www.opengis.net/spec/landinfra/1.0/conf/land-infra"/>
    <skos:narrower rdf:resource="http://www.opengis.net/spec/landinfra/1.0/req/land-infra/19109"/>
    <spec:purpose>Verify that Features shall be supported by a Land and Infrastructure encoding in accordance with the uml:feature requirement in ISO 19109:2015 Clause 8.2.6 and shown in Figure 9, as follows:   Each instance of FeatureType shall be implemented by the encoding’s equivalent of a UML Class having a generalization association with AnyFeature and with a stereotype of &lt;&lt;FeatureType&gt;&gt;.</spec:purpose>
  </rdf:Description>
  <rdf:Description rdf:about="http://www.opengis.net/spec/landinfra/1.0/req/land-infra/19109">
    <rdf:type rdf:resource="http://www.opengis.net/def/ont/modspec/Requirement"/>
    <rdf:type rdf:resource="http://www.w3.org/2004/02/skos/core#Concept"/>
    <skos:prefLabel>Requirement: /req/land-infra/19109</skos:prefLabel>
    <skos:broader rdf:resource="http://www.opengis.net/spec/landinfra/1.0/req/land-infra"/>
    <skos:broader rdf:resource="http://www.opengis.net/spec/landinfra/1.0/conf/land-infra/19109"/>
    <skos:definition>Features shall be supported by a Land and Infrastructure encoding in accordance with the uml:feature requirement in ISO 19109:2015 Clause 8.2.6 and shown in Figure 9, as follows: Each instance of FeatureType shall be implemented by the encoding’s equivalent of a UML Class having a generalization association with AnyFeature and with a stereotype of &lt;&gt;.</skos:definition>
    <skos:inScheme rdf:resource="http://www.opengis.net/spec/landinfra/1.0"/>
  </rdf:Description>
  <rdf:Description rdf:about="http://www.opengis.net/spec/landinfra/1.0/conf/railway">
    <skos:narrower rdf:resource="http://www.opengis.net/spec/landinfra/1.0/conf/railway/alignment"/>
    <skos:narrower rdf:resource="http://www.opengis.net/spec/landinfra/1.0/conf/railway/classes"/>
    <skos:narrower rdf:resource="http://www.opengis.net/spec/landinfra/1.0/conf/railway/cant"/>
    <skos:narrower rdf:resource="http://www.opengis.net/spec/landinfra/1.0/req/railway"/>
    <spec:dependency rdf:resource="http://www.opengis.net/spec/landinfra/1.0/conf/facility"/>
    <skos:prefLabel>Conformance Class: Railway</skos:prefLabel>
    <skos:definition>The Railway Requirements Class supports those use cases where a designer wishes to exchange the output of the railway design with someone who is likely to use if for purposes other than further design. Consequently, the Railway Requirements Class covers design output such as 3D railway elements and track geometry including superelevation (cant).</skos:definition>
    <rdf:type rdf:resource="http://www.w3.org/2004/02/skos/core#Concept"/>
    <rdf:type rdf:resource="http://www.opengis.net/def/ont/modspec/ConformanceClass"/>
    <skos:inScheme rdf:resource="http://www.opengis.net/spec/landinfra/1.0"/>
    <spec:requirementsTested rdf:resource="http://www.opengis.net/spec/landinfra/1.0/req/railway"/>
    <spec:conformanceTest rdf:resource="http://www.opengis.net/spec/landinfra/1.0/conf/railway/cant"/>
    <spec:conformanceTest rdf:resource="http://www.opengis.net/spec/landinfra/1.0/conf/railway/alignment"/>
    <spec:conformanceTest rdf:resource="http://www.opengis.net/spec/landinfra/1.0/conf/railway/classes"/>
    <skos:broader rdf:resource="http://www.opengis.net/spec/landinfra/1.0/conf/facility"/>
  </rdf:Description>
  <rdf:Description rdf:about="http://www.opengis.net/spec/landinfra/1.0/req/land-infra">
    <skos:narrower rdf:resource="http://www.opengis.net/spec/landinfra/1.0/req/land-infra/19109"/>
    <skos:narrower rdf:resource="http://www.opengis.net/spec/landinfra/1.0/req/land-infra/19103"/>
    <skos:narrower rdf:resource="http://www.opengis.net/spec/landinfra/1.0/req/land-division"/>
    <skos:narrower rdf:resource="http://www.opengis.net/spec/landinfra/1.0/req/land-infra/topic-19-extensions"/>
    <skos:narrower rdf:resource="http://www.opengis.net/spec/landinfra/1.0/req/facility"/>
    <skos:narrower rdf:resource="http://www.opengis.net/spec/landinfra/1.0/req/land-feature"/>
    <skos:narrower rdf:resource="http://www.opengis.net/spec/landinfra/1.0/req/land-infra/topic-19-core"/>
    <skos:narrower rdf:resource="http://www.opengis.net/spec/landinfra/1.0/req/land-infra/dataset"/>
    <skos:narrower rdf:resource="http://www.opengis.net/spec/landinfra/1.0/req/land-infra/featureID"/>
    <skos:narrower rdf:resource="http://www.opengis.net/spec/landinfra/1.0/req/survey"/>
    <skos:narrower rdf:resource="http://www.opengis.net/spec/landinfra/1.0/req/land-infra/subjects"/>
    <skos:narrower rdf:resource="http://www.opengis.net/spec/landinfra/1.0/req/land-infra/classes"/>
    <skos:narrower rdf:resource="http://www.opengis.net/spec/landinfra/1.0/req/land-infra/topic-1"/>
    <skos:narrower rdf:resource="http://www.opengis.net/spec/landinfra/1.0/req/land-infra/crs"/>
    <skos:definition>Requirement Class: LandInfra</skos:definition>
    <skos:prefLabel>Requirement Class: LandInfra</skos:prefLabel>
    <spec:normativeStatement rdf:resource="http://www.opengis.net/spec/landinfra/1.0/req/land-infra/topic-19-extensions"/>
    <spec:normativeStatement rdf:resource="http://www.opengis.net/spec/landinfra/1.0/req/land-infra/topic-19-core"/>
    <spec:normativeStatement rdf:resource="http://www.opengis.net/spec/landinfra/1.0/req/land-infra/dataset"/>
    <spec:normativeStatement rdf:resource="http://www.opengis.net/spec/landinfra/1.0/req/land-infra/subjects"/>
    <spec:normativeStatement rdf:resource="http://www.opengis.net/spec/landinfra/1.0/req/land-infra/topic-1"/>
    <spec:normativeStatement rdf:resource="http://www.opengis.net/spec/landinfra/1.0/req/land-infra/featureID"/>
    <spec:normativeStatement rdf:resource="http://www.opengis.net/spec/landinfra/1.0/req/land-infra/19109"/>
    <spec:normativeStatement rdf:resource="http://www.opengis.net/spec/landinfra/1.0/req/land-infra/19103"/>
    <spec:normativeStatement rdf:resource="http://www.opengis.net/spec/landinfra/1.0/req/land-infra/classes"/>
    <spec:normativeStatement rdf:resource="http://www.opengis.net/spec/landinfra/1.0/req/land-infra/crs"/>
    <skos:inScheme rdf:resource="http://www.opengis.net/spec/landinfra/1.0"/>
    <rdf:type rdf:resource="http://www.opengis.net/def/ont/modspec/RequirementClass"/>
    <rdf:type rdf:resource="http://www.w3.org/2004/02/skos/core#Concept"/>
    <skos:broader rdf:resource="http://www.opengis.net/spec/landinfra/1.0/conf/land-infra"/>
  </rdf:Description>
  <rdf:Description rdf:about="http://www.opengis.net/spec/landinfra/1.0/req/road">
    <skos:inScheme rdf:resource="http://www.opengis.net/spec/landinfra/1.0"/>
    <spec:normativeStatement rdf:resource="http://www.opengis.net/spec/landinfra/1.0/req/road/alignment"/>
    <spec:normativeStatement rdf:resource="http://www.opengis.net/spec/landinfra/1.0/req/road-cross-section/alignment"/>
    <spec:normativeStatement rdf:resource="http://www.opengis.net/spec/landinfra/1.0/req/road/classes"/>
    <spec:normativeStatement rdf:resource="http://www.opengis.net/spec/landinfra/1.0/req/road-cross-section/classes"/>
    <rdf:type rdf:resource="http://www.opengis.net/def/ont/modspec/RequirementClass"/>
    <rdf:type rdf:resource="http://www.w3.org/2004/02/skos/core#Concept"/>
    <skos:broader rdf:resource="http://www.opengis.net/spec/landinfra/1.0/conf/road"/>
    <skos:broader rdf:resource="http://www.opengis.net/spec/landinfra/1.0/req/facility"/>
    <spec:dependency rdf:resource="http://www.opengis.net/spec/landinfra/1.0/req/facility"/>
    <skos:definition>The Road Requirements Class supports those use cases in which a designer wishes to exchange the output of the design with someone who is likely to use it for purposes other than completing the road design.  Consequently, the Road Requirements Class includes several alternative ways for representing a design such as with 3D RoadElements, 3D StringLines (aka profile views, longitudinal breaklines, long sections), and 3D surfaces and layers, as well as collections of these. </skos:definition>
    <skos:narrower rdf:resource="http://www.opengis.net/spec/landinfra/1.0/req/road-cross-section"/>
    <skos:narrower rdf:resource="http://www.opengis.net/spec/landinfra/1.0/req/road-cross-section/alignment"/>
    <skos:narrower rdf:resource="http://www.opengis.net/spec/landinfra/1.0/req/road/classes"/>
    <skos:narrower rdf:resource="http://www.opengis.net/spec/landinfra/1.0/req/road-cross-section/classes"/>
    <skos:narrower rdf:resource="http://www.opengis.net/spec/landinfra/1.0/req/road/alignment"/>
    <skos:prefLabel>Requirement Class: Road</skos:prefLabel>
  </rdf:Description>
  <rdf:Description rdf:about="http://www.opengis.net/spec/landinfra/1.0/req/land-infra/subjects">
    <skos:broader rdf:resource="http://www.opengis.net/spec/landinfra/1.0/conf/land-infra/subjects"/>
    <skos:broader rdf:resource="http://www.opengis.net/spec/landinfra/1.0/req/land-infra"/>
    <rdf:type rdf:resource="http://www.w3.org/2004/02/skos/core#Concept"/>
    <rdf:type rdf:resource="http://www.opengis.net/def/ont/modspec/Requirement"/>
    <skos:inScheme rdf:resource="http://www.opengis.net/spec/landinfra/1.0"/>
    <skos:definition>A Land and Infrastructure encoding shall specify which of the LandInfra subjects it supports: Facility, LandFeature, LandDivision, and Survey.</skos:definition>
    <skos:prefLabel>Requirement: /req/land-infra/subjects</skos:prefLabel>
  </rdf:Description>
  <rdf:Description rdf:about="http://www.opengis.net/spec/landinfra/1.0/req/land-feature/alignment">
    <rdf:type rdf:resource="http://www.w3.org/2004/02/skos/core#Concept"/>
    <rdf:type rdf:resource="http://www.opengis.net/def/ont/modspec/Requirement"/>
    <skos:prefLabel>Requirement: /req/land-feature/alignment</skos:prefLabel>
    <skos:broader rdf:resource="http://www.opengis.net/spec/landinfra/1.0/conf/land-feature/alignment"/>
    <skos:broader rdf:resource="http://www.opengis.net/spec/landinfra/1.0/req/land-feature"/>
    <skos:inScheme rdf:resource="http://www.opengis.net/spec/landinfra/1.0"/>
    <skos:definition>If an encoding allows the linear element used for a LandLayer to be an Alignment, then that encoding shall support the Alignment Requirements Class.</skos:definition>
  </rdf:Description>
  <rdf:Description rdf:about="http://www.opengis.net/spec/landinfra/1.0/conf/equipment/classes">
    <skos:inScheme rdf:resource="http://www.opengis.net/spec/landinfra/1.0"/>
    <skos:broader rdf:resource="http://www.opengis.net/spec/landinfra/1.0/conf/equipment"/>
    <spec:testType rdf:resource="http://www.opengis.net/def/ont/modspec/Capabilities"/>
    <rdf:type rdf:resource="http://www.opengis.net/def/ont/modspec/ConformanceTest"/>
    <rdf:type rdf:resource="http://www.w3.org/2004/02/skos/core#Concept"/>
    <skos:narrower rdf:resource="http://www.opengis.net/spec/landinfra/1.0/req/equipment/classes"/>
    <spec:purpose>Verify that the encoding provides the Equipment Requirements Class Classes shown in blue in Figure 48 in a manner consistent with the encoding.  An encoding shall decide which SurveySensor types it will support and define appropriate requirements classes accordingly.</spec:purpose>
    <skos:prefLabel>Conformance Test: http://www.opengis.net/spec/landinfra/1.0/conf/equipment/classes</skos:prefLabel>
    <spec:method>Inspect the encoding to verify the above requirement.</spec:method>
    <spec:requirement rdf:resource="http://www.opengis.net/spec/landinfra/1.0/req/equipment/classes"/>
    <skos:definition>Verify that the encoding provides the Equipment Requirements Class Classes shown in blue in Figure 48 in a manner consistent with the encoding.  An encoding shall decide which SurveySensor types it will support and define appropriate requirements classes accordingly.</skos:definition>
  </rdf:Description>
  <rdf:Description rdf:about="http://www.opengis.net/spec/landinfra/1.0/req/land-infra/topic-19-core">
    <skos:prefLabel>Requirement: /req/land-infra/topic-19-core</skos:prefLabel>
    <skos:inScheme rdf:resource="http://www.opengis.net/spec/landinfra/1.0"/>
    <skos:broader rdf:resource="http://www.opengis.net/spec/landinfra/1.0/req/land-infra"/>
    <skos:broader rdf:resource="http://www.opengis.net/spec/landinfra/1.0/conf/land-infra/topic-19-core"/>
    <rdf:type rdf:resource="http://www.opengis.net/def/ont/modspec/Requirement"/>
    <rdf:type rdf:resource="http://www.w3.org/2004/02/skos/core#Concept"/>
    <skos:definition>If a Land and Infrastructure encoding supports linearly referenced locations, then the encoding shall support the PositionExpression and related Classes specified in the OGC Abstract Specification Topic 19, core Linear Referencing (LR) Package shown in pink in Figure 7 that are appropriate to the supported subject area(s).</skos:definition>
  </rdf:Description>
  <rdf:Description rdf:about="http://www.opengis.net/spec/landinfra/1.0/conf/alignment/classes">
    <skos:broader rdf:resource="http://www.opengis.net/spec/landinfra/1.0/conf/alignment"/>
    <spec:method>Inspect the encoding to verify the above requirement.</spec:method>
    <spec:purpose>If an encoding includes Alignments, then verify that the encoding provides the Alignment Requirements Class Classes shown in blue in Figure 15 in a manner consistent with the encoding.</spec:purpose>
    <spec:testType rdf:resource="http://www.opengis.net/def/ont/modspec/Capabilities"/>
    <spec:requirement rdf:resource="http://www.opengis.net/spec/landinfra/1.0/req/alignment/classes"/>
    <skos:prefLabel>Conformance Test: http://www.opengis.net/spec/landinfra/1.0/conf/alignment/classes</skos:prefLabel>
    <skos:narrower rdf:resource="http://www.opengis.net/spec/landinfra/1.0/req/alignment/classes"/>
    <skos:definition>If an encoding includes Alignments, then verify that the encoding provides the Alignment Requirements Class Classes shown in blue in Figure 15 in a manner consistent with the encoding.</skos:definition>
    <skos:inScheme rdf:resource="http://www.opengis.net/spec/landinfra/1.0"/>
    <rdf:type rdf:resource="http://www.w3.org/2004/02/skos/core#Concept"/>
    <rdf:type rdf:resource="http://www.opengis.net/def/ont/modspec/ConformanceTest"/>
  </rdf:Description>
  <rdf:Description rdf:about="http://www.opengis.net/spec/landinfra/1.0/req/facility/classes">
    <skos:inScheme rdf:resource="http://www.opengis.net/spec/landinfra/1.0"/>
    <skos:prefLabel>Requirement: /req/facility/classes</skos:prefLabel>
    <rdf:type rdf:resource="http://www.w3.org/2004/02/skos/core#Concept"/>
    <rdf:type rdf:resource="http://www.opengis.net/def/ont/modspec/Requirement"/>
    <skos:definition>The Facility Requirements Class Classes shown in blue in Figure 10 shall be provided for by the encoding in a manner consistent with the encoding.</skos:definition>
    <skos:broader rdf:resource="http://www.opengis.net/spec/landinfra/1.0/req/facility"/>
    <skos:broader rdf:resource="http://www.opengis.net/spec/landinfra/1.0/conf/facility/classes"/>
  </rdf:Description>
  <rdf:Description rdf:about="http://www.opengis.net/spec/landinfra/1.0/req/railway/cant">
    <rdf:type rdf:resource="http://www.w3.org/2004/02/skos/core#Concept"/>
    <rdf:type rdf:resource="http://www.opengis.net/def/ont/modspec/Requirement"/>
    <skos:broader rdf:resource="http://www.opengis.net/spec/landinfra/1.0/conf/railway/cant"/>
    <skos:broader rdf:resource="http://www.opengis.net/spec/landinfra/1.0/req/railway"/>
    <skos:definition>An encoding shall specify as a requirement that each CantSpecification shall cover the entire linear element the CantSpecification is located along from the linear element’s start to its end, and that the CantSpecification shall include CantEvents at the start and end of the linear element and wherever else there is a cant break along the linear element.</skos:definition>
    <skos:inScheme rdf:resource="http://www.opengis.net/spec/landinfra/1.0"/>
    <skos:prefLabel>Requirement: /req/railway/cant</skos:prefLabel>
  </rdf:Description>
  <rdf:Description rdf:about="http://www.opengis.net/spec/landinfra/1.0/req/land-infra/dataset">
    <rdf:type rdf:resource="http://www.opengis.net/def/ont/modspec/Requirement"/>
    <rdf:type rdf:resource="http://www.w3.org/2004/02/skos/core#Concept"/>
    <skos:prefLabel>Requirement: /req/land-infra/dataset</skos:prefLabel>
    <skos:broader rdf:resource="http://www.opengis.net/spec/landinfra/1.0/conf/land-infra/dataset"/>
    <skos:broader rdf:resource="http://www.opengis.net/spec/landinfra/1.0/req/land-infra"/>
    <skos:definition>A Land and Infrastructure encoding shall specify a LandInfra dataset in whatever format that is appropriate to that encoding (e.g., an XML document for a GML encoding).</skos:definition>
    <skos:inScheme rdf:resource="http://www.opengis.net/spec/landinfra/1.0"/>
  </rdf:Description>
  <rdf:Description rdf:about="http://www.opengis.net/spec/landinfra/1.0/req/land-infra/19103">
    <skos:definition>A Land and Infrastructure encoding shall support the core data types specified in ISO 19103 Clause 7 and shown in pink in Figure 5 that are appropriate to the supported subject area(s).</skos:definition>
    <skos:broader rdf:resource="http://www.opengis.net/spec/landinfra/1.0/conf/land-infra/19103"/>
    <skos:broader rdf:resource="http://www.opengis.net/spec/landinfra/1.0/req/land-infra"/>
    <skos:inScheme rdf:resource="http://www.opengis.net/spec/landinfra/1.0"/>
    <rdf:type rdf:resource="http://www.opengis.net/def/ont/modspec/Requirement"/>
    <rdf:type rdf:resource="http://www.w3.org/2004/02/skos/core#Concept"/>
    <skos:prefLabel>Requirement: /req/land-infra/19103</skos:prefLabel>
  </rdf:Description>
  <rdf:Description rdf:about="http://www.opengis.net/spec/landinfra/1.0/conf/alignment/description">
    <rdf:type rdf:resource="http://www.w3.org/2004/02/skos/core#Concept"/>
    <rdf:type rdf:resource="http://www.opengis.net/def/ont/modspec/ConformanceTest"/>
    <skos:definition>Verify that an encoding which includes Alignments shall specify that all of the included Alignments shall be continuous, non-overlapping, and non-branching (though it may contain intersections with other Alignments) and that if it is used within the context of a Project, the included Alignment shall be for a single alternative, as specified by the ProjectPart.</skos:definition>
    <skos:broader rdf:resource="http://www.opengis.net/spec/landinfra/1.0/conf/alignment"/>
    <spec:requirement rdf:resource="http://www.opengis.net/spec/landinfra/1.0/req/alignment/description"/>
    <skos:inScheme rdf:resource="http://www.opengis.net/spec/landinfra/1.0"/>
    <skos:narrower rdf:resource="http://www.opengis.net/spec/landinfra/1.0/req/alignment/description"/>
    <spec:purpose>Verify that an encoding which includes Alignments shall specify that all of the included Alignments shall be continuous, non-overlapping, and non-branching (though it may contain intersections with other Alignments) and that if it is used within the context of a Project, the included Alignment shall be for a single alternative, as specified by the ProjectPart.</spec:purpose>
    <spec:method>Inspect the encoding to verify the above requirement.</spec:method>
    <skos:prefLabel>Conformance Test: http://www.opengis.net/spec/landinfra/1.0/conf/alignment/description</skos:prefLabel>
    <spec:testType rdf:resource="http://www.opengis.net/def/ont/modspec/Capabilities"/>
  </rdf:Description>
  <rdf:Description rdf:about="http://www.opengis.net/spec/landinfra/1.0/req/road-cross-section/classes">
    <rdf:type rdf:resource="http://www.w3.org/2004/02/skos/core#Concept"/>
    <rdf:type rdf:resource="http://www.opengis.net/def/ont/modspec/Requirement"/>
    <skos:prefLabel>Requirement: /req/road-cross-section/classes</skos:prefLabel>
    <skos:broader rdf:resource="http://www.opengis.net/spec/landinfra/1.0/req/road"/>
    <skos:broader rdf:resource="http://www.opengis.net/spec/landinfra/1.0/conf/road-cross-section/classes"/>
    <skos:broader rdf:resource="http://www.opengis.net/spec/landinfra/1.0/req/road-cross-section"/>
    <skos:definition>The RoadCrossSection Requirements Class Classes shown in blue in Figure 25 shall be provided for by the encoding in a manner consistent with the encoding.</skos:definition>
    <skos:inScheme rdf:resource="http://www.opengis.net/spec/landinfra/1.0"/>
  </rdf:Description>
  <rdf:Description rdf:about="http://www.opengis.net/spec/landinfra/1.0/req/observations/classes">
    <skos:definition>The Observations Requirements Class Classes shown in blue in Figure 41Figure 43 shall be provided for by the encoding in a manner consistent with the encoding. An encoding shall decide which SurveyObservation types it will support and define appropriate requirements classes accordingly. This then would include any dependent types (example SatelliteSystemType has only to be supported if the encoding will support GNSS Observations).</skos:definition>
    <rdf:type rdf:resource="http://www.opengis.net/def/ont/modspec/Requirement"/>
    <rdf:type rdf:resource="http://www.w3.org/2004/02/skos/core#Concept"/>
    <skos:broader rdf:resource="http://www.opengis.net/spec/landinfra/1.0/conf/observations/classes"/>
    <skos:broader rdf:resource="http://www.opengis.net/spec/landinfra/1.0/req/observations"/>
    <skos:prefLabel>Requirement: /req/observations/classes</skos:prefLabel>
    <skos:inScheme rdf:resource="http://www.opengis.net/spec/landinfra/1.0"/>
  </rdf:Description>
  <rdf:Description rdf:about="http://www.opengis.net/spec/landinfra/1.0/req/equipment/classes">
    <skos:prefLabel>Requirement: /req/equipment/classes</skos:prefLabel>
    <rdf:type rdf:resource="http://www.opengis.net/def/ont/modspec/Requirement"/>
    <rdf:type rdf:resource="http://www.w3.org/2004/02/skos/core#Concept"/>
    <skos:broader rdf:resource="http://www.opengis.net/spec/landinfra/1.0/req/equipment"/>
    <skos:broader rdf:resource="http://www.opengis.net/spec/landinfra/1.0/conf/equipment/classes"/>
    <skos:definition>The Equipment Requirements Class Classes shown in blue in Figure 48 shall be provided for by the encoding in a manner consistent with the encoding. An encoding shall decide which SurveySensor types it will support and define appropriate requirements classes accordingly.</skos:definition>
    <skos:inScheme rdf:resource="http://www.opengis.net/spec/landinfra/1.0"/>
  </rdf:Description>
  <rdf:Description rdf:about="http://www.opengis.net/spec/landinfra/1.0/req/alignment/description">
    <rdf:type rdf:resource="http://www.opengis.net/def/ont/modspec/Requirement"/>
    <rdf:type rdf:resource="http://www.w3.org/2004/02/skos/core#Concept"/>
    <skos:broader rdf:resource="http://www.opengis.net/spec/landinfra/1.0/req/alignment"/>
    <skos:broader rdf:resource="http://www.opengis.net/spec/landinfra/1.0/conf/alignment/description"/>
    <skos:prefLabel>Requirement: /req/alignment/description</skos:prefLabel>
    <skos:inScheme rdf:resource="http://www.opengis.net/spec/landinfra/1.0"/>
    <skos:definition>An encoding which includes Alignments shall specify that all of the included Alignments shall be continuous, non-overlapping, and non-branching (though it may contain intersections with other Alignments) and that if it is used within the context of a Project, the included Alignment shall be for a single alternative, as specified by the ProjectPart.</skos:definition>
  </rdf:Description>
</rdf:RDF>
