@prefix hyf: <https://www.opengis.net/def/schema/hy_features/hyf/> .
@prefix owl: <http://www.w3.org/2002/07/owl#> .
@prefix skos: <http://www.w3.org/2004/02/skos/core#> .

skos:definition a owl:AnnotationProperty .

hyf:HY_Canal a skos:Concept ;
    skos:broader hyf:HY_WaterBody ;
    skos:definition "The HY_Canal feature type defines the existence of body of surface water, participating in a hydrographic network, special due to its artificial origin (man-made)."@en ;
    skos:inScheme hyf: .

hyf:HY_CartographicRealization a skos:Concept ;
    skos:broader hyf:HY_CatchmentRealization ;
    skos:definition """The HY_CartographicRealization feature type realizes a catchment as set of separate cartographic layers or maps, displaying a network of hydrologic features which may be connected at the representation level, or not.

Specializing HY_CatchmentRealization, it inherits from generalization the shape attribute and the realizedCatchment association."""@en ;
    skos:inScheme hyf: .

hyf:HY_CatchmentAggregate a skos:Concept ;
    skos:broader hyf:HY_Catchment ;
    skos:definition """The HY_CatchmentAggregate feature type (Figure 30) specializes the HY_Catchment type as a set of non-overlapping dendritic and interior catchments arranged in an encompassing catchment. This can be used to describe multiple inflows into a catchment aggregate through several hydrologically discrete sub-catchments each with a single inflow, and contributing to a joined outflow of the catchment aggregate, including the 'nillable' outflow of interior catchments. Nillable is meant here to signify that the hydro nexus logically exists in the form of flow to the subsurface or atmosphere but is unknown in a given implementation.

Being a special type of the HY_Catchment, the catchment aggregate may be part of a containing catchment at the next higher level of hierarchy, which consists of similar-scale neighboring catchments. The catchment aggregate does not necessarily imply a series of nested containing catchments. It primarily allows navigation to the 'highest' level system (total drainage basin) as typically used for reporting purposes.

HY_CatchmentAggregate inherits through generalization the outflow, inflow, containingCatchment, containedCatchment, conjointCatchment, upperCatchment, lowerCatchment, and catchmentRealization properties, and has exorheicDrainage and endorheicDrainage associations."""@en ;
    skos:inScheme hyf: .

hyf:HY_CatchmentArea a skos:Concept ;
    skos:broader hyf:HY_CatchmentRealization ;
    skos:definition """The HY_CatchmentArea feature type realizes a catchment specifically as a catchment area connecting the inflow and outflow of the catchment it realizes.

HY_CatchmentArea specializes HY_CatchmentRealization with respect to an implied areal geometric representation. Topologically, the catchment area connecting the inflow and outflow of the catchment is a face bounded inwards by an inflow edge and outwards by an outflow edge. Hydrologically, catchment area refers to the area having a common outlet for its runoff.

Through generalization, HY_CatchmentArea inherits the shape and the realizedCatchment properties. The optional shape of the catchment may be implemented as a surface."""@en ;
    skos:inScheme hyf: .

hyf:HY_CatchmentDivide a skos:Concept ;
    skos:broader hyf:HY_CatchmentRealization ;
    skos:definition """The HY_CatchmentDivide feature type realizes a catchment specifically as catchment boundary connecting the inflow and outflow of the catchment it realizes, whereby inflow and outflow may overlay.

Implying a linear geometric representation, a catchment boundary is topologically understood as an edge bounded by inflow node and outflow nodes, and corresponding to left-bank and right-bank catchment faces inside of the boundary. Hydrologically, the boundary refers to the summit line separating adjacent catchments.

Through generalization, HY_CatchmentDivide inherits the shape and the realizedCatchment properties. The shape of the catchment divide may be implemented as a composition of succeeding curves or a polygon ring."""@en ;
    skos:inScheme hyf: .

hyf:HY_Channel a skos:Concept ;
    skos:broader hyf:HY_Depression ;
    skos:definition """The HY_Channel feature type specializes the HY_Depression class with respect to a natural or man-made, open or closed channel through or along which water may or may not flow. A channel is part of the network of channels and depressions which forms the connecting system for the hydrographic network; a channel may have vertical sections at right angles to the main (average) direction of flow or along its centerline.

HY_Channel has an association indicating the channelNetwork in which it participates. It carries the associations: stream, bedProfileTransversal and bedProfileLongitudinal. HY_Channel inherits from generalization the confinedWaterBody association and the outflow-at-benchmark constraint. An outlet-at-profile constraint emphasizes the recognition of vertical section as the outlet of the catchment that is realized by the channel network."""@en ;
    skos:inScheme hyf: .

hyf:HY_ChannelNetwork a skos:Concept ;
    skos:definition """The HY_ChannelNetwork feature type specializes the HY_HydroNetwork realization defined in the Hydro Feature core model, specifically as an aggregate of surface depressions and surface channels which continuously or periodically contain water, without imposing a particular drainage pattern. This allows representation of the network, even if logically connected features are not connected at the representation level. If the realized catchment is connected with other catchments via hydro nexuses, the channel network is considered connected to the channel network realizing these catchments.

HY_ChannelNetwork has surfaceDepression and surfaceChannel associations, and carries a drainagePattern attribute; it inherits through generalization the shape attribute, the realizedCatchment association as well as flowpath, catchmentDivide and catchmentArea associations. Depending on the application, the channel network and the related features may be described by suitable attributes. A channel-flowpath constraint is defined to support the recognition of the channel as flowpath realizing the catchment."""@en ;
    skos:inScheme hyf: ;
    skos:topConceptOf hyf: .

hyf:HY_CrossSection a skos:Concept ;
    skos:definition """The HY_CrossSection feature type conceptualizes the segmentation of a waterbody or a containing channel through vertical sections. Taking into account the conceptual separation of a watercourse, the cross section concept refers to both the cross section of a waterbody orthogonal to the direction of flow, and to the transversal bed profile of a channel.

A cross section associates a crossSectionPoint which should be used to identify a permanent reference location at a vertical section which realizes the conceptual hydro nexus of the catchment realized by the associated channel or waterbody."""@en ;
    skos:inScheme hyf: ;
    skos:topConceptOf hyf: .

hyf:HY_DendriticCatchment a skos:Concept ;
    skos:broader hyf:HY_Catchment ;
    skos:definition """The HY_DendriticCatchment feature type (Figure 31) specializes the general HY_Catchment class as a catchment which is determined by a single common downstream catchment. It represents the catchment as the topological link between an inflow and an outflow. This allows catchments to be connected in a dendritic network by upstream-downstream relationships without knowing the complex hydrology between inflow and outflow. This concept requires a stable identifier purposefully assigned to the catchment and that catchments are delineated as a simple tree hierarchy.

HY_DendriticCatchment inherits from generalization the code, outflow, inflow, containingCatchment, containedCatchment, conjointCatchment, upperCatchment, lowerCatchment, and catchmentRealization properties, and has an encompassingCatchment association. The dendritic nature of this feature is enforced through single-outflow, single-receiving-catchment and single-lower-catchment constraints."""@en ;
    skos:inScheme hyf: .

hyf:HY_Estuary a skos:Concept ;
    skos:broader hyf:HY_WaterBody ;
    skos:definition "The HY_Estuary feature type defines the existence of body of surface water, participating in a hydrographic network, special due to branching and its interaction with the open sea."@en ;
    skos:inScheme hyf: .

hyf:HY_FlowPath a skos:Concept ;
    skos:broader hyf:HY_CatchmentRealization ;
    skos:definition """The HY_Flowpath feature type realizes a catchment specifically as a path connecting the inflow and outflow of the catchment it realizes.

HY_Flowpath specializes HY_CatchmentRealization with respect to an implied linear geometric representation including a straight or curved line. Topologically, the flowpath connects the inflow and outflow of the catchment, and is understood as an edge bounded by an inflow node and an outflow node, and corresponding to left-bank and right-bank catchment faces. Hydrologically, the flowpath is a line describing a moving particle of water.

Through generalization, HY_Flowpath inherits the shape and the realizedCatchment properties. The optional shape of the flowpath is usually a single curve."""@en ;
    skos:inScheme hyf: .

hyf:HY_HydroFeatureName a skos:Concept ;
    skos:definition "pattern to handle cultural, political and historical variability of names. This supports the assignment of a referenceable name for all or parts of a hydrologic feature without necessarily having a formal model for the naming."@en ;
    skos:inScheme hyf: ;
    skos:topConceptOf hyf: .

hyf:HY_HydroLocation a skos:Concept ;
    skos:definition """The HY_HydroLocation feature type (Figure 35) conceptualizes the idea that a hydro nexus can be realized by practically any feature of interest. The hydro nexus concept is used to define the hydrologic determination of a catchment but, like the catchment concept, does not have inherent realization(s). Any hydrologically significant feature that can be identified as (said to be) the outlet of a catchment may realize the hydro nexus. Typically, this will be a permanent, stable location that is fixed and/or referenced by coordinates.

Landmarks such as confluences, points corresponding to vertical sections, or the position of a monitoring station on a river are typical realizations of the hydro nexus. Other kinds of hydro nexus realizations that don't carry normal surface water characteristics as defined in this standard, e.g. a spring where groundwater enters the surface, an arbitrary point projected onto the surface, or a nexus that collects many disjoint locations may use or specialize the general HY_HydroLocation type.

Topologically, the HY_HydroLocation should be understood to be the boundary of the corresponding catchment, and always of lower topological dimension than the catchment. Even though the topological realization of a hydro nexus is typically as a node between catchment edges, a nexus realization may also have any geometric representation, including a single point.

In many cases, HY_HydroLocations are known but corresponding catchments and hydro nexuses are not defined. For example, stream gages that are part of a catchment dataset whose hydro nexus features are realized by confluences. Both the stream gages and confluences are HY_HydroLocations, but the stream gages’ hydro nexus features are not defined. Using this concept, HY_HydroLocation is expected to be used to link between datasets that have catchments delineated for different HY_HydroLocations.

HY_HydroLocation carries two attributes: shape and hydroLocationType. It has referencedPosition and realizedNexus associations implying the hydro-complex feature collection."""@en ;
    skos:inScheme hyf: ;
    skos:prefLabel "ReferenceLocation"@en ;
    skos:topConceptOf hyf: .

hyf:HY_HydroNetwork a skos:Concept ;
    skos:broader hyf:HY_CatchmentRealization ;
    skos:definition """The HY_HydroNetwork feature type realizes a catchment as a network of connected hydrologic features. Such a network realizes the hierarchical network of logically connected catchments contained in a larger catchment. It may be a sequence of flowpaths, an aggregate of catchment areas or a mesh of catchment divides.

HY_HydroNetwork feature type specializes HY_CatchmentRealization. Through generalization it inherits the shape and the realizedCatchment properties, and carries the associations flowpath, catchmentDivide and catchmentArea. The optional shape of the is usually given through the individual geometry of the network parts."""@en ;
    skos:inScheme hyf: .

hyf:HY_HydroNexus a skos:Concept ;
    skos:definition """The HY_HydroNexus feature type (Figure 33) conceptualizes a hydrologically determined nexus of a corresponding catchment (Figure 26). The hydro nexus represents the place where a catchment interacts with another catchment, i.e. where the outflow of a contributing catchment becomes inflow into a receiving catchment. A catchment may receive flow from several upstream catchments or contribute flow to several downstream catchments through a single hydro nexus. Through shared identity, each hydro nexus feature may be associated with different realizations within a hydrologic complex given that each realization has the same hydrologic function or characteristics. This includes the topological realization as a node on the one-dimensional flowpath (edge) in terms of a topological 'boundary'.

Placed topologically relative to a catchment which links inflow and outflow, a hydro nexus has a position relative to another hydro nexus that is 'fixed' in the network by the catchments it is associated with. Additionally, the union of catchment and hydro nexus(es) can be used to define a linear river reference system, where an inflow or outflow node is the origin and the flowpath realizing the catchment is the linear element along which a position can be determined."""@en ;
    skos:inScheme hyf: ;
    skos:topConceptOf hyf: .

hyf:HY_HydrographicNetwork a skos:Concept ;
    skos:definition """The HY_HydrographicNetwork feature type specializes the HY_HydroNetwork realization defined in the Hydro Feature core model, specifically as an aggregate of permanent or temporary bodies standing in depressions or moving in channels. If the realized catchment is connected with other catchments via hydro nexuses, the hydrographic network is considered connected to the network realizing these catchments. This allows representation of the network, even if logically connected features are not connected at the representation level. If required, an application focused on surface-waterbodies contained in channels or depressions may use the defined relationships to describe the realization of a catchment by the hydrographic network, or network parts associated with the channel network.

HY_HydrographicNetwork has a networkWaterBody association. Through generalization, it inherits the shape attribute and the realizedCatchment association as well as flowpath, catchmentDivide and catchmentArea associations, and. A waterbody-flowpath constraint supports the recognition of the waterbody as a flowpath realizing the catchment."""@en ;
    skos:inScheme hyf: ;
    skos:topConceptOf hyf: .

hyf:HY_HydrometricFeature a skos:Concept ;
    skos:definition """The HY_HydrometricFeature feature type provides a concept of a monitoring station at which data on water are obtained that realizes the catchment either separately or as part of the hydrometric network (Figure 45).

HY_HydrometricFeature has associations for the hydrometricNetwork in which it participates, and a positionOnRiver. An outlet-at-station constraint emphasizes the recognition of a monitoring station as outlet of the catchment that is realized by the hydrometric network."""@en ;
    skos:inScheme hyf: ;
    skos:topConceptOf hyf: .

hyf:HY_HydrometricNetwork a skos:Concept ;
    skos:definition """The HY_HydrometricNetwork feature type specializes the HY_HydroNetwork realization specifically as an aggregate of hydrometric features.

HY_HydrometricNetwork has a networkStation association, and inherits through generalization the shape attribute, the realizedCatchment, flowpath, catchmentDivide and catchmentArea associations."""@en ;
    skos:inScheme hyf: ;
    skos:topConceptOf hyf: .

hyf:HY_Impoundment a skos:Concept ;
    skos:broader hyf:HY_WaterBody ;
    skos:definition "The HY_Impoundment feature type defines the existence of body of surface water, participating in a hydrographic network, special due to be formed by collecting water, as by a dam."@en ;
    skos:inScheme hyf: .

hyf:HY_IndirectPosition a skos:Concept ;
    skos:definition """The HY_IndirectPosition feature type defines the location referenced along an axis, without the necessity of a geometric realization. Indirect position uses a catchment-specific reference system which defines the flowpath as the required linear element along which the position is determined. The indirect position is then expressed as the distance from the upstream and/or downstream end of the flowpath, or from a referent that is already located on that flowpath.

The (indirect) position of an outflow node referenced along an upstream oriented flowpath can be expressed as the distance from an upstream inflow node located on that flowpath, while the (indirect) position of an inflow node referenced along a downstream oriented flowpath can be expressed as distance from a downstream outflow node located on the flowpath. An ‘intermediate’ position referencing known inflow and outflow nodes bounding a flowpath at both ends can be expressed as part of the distance along the entire flowpath, measured from the upstream end of an upstream flowpath, and/or from the downstream end of a downstream flowpath. A position referencing an already referenced location on the flowpath can be expressed as part of the distance along the entire flowpath, measured from the ‘located referent’.

HY_IndirectPosition carries the distanceExpression, and distanceDescription attributes, and has linearElement, locatedReferent and a referenceLocation associations. A point-referent constraint emphasizes the topological relationship between the linear element and point representation of the reference location; a measure-along-flowpath constraint defines the flowpath as the linear element to be used whenever a position is expressed as a distance from a referent."""@en ;
    skos:inScheme hyf: ;
    skos:topConceptOf hyf: .

hyf:HY_InteriorCatchment a skos:Concept ;
    skos:broader hyf:HY_Catchment ;
    skos:definition "The HY_InteriorCatchment feature type (Figure 32) specializes the general HY_Catchment class as a catchment which is generally not connected to other catchments. This class describes the interior catchment as a catchment enveloped by other catchments to which it may temporarily contribute. While the interior catchment concept precludes flow to neighboring surface catchments, holistically it is a candidate for establishing connections to groundwater or atmospheric systems."@en ;
    skos:inScheme hyf: .

hyf:HY_Lagoon a skos:Concept ;
    skos:broader hyf:HY_WaterBody ;
    skos:definition "The HY_Lagoon feature type defines the existence of body of surface water, participating in a hydrographic network, special due to its shallow depth and interaction with the open sea."@en ;
    skos:inScheme hyf: .

hyf:HY_Lake a skos:Concept ;
    skos:broader hyf:HY_WaterBody ;
    skos:definition "The HY_Lake feature type defines the existence of body of surface water, participating in a hydrographic network, special due to its considerable size."@en ;
    skos:inScheme hyf: .

hyf:HY_LongitudinalSection a skos:Concept ;
    skos:definition """The HY_LongitudinalSection feature type conceptualizes the segmentation of a waterbody or a containing channel through vertical sections. Taking into account the conceptual separation of a watercourse, the longitudinal section concept refers to both the vertical section of a waterbody along its centerline, and to the longitudinal bed profile of a channel.

A longitudinal section associates a longitudalinalSectionPoint which should be used to identify a permanent reference location at a vertical section which realizes the conceptual hydro nexus of the catchment realized by the associated channel or waterbody."""@en ;
    skos:inScheme hyf: ;
    skos:topConceptOf hyf: .

hyf:HY_Reservoir a skos:Concept ;
    skos:definition """The HY_Reservoir feature type describes the water body, either natural or man-made, used for storage, regulation and control of water resources. The reservoir concept refers to a volume of water managed in zones between operating levels.

HY_Reservoir associates to a reservoir the storedWaterBody and a reservoirZone."""@en ;
    skos:inScheme hyf: ;
    skos:topConceptOf hyf: .

hyf:HY_River a skos:Concept ;
    skos:broader hyf:HY_WaterBody ;
    skos:definition "The HY_River feature type defines the existence of body of surface water, participating in a hydrographic network, special due to its property to permanently or temporarily flow."@en ;
    skos:inScheme hyf: ;
    skos:prefLabel "HY_Stream"@en .

hyf:HY_WaterBodyStratum a skos:Concept ;
    skos:definition """The HY_WaterBodyStratum feature type describes a horizontal layer in a stratified waterbody determined by differences in thermal or salinity characteristics or by oxygen or nutrient content, or by virtual storage zones of a reservoir.

HY_WaterBodyStratum carries the properties: stratumType and benchmark."""@en ;
    skos:inScheme hyf: ;
    skos:topConceptOf hyf: .

hyf:HY_Water_LiquidPhase a skos:Concept ;
    skos:definition """The HY_Water_LiquidPhase feature type provides a simple concept of the accumulation of water in waterbodies. This definition refers to the matter accumulated to a mass of water. In its liquid form water is considered accumulated in waterbodies. The accumulation of water in the atmosphere or below the land surface, e.g. rain, soil moisture or groundwater, is not in scope of this standard, as well as the accumulation of snow and ice in glaciers which is subject of glaciology science.

Contextually related information models may use the HY_Water_LiquidPhase feature type to build relationships to an accumulating waterbody, and ultimately to the catchment realized either by the waterbody or by the network of which the waterbody is part.

HY_Water_LiquidPhase has an association with the accumulatingWaterBody which may be used to identify the waterbody (as part of the hydrographic network) where liquid water is accumulated."""@en ;
    skos:inScheme hyf: ;
    skos:topConceptOf hyf: .

hyf:HY_Water_SolidPhase a skos:Concept ;
    skos:definition """The HY_Water_SolidPhase feature type provides a simple concept of the accumulation of water in waterbodies. This definition refers to the matter accumulated to a mass of water. In its solid form water is considered accumulated in water bodies after melting, or as a layer of ice or snow on an open waterbody. The accumulation of water in the atmosphere or below the land surface, e.g. rain, soil moisture or groundwater, is not in scope of this standard, as well as the accumulation of snow and ice in glaciers which is subject of glaciology science.

Contextually related information models may use the HY_Water_LiquidPhase and HY_Water_SolidPhase feature types to build relationships to an accumulating waterbody, and ultimately to the catchment realized either by the waterbody or by the network of which the waterbody is part.

HY_Water_LiquidPhase has an association with the accumulatingWaterBody; HY_Water_SolidPhase has associations with the water from snowmelt and coveredWaterBody. These associations may be used to identify the waterbody (as part of the hydrographic network) where liquid water is accumulated."""@en ;
    skos:inScheme hyf: ;
    skos:topConceptOf hyf: .

hyf:accumulatingWaterBody a skos:Concept ;
    skos:definition "water body (stratum) wherein liquid water is accumulated."@en ;
    skos:inScheme hyf: ;
    skos:topConceptOf hyf: .

hyf:bedProfileLongitudinal a skos:Concept ;
    skos:definition "identifies a longitudinal vertical shape of a channel, carrying a permanent reference location which realizes the hydro nexus of the catchment which is realized by the channel."@en ;
    skos:inScheme hyf: ;
    skos:topConceptOf hyf: .

hyf:bedProfileTransversal a skos:Concept ;
    skos:definition "identifies a transversal vertical shape of a channel, carrying a permanent reference location which realizes the hydro nexus of the catchment which is realized by the channel."@en ;
    skos:inScheme hyf: ;
    skos:topConceptOf hyf: .

hyf:catchmentArea a skos:Concept ;
    skos:definition "catchment area that participates in the network."@en ;
    skos:inScheme hyf: ;
    skos:topConceptOf hyf: .

hyf:catchmentDivide a skos:Concept ;
    skos:definition "catchment boundary that participates in the network."@en ;
    skos:inScheme hyf: ;
    skos:topConceptOf hyf: .

hyf:catchmentRealization a skos:Concept ;
    skos:definition "topological or geographic feature which realizes the logical catchment."@en ;
    skos:inScheme hyf: ;
    skos:topConceptOf hyf: .

hyf:confinedWaterBody a skos:Concept ;
    skos:definition "identifies a stratum of waterbody contained in the depression."@en ;
    skos:inScheme hyf: ;
    skos:topConceptOf hyf: .

hyf:conjointCatchment a skos:Concept ;
    skos:definition "catchment that interacts with the catchment across an internal boundary line."@en ;
    skos:inScheme hyf: ;
    skos:topConceptOf hyf: .

hyf:containedCatchment a skos:Concept ;
    skos:definition "catchment nested in a containing catchment."@en ;
    skos:inScheme hyf: ;
    skos:topConceptOf hyf: .

hyf:containingCatchment a skos:Concept ;
    skos:definition "catchment nesting contained catchments."@en ;
    skos:inScheme hyf: ;
    skos:topConceptOf hyf: .

hyf:contributingCatchment a skos:Concept ;
    skos:definition "identifies the catchment that contributes flow to this hydro nexus. This allows connection of a catchment's outflow to an identified inflow and to determine its position through referencing the inflow."@en ;
    skos:inScheme hyf: ;
    skos:topConceptOf hyf: .

hyf:coveredWaterBody a skos:Concept ;
    skos:definition "body of open water covered by a layer of ice or snow."@en ;
    skos:inScheme hyf: ;
    skos:topConceptOf hyf: .

hyf:downstreamWaterBody a skos:Concept ;
    skos:definition "identifies another waterbody immediately downstream, allowing network navigation without knowing an inflow or outflow of the catchment realized by the waterbody."@en ;
    skos:inScheme hyf: ;
    skos:topConceptOf hyf: .

hyf:endorheicDrainage a skos:Concept ;
    skos:definition "should be used to identify an endorheic-drained catchment, which is not, but may be temporarily connected to the enveloping catchment."@en ;
    skos:inScheme hyf: ;
    skos:topConceptOf hyf: .

hyf:exorheicDrainage a skos:Concept ;
    skos:definition "should be used to identify an exorheic-drained catchment which is permanently connected to the encompassing catchment."@en ;
    skos:inScheme hyf: ;
    skos:topConceptOf hyf: .

hyf:flowpath a skos:Concept ;
    skos:definition "flowpath that participates in the network."@en ;
    skos:inScheme hyf: ;
    skos:topConceptOf hyf: .

hyf:inflow a skos:Concept ;
    skos:definition "hydro nexus in terms of an inflow to the receiving catchment. For a dendritic network of catchments, the outflow of a contributing catchment coincides with the inflow to a receiving catchment. This supports description of upstream-downstream relationships between catchments."@en ;
    skos:inScheme hyf: ;
    skos:topConceptOf hyf: .

hyf:linearElement a skos:Concept ;
    skos:definition "identifies a flowpath used as the linear element along which a position is assigned to a hydro-location, or any feature of interest."@en ;
    skos:inScheme hyf: ;
    skos:topConceptOf hyf: .

hyf:locatedReferent a skos:Concept ;
    skos:definition "identifies an already referenced location such as a catchment outlet relative to which a position may be assigned to a feature of interest."@en ;
    skos:inScheme hyf: ;
    skos:topConceptOf hyf: .

hyf:lowerCatchment a skos:Concept ;
    skos:definition "catchment located immediately below of the catchment,"@en ;
    skos:inScheme hyf: ;
    skos:topConceptOf hyf: .

hyf:name a skos:Concept ;
    skos:definition "name given to the hydrologic feature in cultural, political or historical context."@en ;
    skos:inScheme hyf: ;
    skos:topConceptOf hyf: .

hyf:networkStation a skos:Concept ;
    skos:definition "hydrometric feature which realizes the catchment either separately, or as part of the hydrometric network."@en ;
    skos:inScheme hyf: ;
    skos:topConceptOf hyf: .

hyf:networkWaterBody a skos:Concept ;
    skos:definition "waterbody which realizes the catchment either separately, or as part of the hydrographic network."@en ;
    skos:inScheme hyf: ;
    skos:topConceptOf hyf: .

hyf:nexusRealization a skos:Concept ;
    skos:definition "identifies a hydrologic feature which realizes the hydro nexus. A topological nexus realization is of lower dimension than the realization of the corresponding catchment. Example: an outflow node realizing the nexus would be of lower dimension than the flowpath edge realizing the contributing catchment."@en ;
    skos:inScheme hyf: ;
    skos:topConceptOf hyf: .

hyf:outflow a skos:Concept ;
    skos:definition "hydro nexus in terms of an outflow of the contributing catchment. For a dendritic network of catchments, the outflow of a contributing catchment coincides with the inflow to a receiving catchment. This supports description of upstream-downstream relationships between catchments."@en ;
    skos:inScheme hyf: ;
    skos:topConceptOf hyf: .

hyf:realizedCatchment a skos:Concept ;
    skos:definition "identifies the one and only one catchment that is realized by a particular feature. Referencing the hydrologic complex containing the catchment and all of its realizations, supports a catchment's existence to be recognized and linked to multiple realizations without the complexity and full detail of a scientific model. By referencing the catchment topology, topological relationships can be established and common identifiers assigned."@en ;
    skos:inScheme hyf: ;
    skos:topConceptOf hyf: .

hyf:realizedNexus a skos:Concept ;
    skos:definition "identifies the one and only one nexus that is realized by a particular feature. Referencing the hydrologic complex containing the hydro nexus and all of its realizations, supports an arbitrary feature of interest to be recognized as outlet of a catchment, and to be placed using the river referencing defined in this standard."@en ;
    skos:inScheme hyf: ;
    skos:topConceptOf hyf: .

hyf:receivingCatchment a skos:Concept ;
    skos:definition "identifies the catchment that receives flow from this hydro nexus. This allows connection of a catchment's inflow to an identified outflow and to determine its position through referencing the outflow."@en ;
    skos:inScheme hyf: ;
    skos:topConceptOf hyf: .

hyf:referenceLocation a skos:Concept ;
    skos:definition "identifies the permanent reference location, usually an existing inflow or outflow hydro nexus relative to which a position is assigned to a hydro location feature of interest."@en ;
    skos:inScheme hyf: ;
    skos:topConceptOf hyf: .

hyf:referencedPosition a skos:Concept ;
    skos:definition "position expressed as measured or otherwise described distance from a known, already located referent. Commonly, this is used to locate a feature of interest such as a hydrometric station in relation to a catchment's outlet fixed by co-ordinates."@en ;
    skos:inScheme hyf: ;
    skos:topConceptOf hyf: .

hyf:reservoirZone a skos:Concept ;
    skos:definition "identifies the waterbody stratum used for storage, for example a management zone, or flood control zone."@en ;
    skos:inScheme hyf: ;
    skos:topConceptOf hyf: .

hyf:snowmelt a skos:Concept ;
    skos:definition "liquid water from melting of snow."@en ;
    skos:inScheme hyf: ;
    skos:topConceptOf hyf: .

hyf:standingWater a skos:Concept ;
    skos:definition "identifies the body of stagnant water contained in the depression."@en ;
    skos:inScheme hyf: ;
    skos:topConceptOf hyf: .

hyf:storage a skos:Concept ;
    skos:definition "identifies a reservoir storing water as a resource for future use. This may be used to describe storage characteristics of the water body participating in the hydrographic network."@en ;
    skos:inScheme hyf: ;
    skos:topConceptOf hyf: .

hyf:storedWaterBody a skos:Concept ;
    skos:definition "identifies the network waterbody that specifies the connectivity of the storage reservoir in the hydrographic network."@en ;
    skos:inScheme hyf: ;
    skos:topConceptOf hyf: .

hyf:stratum a skos:Concept ;
    skos:definition "identifies a horizontal layer of consistent characteristics, or a storage zone of a reservoir."@en ;
    skos:inScheme hyf: ;
    skos:topConceptOf hyf: .

hyf:stream a skos:Concept ;
    skos:definition "identifies the waterbody periodically or continuously flowing in the channel, including subterranean streams."@en ;
    skos:inScheme hyf: ;
    skos:topConceptOf hyf: .

hyf:streamCrossSection a skos:Concept ;
    skos:definition "identifies a vertical section at right angles to the main (average) direction of flow."@en ;
    skos:inScheme hyf: ;
    skos:topConceptOf hyf: .

hyf:streamLongitudinalSection a skos:Concept ;
    skos:definition "identifies a vertical section or along a centerline."@en ;
    skos:inScheme hyf: ;
    skos:topConceptOf hyf: .

hyf:surfaceChannel a skos:Concept ;
    skos:definition "channel on the land surface which realizes the catchment either separately, or as part of the channel network."@en ;
    skos:inScheme hyf: ;
    skos:topConceptOf hyf: .

hyf:surfaceDepression a skos:Concept ;
    skos:definition "depression on the land surface which realizes the catchment either separately, or as part of the channel network."@en ;
    skos:inScheme hyf: ;
    skos:topConceptOf hyf: .

hyf:upperCatchment a skos:Concept ;
    skos:definition "catchment located immediately above of the catchment,"@en ;
    skos:inScheme hyf: ;
    skos:topConceptOf hyf: .

hyf:upstreamWaterBody a skos:Concept ;
    skos:definition "identifies another waterbody immediately upstream, allowing network navigation without knowing an inflow or outflow of the catchment realized by the waterbody."@en ;
    skos:inScheme hyf: ;
    skos:topConceptOf hyf: .

hyf:watercourse a skos:Concept ;
    skos:definition "identifies the natural or man-made channel which continuously or periodically contains moving water, including large interstices in the ground, such as cave, cavern or a group of these."@en ;
    skos:inScheme hyf: ;
    skos:topConceptOf hyf: .

hyf:waterpool a skos:Concept ;
    skos:definition "identifies the natural or artificial depression which contains standing water, including large interstices in the ground, such as cave, cavern or a group of these."@en ;
    skos:inScheme hyf: ;
    skos:topConceptOf hyf: .

hyf:HY_Depression a skos:Concept ;
    skos:definition """The HY_Depression feature type specializes the general HY_HydroFeature class. It describes land lower than the surrounding land as a container for standing water. A depression is part of the network of channels and depressions forming the connecting system in which waterbodies are contained as parts of hydrographic network.

Through generalization, HY_Depression inherits the name property. It has associations for the surfaceNetwork in which it participates, a body of standingWater and a stratum of a confinedWaterBody. An outlet-at-benchmark constraint emphasizes that a benchmark on the confined waterbody at the outlet of the catchment that is realized by the channel network."""@en ;
    skos:inScheme hyf: ;
    skos:narrower hyf:HY_Channel ;
    skos:topConceptOf hyf: .

hyf:HY_HydroFeature a skos:Concept ;
    skos:definition "basic feature to reflect the properties that all hydrologic features have."@en ;
    skos:inScheme hyf: ;
    skos:narrower hyf:HY_Catchment ;
    skos:topConceptOf hyf: .

hyf:HY_Catchment a skos:Concept ;
    skos:broader hyf:HY_HydroFeature ;
    skos:definition """The Catchment model conceptualizes the hydrologic determination of a catchment through inflow and outflow hydro nexus features with the role of getting flow from a contributing catchment, or providing inflow to a receiving catchment (Figure 25 and Figure 26). Conceptually, each catchment has an outflow hydro nexus, and any hydro nexus has a corresponding catchment, even if catchment and/or hydro nexus may not be present in a particular application. A catchment interacts with upper and lower catchments via associated hydro nexuses, and ultimately contributes flow to the hydro nexus of a containing catchment. The catchment should be understood as the logical link between two hydro nexuses.

The HY_Catchment feature type captures the union of catchment and hydro nexus, and the multiple realizations of the holistic catchment concept. These realizations include both topological realizations, as well as their geometric representation. HY_Catchment may be further specialized with respect to catchment interaction.

The HY_Catchment feature type (Figure 26) specializes the general HY_HydroFeature type. Through generalization, HY_Catchment inherits the name property. It carries a code attribute and the associations: outflow, inflow, containingCatchment, containedCatchment, conjointCatchment, upperCatchment, lowerCatchment, catchmentRealization."""@en ;
    skos:inScheme hyf: ;
    skos:narrower hyf:HY_CatchmentAggregate,
        hyf:HY_DendriticCatchment,
        hyf:HY_InteriorCatchment .

hyf:HY_CatchmentRealization a skos:Concept ;
    skos:definition """The HY_CatchmentRealization feature type (Figure 34) is based on the idea that there are multiple hydrology-specific perspectives of the holistic catchment concept that are used to describe a catchment as a unit of study shared across sub-domains and studies.

A given catchment realization exists within a hydrologic complex in that, if a catchment realization exists, it exists in the same hydrologic complex as the catchment it realizes. In this way, any realization of a catchment has the same hydrologic determination of the catchment it realizes. If a catchment is connected with other catchments via inflow and/or outflow hydro nexuses, its realizations are also connected. A realization of the logical catchment is always of higher topological dimension than the realization of the corresponding hydro nexus topological boundary. For example, a linear flowpath realizing a catchment may be understood as an edge between inflow and outflow nodes; the areal realization of a catchment as a face bounded by linear inflow and outflow.

The catchment realization features defined in this standard refer to objects on the land surface for the purpose of surface water hydrology. In other contexts, other types of catchment realization may exist. Catchment realizations that do not conform to those defined in this standard, for instance realizations in 3- or 4-dimensional perspectives, may be implemented using the general HY_CatchmentRealization type. HY_CatchmentRealization carries a shape attribute and as a realizedCatchment association."""@en ;
    skos:inScheme hyf: ;
    skos:narrower hyf:HY_CartographicRealization,
        hyf:HY_CatchmentArea,
        hyf:HY_CatchmentDivide,
        hyf:HY_FlowPath,
        hyf:HY_HydroNetwork ;
    skos:topConceptOf hyf: .

hyf:HY_WaterBody a skos:Concept ;
    skos:definition """The HY_WaterBody feature type specializes the general HY_HydroFeature class. A waterbody is part of the hydrographic network and is either standing in a depression or flowing in a channel, which are parts of the channel network. A waterbody may be segmented in vertical sections at right angles to the main (average) direction of flow or along its centerline, and horizontal strata. Conceptually, each waterbody, or a stratum, could be thought of as a reservoir used for storage, regulation or control of water recourses.

Through generalization, HY_WaterBody inherits the name property. It has associations for the hydrographicNetwork in which it participates, the containing waterpool and watercourse, the vertical streamCrossSection, streamLongitudinalSection, a horizontal stratum, and a reservoir for storage of water. Outlet-at-section and outlet-at-landmark constraints emphasize the recognition of a fixed landmark as outlet of the catchment realized by hydrographic network."""@en ;
    skos:inScheme hyf: ;
    skos:narrower hyf:HY_Canal,
        hyf:HY_Estuary,
        hyf:HY_Impoundment,
        hyf:HY_Lagoon,
        hyf:HY_Lake,
        hyf:HY_River ;
    skos:topConceptOf hyf: .

hyf: a skos:ConceptScheme ;
    skos:definition """The HydroFeature module (Figure 21) provides the core concepts of a named hydrologic feature in the Named Feature, of a hydrologic complex in which the union of catchment and its common outlet is realized in several ways by a collection of hydrologic features, and of a river referencing system which allows placement of an arbitrary feature ‘along a river’ using linear referencing along a one-dimensional topological, flowpath realization.

The HY_HydroFeature feature type is defined as hydrology-specific instance of the General Feature metaclass (as defined in the OGC General Feature Model, GFM), whose identity needs to be maintained and tracked through a processing chain from measurement to distribution of hydrologic information.
As an instance of the General Feature metaclass a feature type is identified by a unique identifier and typical properties. Typically, a hydrologic feature is additionally identified through names in common usage and through hydrologically significant characteristics.

The HY_HydroFeature feature type is specialized into more specific feature types (Figure 23), which specify additional properties and represent particular hydrologic phenomena.Providing a standard terminology for the typical relationships between hydrologic features allows the hydrosphere to be expressed in a consistent way across multiple data products, regardless of various spatial or temporal representations.

The definitions of HydroFeature feature types are rooted in the definitions documented in the WMO/UNESCO Glossary of Hydrology. They are applied regardless of their application context in respect to the Earth's surface. For the purpose of testing the applicability of the HY_Features conceptual model in the context of surface water hydrology, the definitions in this standard refer to surface water hydrology. A conceptual model capturing the specifics of features associated with the groundwater domain is developed with reference to the OGC WaterML 2: Part 4 – GroundwaterML2 standard."""@en,
        """The Hydrometric Network application schema (Figure 45) defines a logical model to take into account a network of hydrometric stations as a specific realization of the catchment in the perspective of hydrologic observation, without the detail of an observation strategy.

The Hydrometric Network model specifies the concepts defined in the Hydro Feature core model.. The general concept is that of a network of logically connected hydrometric stations realizing as a whole the catchment. This enables contextually related information models to relate monitoring stations and observing posts to hydrologic features, as is often required for environmental reporting or when interpreting, analyzing and processing observation results."""@en,
        """The Surface Hydro Feature application schema provides common concepts of hydrologic features occurring on the land surface and specifies the core concepts defined in the abstract Hydro Feature application schema. This will enable contextually linked information models to build relationships between multiple realizations of the same catchments. Typical realizations of the catchment concept and hydro nexuses can be described in a consistent way using standard terminology for the relationships between surface water features defined in this application schema.

The Surface Hydro Feature model (Figure 37) conceptualizes the accumulation of water on the land surface in waterbodies, each made unique by its origin, size, or movement. With respect to the management and storage of water resources, a concept of water storage is provided and allows any waterbody type to be considered a managed reservoir.

Relying on a conceptual separation of waterbody and container, the Surface Hydro Feature schema defines a network of potentially connected depressions and channels on the land surface which periodically or continuously contain water. Separate from the hydrographic network of permanent or temporary waterbodies, the channel network can be used as the connecting system.

The definitions in this schema are rooted in the definitions given in the WMO/UNESCO Glossary of Hydrology which defines a network of watercourse regardless of the location in respect to the Earth's surface. The conceptual model defined here has been vetted in the context of surface water hydrology. In other words, in this standard, 'channel network' and 'hydrographic network' refer to surface channels or other containers for surface-waterbodies.

The Surface Hydro Feature application schema contains the leaf packages: Channel Network, Hydrographic Network, Water Body Types and Storage."""@en ;
    skos:hasTopConcept hyf:HY_CatchmentRealization,
        hyf:HY_ChannelNetwork,
        hyf:HY_CrossSection,
        hyf:HY_Depression,
        hyf:HY_HydroFeature,
        hyf:HY_HydroFeatureName,
        hyf:HY_HydroLocation,
        hyf:HY_HydroNexus,
        hyf:HY_HydrographicNetwork,
        hyf:HY_HydrometricFeature,
        hyf:HY_HydrometricNetwork,
        hyf:HY_IndirectPosition,
        hyf:HY_LongitudinalSection,
        hyf:HY_Reservoir,
        hyf:HY_WaterBody,
        hyf:HY_WaterBodyStratum,
        hyf:HY_Water_LiquidPhase,
        hyf:HY_Water_SolidPhase,
        hyf:accumulatingWaterBody,
        hyf:bedProfileLongitudinal,
        hyf:bedProfileTransversal,
        hyf:catchmentArea,
        hyf:catchmentDivide,
        hyf:catchmentRealization,
        hyf:confinedWaterBody,
        hyf:conjointCatchment,
        hyf:containedCatchment,
        hyf:containingCatchment,
        hyf:contributingCatchment,
        hyf:coveredWaterBody,
        hyf:downstreamWaterBody,
        hyf:endorheicDrainage,
        hyf:exorheicDrainage,
        hyf:flowpath,
        hyf:inflow,
        hyf:linearElement,
        hyf:locatedReferent,
        hyf:lowerCatchment,
        hyf:name,
        hyf:networkStation,
        hyf:networkWaterBody,
        hyf:nexusRealization,
        hyf:outflow,
        hyf:realizedCatchment,
        hyf:realizedNexus,
        hyf:receivingCatchment,
        hyf:referenceLocation,
        hyf:referencedPosition,
        hyf:reservoirZone,
        hyf:snowmelt,
        hyf:standingWater,
        hyf:storage,
        hyf:storedWaterBody,
        hyf:stratum,
        hyf:stream,
        hyf:streamCrossSection,
        hyf:streamLongitudinalSection,
        hyf:surfaceChannel,
        hyf:surfaceDepression,
        hyf:upperCatchment,
        hyf:upstreamWaterBody,
        hyf:watercourse,
        hyf:waterpool .

