<?xml version="1.0" encoding="utf-8"?>
<rdf:RDF
   xmlns:dc="http://purl.org/dc/elements/1.1/"
   xmlns:dcterms="http://purl.org/dc/terms/"
   xmlns:ns1="http://www.opengis.net/def/metamodel/ogc-na/"
   xmlns:owl="http://www.w3.org/2002/07/owl#"
   xmlns:rdf="http://www.w3.org/1999/02/22-rdf-syntax-ns#"
   xmlns:rdfs="http://www.w3.org/2000/01/rdf-schema#"
   xmlns:skos="http://www.w3.org/2004/02/skos/core#"
>
  <rdf:Description rdf:about="https://www.opengis.net/def/security/1.0/codelist/authentication/SAML2_PublicKeyPGP">
    <rdf:type rdf:resource="http://www.w3.org/2004/02/skos/core#Concept"/>
    <rdfs:seeAlso rdf:resource="https://www.opengis.net/def/security/1.0/codelist/authentication/SAML2_PublicKeyPGP?_view=alternates"/>
    <rdfs:seeAlso rdf:resource="http://schemas.opengis.net/security/1.0/codelist/authentication.xml"/>
    <skos:notation rdf:datatype="http://www.opengis.net/def/metamodel/URN">urn:oasis:names:tc:SAML:2.0:ac:classes:PGP</skos:notation>
    <skos:prefLabel xml:lang="en">SAML2_PublicKeyPGP</skos:prefLabel>
    <skos:definition>As specified in https://docs.oasis-open.org/security/saml/v2.0/saml-authn-context-2.0-os.pdf</skos:definition>
    <skos:inScheme rdf:resource="https://www.opengis.net/def/security/1.0/codelist/authentication"/>
    <ns1:status rdf:resource="http://www.opengis.net/def/status/valid"/>
  </rdf:Description>
  <rdf:Description rdf:about="https://www.opengis.net/def/security/1.0/codelist/authentication">
    <ns1:equivalentCollection rdf:resource="https://www.opengis.net/def/security/1.0/codelist/authentication/"/>
    <rdf:type rdf:resource="http://rdfs.org/ns/void#Dataset"/>
    <rdf:type rdf:resource="http://www.w3.org/2004/02/skos/core#ConceptScheme"/>
    <rdfs:seeAlso rdf:resource="http://schemas.opengis.net/security/1.0/codelist/authentication.xml"/>
    <skos:prefLabel xml:lang="en">Authentication</skos:prefLabel>
    <skos:definition>identification of authentication methods</skos:definition>
    <skos:notation rdf:datatype="http://www.opengis.net/def/metamodel/URN">urn:ogc:def:security:authentication</skos:notation>
    <ns1:collectionView rdf:resource="https://www.opengis.net/def/security/1.0/codelist/authentication/"/>
    <dcterms:source rdf:resource="http://www.opengis.net/def/entities/bodies/ogcna"/>
  </rdf:Description>
  <rdf:Description rdf:about="https://www.opengis.net/def/security/1.0/codelist/authentication/SAML2_Kerberos">
    <rdf:type rdf:resource="http://www.w3.org/2004/02/skos/core#Concept"/>
    <rdfs:seeAlso rdf:resource="https://www.opengis.net/def/security/1.0/codelist/authentication/SAML2_Kerberos?_view=alternates"/>
    <rdfs:seeAlso rdf:resource="http://schemas.opengis.net/security/1.0/codelist/authentication.xml"/>
    <skos:notation rdf:datatype="http://www.opengis.net/def/metamodel/URN">urn:oasis:names:tc:SAML:2.0:ac:classes:Kerberos</skos:notation>
    <skos:prefLabel xml:lang="en">SAML2_Kerberos</skos:prefLabel>
    <skos:definition>As specified in https://docs.oasis-open.org/security/saml/v2.0/saml-authn-context-2.0-os.pdf</skos:definition>
    <skos:inScheme rdf:resource="https://www.opengis.net/def/security/1.0/codelist/authentication"/>
    <ns1:status rdf:resource="http://www.opengis.net/def/status/valid"/>
  </rdf:Description>
  <rdf:Description rdf:about="https://www.opengis.net/def/security/1.0/codelist/authentication/SAML2_MobileOneFactorUnregistered">
    <skos:inScheme rdf:resource="https://www.opengis.net/def/security/1.0/codelist/authentication"/>
    <rdf:type rdf:resource="http://www.w3.org/2004/02/skos/core#Concept"/>
    <rdfs:seeAlso rdf:resource="https://www.opengis.net/def/security/1.0/codelist/authentication/SAML2_MobileOneFactorUnregistered?_view=alternates"/>
    <rdfs:seeAlso rdf:resource="http://schemas.opengis.net/security/1.0/codelist/authentication.xml"/>
    <skos:notation rdf:datatype="http://www.opengis.net/def/metamodel/URN">urn:oasis:names:tc:SAML:2.0:ac:classes:MobileOneFactorUnregistered</skos:notation>
    <skos:prefLabel xml:lang="en">SAML2_MobileOneFactorUnregistered</skos:prefLabel>
    <skos:definition>As specified in https://docs.oasis-open.org/security/saml/v2.0/saml-authn-context-2.0-os.pdf</skos:definition>
    <ns1:status rdf:resource="http://www.opengis.net/def/status/valid"/>
  </rdf:Description>
  <rdf:Description rdf:about="https://www.opengis.net/def/security/1.0/codelist/authentication/SAML2_PublicKeyX509">
    <skos:inScheme rdf:resource="https://www.opengis.net/def/security/1.0/codelist/authentication"/>
    <rdf:type rdf:resource="http://www.w3.org/2004/02/skos/core#Concept"/>
    <rdfs:seeAlso rdf:resource="https://www.opengis.net/def/security/1.0/codelist/authentication/SAML2_PublicKeyX509?_view=alternates"/>
    <rdfs:seeAlso rdf:resource="http://schemas.opengis.net/security/1.0/codelist/authentication.xml"/>
    <skos:notation rdf:datatype="http://www.opengis.net/def/metamodel/URN">urn:oasis:names:tc:SAML:2.0:ac:classes:X509</skos:notation>
    <skos:prefLabel xml:lang="en">SAML2_PublicKeyX509</skos:prefLabel>
    <skos:definition>As specified in https://docs.oasis-open.org/security/saml/v2.0/saml-authn-context-2.0-os.pdf</skos:definition>
    <ns1:status rdf:resource="http://www.opengis.net/def/status/valid"/>
  </rdf:Description>
  <rdf:Description rdf:about="https://www.opengis.net/def/security/1.0/codelist/authentication/SAML2_SoftwarePKI">
    <skos:inScheme rdf:resource="https://www.opengis.net/def/security/1.0/codelist/authentication"/>
    <rdf:type rdf:resource="http://www.w3.org/2004/02/skos/core#Concept"/>
    <rdfs:seeAlso rdf:resource="https://www.opengis.net/def/security/1.0/codelist/authentication/SAML2_SoftwarePKI?_view=alternates"/>
    <rdfs:seeAlso rdf:resource="http://schemas.opengis.net/security/1.0/codelist/authentication.xml"/>
    <skos:notation rdf:datatype="http://www.opengis.net/def/metamodel/URN">urn:oasis:names:tc:SAML:2.0:ac:classes:SoftwarePKI</skos:notation>
    <skos:prefLabel xml:lang="en">SAML2_SoftwarePKI</skos:prefLabel>
    <skos:definition>As specified in https://docs.oasis-open.org/security/saml/v2.0/saml-authn-context-2.0-os.pdf</skos:definition>
    <ns1:status rdf:resource="http://www.opengis.net/def/status/valid"/>
  </rdf:Description>
  <rdf:Description rdf:about="https://www.opengis.net/def/security/1.0/codelist/authentication/TLS_CLIENT_CERTIFICATE">
    <skos:inScheme rdf:resource="https://www.opengis.net/def/security/1.0/codelist/authentication"/>
    <rdf:type rdf:resource="http://www.w3.org/2004/02/skos/core#Concept"/>
    <rdfs:seeAlso rdf:resource="https://www.opengis.net/def/security/1.0/codelist/authentication/TLS_CLIENT_CERTIFICATE?_view=alternates"/>
    <rdfs:seeAlso rdf:resource="http://schemas.opengis.net/security/1.0/codelist/authentication.xml"/>
    <skos:notation rdf:datatype="http://www.opengis.net/def/metamodel/URN">urn:ogc:def:security:authentication:ietf:5246:client_certificate</skos:notation>
    <skos:prefLabel xml:lang="en">TLS_CLIENT_CERTIFICATE</skos:prefLabel>
    <skos:definition>This type of authentication is an extension to the TLS handshake as outlined in section 7.4.4: "A non-anonymous server can optionally request a certificate from the client, if appropriate for the selected cipher suite.  This message, if sent, will immediately follow the ServerKeyExchange message (if it is sent; otherwise, this message follows the serverâ€™s Certificate message)."[RFC 5246]	In case the client cannot provide a suitable and valid certificate, no TLS connection gets established.</skos:definition>
    <ns1:status rdf:resource="http://www.opengis.net/def/status/valid"/>
  </rdf:Description>
  <rdf:Description rdf:about="https://www.opengis.net/def/security/1.0/">
    <rdf:type rdf:resource="http://www.w3.org/2004/02/skos/core#Collection"/>
    <skos:prefLabel>OGC Web Services Security 1.0</skos:prefLabel>
    <dc:source>OGC 17-007</dc:source>
    <skos:member rdf:resource="https://www.opengis.net/def/security/1.0/codelist/authentication"/>
    <dcterms:created rdf:datatype="http://www.w3.org/2001/XMLSchema#date">2019-01-23</dcterms:created>
    <owl:sameAs rdf:resource="https://www.opengis.net/def/security/1.0"/>
    <skos:definition>OGC Web Services Security 1.0</skos:definition>
  </rdf:Description>
  <rdf:Description rdf:about="https://www.opengis.net/def/security/1.0/codelist/authentication/SAML2_AuthenticatedTelephony">
    <rdf:type rdf:resource="http://www.w3.org/2004/02/skos/core#Concept"/>
    <rdfs:seeAlso rdf:resource="https://www.opengis.net/def/security/1.0/codelist/authentication/SAML2_AuthenticatedTelephony?_view=alternates"/>
    <rdfs:seeAlso rdf:resource="http://schemas.opengis.net/security/1.0/codelist/authentication.xml"/>
    <skos:notation rdf:datatype="http://www.opengis.net/def/metamodel/URN">urn:oasis:names:tc:SAML:2.0:ac:classes:AuthenticatedTelephony</skos:notation>
    <skos:prefLabel xml:lang="en">SAML2_AuthenticatedTelephony</skos:prefLabel>
    <skos:definition>As specified in https://docs.oasis-open.org/security/saml/v2.0/saml-authn-context-2.0-os.pdf</skos:definition>
    <skos:inScheme rdf:resource="https://www.opengis.net/def/security/1.0/codelist/authentication"/>
    <ns1:status rdf:resource="http://www.opengis.net/def/status/valid"/>
  </rdf:Description>
  <rdf:Description rdf:about="https://www.opengis.net/def/security/1.0/codelist/authentication/">
    <skos:member rdf:resource="https://www.opengis.net/def/security/1.0/codelist/authentication/HTTP_BASIC"/>
    <skos:member rdf:resource="https://www.opengis.net/def/security/1.0/codelist/authentication/HTTP_DIGEST"/>
    <skos:member rdf:resource="https://www.opengis.net/def/security/1.0/codelist/authentication/OAUTH2_BEARER_TOKEN"/>
    <skos:member rdf:resource="https://www.opengis.net/def/security/1.0/codelist/authentication/SAML2_AuthenticatedTelephony"/>
    <skos:member rdf:resource="https://www.opengis.net/def/security/1.0/codelist/authentication/SAML2_InternetProtocol"/>
    <skos:member rdf:resource="https://www.opengis.net/def/security/1.0/codelist/authentication/SAML2_InternetProtocolPassword"/>
    <skos:member rdf:resource="https://www.opengis.net/def/security/1.0/codelist/authentication/SAML2_Kerberos"/>
    <skos:member rdf:resource="https://www.opengis.net/def/security/1.0/codelist/authentication/SAML2_MobileOneFactorContract"/>
    <skos:member rdf:resource="https://www.opengis.net/def/security/1.0/codelist/authentication/SAML2_MobileOneFactorUnregistered"/>
    <skos:member rdf:resource="https://www.opengis.net/def/security/1.0/codelist/authentication/SAML2_MobileTwoFactorContract"/>
    <skos:member rdf:resource="https://www.opengis.net/def/security/1.0/codelist/authentication/SAML2_MobileTwoFactorUnregistered"/>
    <skos:member rdf:resource="https://www.opengis.net/def/security/1.0/codelist/authentication/SAML2_Password"/>
    <skos:member rdf:resource="https://www.opengis.net/def/security/1.0/codelist/authentication/SAML2_PasswordProtectedTransport"/>
    <skos:member rdf:resource="https://www.opengis.net/def/security/1.0/codelist/authentication/SAML2_PersonalTelephony"/>
    <skos:member rdf:resource="https://www.opengis.net/def/security/1.0/codelist/authentication/SAML2_PreviousSession"/>
    <skos:member rdf:resource="https://www.opengis.net/def/security/1.0/codelist/authentication/SAML2_PublicKeyPGP"/>
    <skos:member rdf:resource="https://www.opengis.net/def/security/1.0/codelist/authentication/SAML2_PublicKeySPKI"/>
    <skos:member rdf:resource="https://www.opengis.net/def/security/1.0/codelist/authentication/SAML2_PublicKeyX509"/>
    <skos:member rdf:resource="https://www.opengis.net/def/security/1.0/codelist/authentication/SAML2_PublicKeyXMLDigitalSignature"/>
    <skos:member rdf:resource="https://www.opengis.net/def/security/1.0/codelist/authentication/SAML2_SecureRemotePassword"/>
    <skos:member rdf:resource="https://www.opengis.net/def/security/1.0/codelist/authentication/SAML2_Smartcard"/>
    <skos:member rdf:resource="https://www.opengis.net/def/security/1.0/codelist/authentication/SAML2_SmartcardPKI"/>
    <skos:member rdf:resource="https://www.opengis.net/def/security/1.0/codelist/authentication/SAML2_SoftwarePKI"/>
    <skos:member rdf:resource="https://www.opengis.net/def/security/1.0/codelist/authentication/SAML2_TLSClient"/>
    <skos:member rdf:resource="https://www.opengis.net/def/security/1.0/codelist/authentication/SAML2_Telephony"/>
    <skos:member rdf:resource="https://www.opengis.net/def/security/1.0/codelist/authentication/SAML2_TelephonyNomadic"/>
    <skos:member rdf:resource="https://www.opengis.net/def/security/1.0/codelist/authentication/SAML2_TimeSyncToken"/>
    <skos:member rdf:resource="https://www.opengis.net/def/security/1.0/codelist/authentication/SAML2_Unspecified"/>
    <skos:member rdf:resource="https://www.opengis.net/def/security/1.0/codelist/authentication/TLS_CLIENT_CERTIFICATE"/>
    <skos:member rdf:resource="https://www.opengis.net/def/security/1.0/codelist/authentication/USERNAME_TOKEN"/>
    <skos:definition>Collection hierarchy for this ConceptScheme</skos:definition>
    <skos:inScheme rdf:resource="https://www.opengis.net/def/security/1.0/codelist/authentication"/>
    <rdf:type rdf:resource="http://www.w3.org/2004/02/skos/core#Collection"/>
    <skos:prefLabel>Concepts in Authentication</skos:prefLabel>
    <dcterms:provenance>Generated by the OGC Definitions Server to support integration of the elements of this ConceptScheme into bigger collections. ogc_skos_profile_entailements.ttl</dcterms:provenance>
  </rdf:Description>
  <rdf:Description rdf:about="https://www.opengis.net/def/security/1.0/codelist/authentication/SAML2_SecureRemotePassword">
    <rdf:type rdf:resource="http://www.w3.org/2004/02/skos/core#Concept"/>
    <rdfs:seeAlso rdf:resource="https://www.opengis.net/def/security/1.0/codelist/authentication/SAML2_SecureRemotePassword?_view=alternates"/>
    <rdfs:seeAlso rdf:resource="http://schemas.opengis.net/security/1.0/codelist/authentication.xml"/>
    <skos:notation rdf:datatype="http://www.opengis.net/def/metamodel/URN">urn:oasis:names:tc:SAML:2.0:ac:classes:SecureRemotePassword</skos:notation>
    <skos:prefLabel xml:lang="en">SAML2_SecureRemotePassword</skos:prefLabel>
    <skos:definition>As specified in https://docs.oasis-open.org/security/saml/v2.0/saml-authn-context-2.0-os.pdf</skos:definition>
    <skos:inScheme rdf:resource="https://www.opengis.net/def/security/1.0/codelist/authentication"/>
    <ns1:status rdf:resource="http://www.opengis.net/def/status/valid"/>
  </rdf:Description>
  <rdf:Description rdf:about="https://www.opengis.net/def/security/1.0/codelist/authentication/SAML2_MobileOneFactorContract">
    <skos:inScheme rdf:resource="https://www.opengis.net/def/security/1.0/codelist/authentication"/>
    <rdf:type rdf:resource="http://www.w3.org/2004/02/skos/core#Concept"/>
    <rdfs:seeAlso rdf:resource="https://www.opengis.net/def/security/1.0/codelist/authentication/SAML2_MobileOneFactorContract?_view=alternates"/>
    <rdfs:seeAlso rdf:resource="http://schemas.opengis.net/security/1.0/codelist/authentication.xml"/>
    <skos:notation rdf:datatype="http://www.opengis.net/def/metamodel/URN">urn:oasis:names:tc:SAML:2.0:ac:classes:MobileOneFactorContract</skos:notation>
    <skos:prefLabel xml:lang="en">SAML2_MobileOneFactorContract</skos:prefLabel>
    <skos:definition>As specified in https://docs.oasis-open.org/security/saml/v2.0/saml-authn-context-2.0-os.pdf</skos:definition>
    <ns1:status rdf:resource="http://www.opengis.net/def/status/valid"/>
  </rdf:Description>
  <rdf:Description rdf:about="https://www.opengis.net/def/security/1.0/codelist/authentication/SAML2_Telephony">
    <skos:inScheme rdf:resource="https://www.opengis.net/def/security/1.0/codelist/authentication"/>
    <rdf:type rdf:resource="http://www.w3.org/2004/02/skos/core#Concept"/>
    <rdfs:seeAlso rdf:resource="https://www.opengis.net/def/security/1.0/codelist/authentication/SAML2_Telephony?_view=alternates"/>
    <rdfs:seeAlso rdf:resource="http://schemas.opengis.net/security/1.0/codelist/authentication.xml"/>
    <skos:notation rdf:datatype="http://www.opengis.net/def/metamodel/URN">urn:oasis:names:tc:SAML:2.0:ac:classes:Telephony</skos:notation>
    <skos:prefLabel xml:lang="en">SAML2_Telephony</skos:prefLabel>
    <skos:definition>As specified in https://docs.oasis-open.org/security/saml/v2.0/saml-authn-context-2.0-os.pdf</skos:definition>
    <ns1:status rdf:resource="http://www.opengis.net/def/status/valid"/>
  </rdf:Description>
  <rdf:Description rdf:about="https://www.opengis.net/def/security/1.0/codelist/authentication/SAML2_MobileTwoFactorUnregistered">
    <skos:inScheme rdf:resource="https://www.opengis.net/def/security/1.0/codelist/authentication"/>
    <rdf:type rdf:resource="http://www.w3.org/2004/02/skos/core#Concept"/>
    <rdfs:seeAlso rdf:resource="https://www.opengis.net/def/security/1.0/codelist/authentication/SAML2_MobileTwoFactorUnregistered?_view=alternates"/>
    <rdfs:seeAlso rdf:resource="http://schemas.opengis.net/security/1.0/codelist/authentication.xml"/>
    <skos:notation rdf:datatype="http://www.opengis.net/def/metamodel/URN">urn:oasis:names:tc:SAML:2.0:ac:classes:MobileTwoFactorUnregistered</skos:notation>
    <skos:prefLabel xml:lang="en">SAML2_MobileTwoFactorUnregistered</skos:prefLabel>
    <skos:definition>As specified in https://docs.oasis-open.org/security/saml/v2.0/saml-authn-context-2.0-os.pdf</skos:definition>
    <ns1:status rdf:resource="http://www.opengis.net/def/status/valid"/>
  </rdf:Description>
  <rdf:Description rdf:about="https://www.opengis.net/def/security/1.0/codelist/authentication/OAUTH2_BEARER_TOKEN">
    <skos:inScheme rdf:resource="https://www.opengis.net/def/security/1.0/codelist/authentication"/>
    <rdf:type rdf:resource="http://www.w3.org/2004/02/skos/core#Concept"/>
    <rdfs:seeAlso rdf:resource="https://www.opengis.net/def/security/1.0/codelist/authentication/OAUTH2_BEARER_TOKEN?_view=alternates"/>
    <rdfs:seeAlso rdf:resource="http://schemas.opengis.net/security/1.0/codelist/authentication.xml"/>
    <skos:notation rdf:datatype="http://www.opengis.net/def/metamodel/URN">urn:ogc:def:security:authentication:ietf:6750:Bearer</skos:notation>
    <skos:prefLabel xml:lang="en">OAUTH2_BEARER_TOKEN</skos:prefLabel>
    <skos:definition>
           In the scenario supported by the OAuth 2.0 SSO profile, a web user or service either accesses a resource
            at a service provider, or accesses an identity provider such that the service provider and desired resource are understood
            or implicit. The web user authenticates (or has already authenticated) to the identity provider, Which then produces an
            authorization grant which was then used by an authorization service to return an access token.  This access token then
            subtitutes as both authentication and authorization on future requests.</skos:definition>
    <ns1:status rdf:resource="http://www.opengis.net/def/status/valid"/>
  </rdf:Description>
  <rdf:Description rdf:about="https://www.opengis.net/def/security/1.0/codelist/authentication/SAML2_MobileTwoFactorContract">
    <rdf:type rdf:resource="http://www.w3.org/2004/02/skos/core#Concept"/>
    <rdfs:seeAlso rdf:resource="https://www.opengis.net/def/security/1.0/codelist/authentication/SAML2_MobileTwoFactorContract?_view=alternates"/>
    <rdfs:seeAlso rdf:resource="http://schemas.opengis.net/security/1.0/codelist/authentication.xml"/>
    <skos:notation rdf:datatype="http://www.opengis.net/def/metamodel/URN">urn:oasis:names:tc:SAML:2.0:ac:classes:MobileTwoFactorContract</skos:notation>
    <skos:prefLabel xml:lang="en">SAML2_MobileTwoFactorContract</skos:prefLabel>
    <skos:definition>As specified in https://docs.oasis-open.org/security/saml/v2.0/saml-authn-context-2.0-os.pdf</skos:definition>
    <skos:inScheme rdf:resource="https://www.opengis.net/def/security/1.0/codelist/authentication"/>
    <ns1:status rdf:resource="http://www.opengis.net/def/status/valid"/>
  </rdf:Description>
  <rdf:Description rdf:about="https://www.opengis.net/def/security/1.0/codelist/authentication/SAML2_PasswordProtectedTransport">
    <rdf:type rdf:resource="http://www.w3.org/2004/02/skos/core#Concept"/>
    <rdfs:seeAlso rdf:resource="https://www.opengis.net/def/security/1.0/codelist/authentication/SAML2_PasswordProtectedTransport?_view=alternates"/>
    <rdfs:seeAlso rdf:resource="http://schemas.opengis.net/security/1.0/codelist/authentication.xml"/>
    <skos:notation rdf:datatype="http://www.opengis.net/def/metamodel/URN">urn:oasis:names:tc:SAML:2.0:ac:classes:PasswordProtectedTransport</skos:notation>
    <skos:prefLabel xml:lang="en">SAML2_PasswordProtectedTransport</skos:prefLabel>
    <skos:definition>As specified in https://docs.oasis-open.org/security/saml/v2.0/saml-authn-context-2.0-os.pdf</skos:definition>
    <skos:inScheme rdf:resource="https://www.opengis.net/def/security/1.0/codelist/authentication"/>
    <ns1:status rdf:resource="http://www.opengis.net/def/status/valid"/>
  </rdf:Description>
  <rdf:Description rdf:about="https://www.opengis.net/def/security/1.0/codelist/authentication/SAML2_PersonalTelephony">
    <rdf:type rdf:resource="http://www.w3.org/2004/02/skos/core#Concept"/>
    <rdfs:seeAlso rdf:resource="https://www.opengis.net/def/security/1.0/codelist/authentication/SAML2_PersonalTelephony?_view=alternates"/>
    <rdfs:seeAlso rdf:resource="http://schemas.opengis.net/security/1.0/codelist/authentication.xml"/>
    <skos:notation rdf:datatype="http://www.opengis.net/def/metamodel/URN">urn:oasis:names:tc:SAML:2.0:ac:classes:PersonalTelephony</skos:notation>
    <skos:prefLabel xml:lang="en">SAML2_PersonalTelephony</skos:prefLabel>
    <skos:definition>As specified in https://docs.oasis-open.org/security/saml/v2.0/saml-authn-context-2.0-os.pdf</skos:definition>
    <skos:inScheme rdf:resource="https://www.opengis.net/def/security/1.0/codelist/authentication"/>
    <ns1:status rdf:resource="http://www.opengis.net/def/status/valid"/>
  </rdf:Description>
  <rdf:Description rdf:about="https://www.opengis.net/def/security/1.0/codelist/authentication/SAML2_Password">
    <skos:inScheme rdf:resource="https://www.opengis.net/def/security/1.0/codelist/authentication"/>
    <rdf:type rdf:resource="http://www.w3.org/2004/02/skos/core#Concept"/>
    <rdfs:seeAlso rdf:resource="https://www.opengis.net/def/security/1.0/codelist/authentication/SAML2_Password?_view=alternates"/>
    <rdfs:seeAlso rdf:resource="http://schemas.opengis.net/security/1.0/codelist/authentication.xml"/>
    <skos:notation rdf:datatype="http://www.opengis.net/def/metamodel/URN">urn:oasis:names:tc:SAML:2.0:ac:classes:Password</skos:notation>
    <skos:prefLabel xml:lang="en">SAML2_Password</skos:prefLabel>
    <skos:definition>As specified in https://docs.oasis-open.org/security/saml/v2.0/saml-authn-context-2.0-os.pdf</skos:definition>
    <ns1:status rdf:resource="http://www.opengis.net/def/status/valid"/>
  </rdf:Description>
  <rdf:Description rdf:about="https://www.opengis.net/def/security/1.0/codelist/authentication/SAML2_SmartcardPKI">
    <skos:inScheme rdf:resource="https://www.opengis.net/def/security/1.0/codelist/authentication"/>
    <rdf:type rdf:resource="http://www.w3.org/2004/02/skos/core#Concept"/>
    <rdfs:seeAlso rdf:resource="https://www.opengis.net/def/security/1.0/codelist/authentication/SAML2_SmartcardPKI?_view=alternates"/>
    <rdfs:seeAlso rdf:resource="http://schemas.opengis.net/security/1.0/codelist/authentication.xml"/>
    <skos:notation rdf:datatype="http://www.opengis.net/def/metamodel/URN">urn:oasis:names:tc:SAML:2.0:ac:classes:SmartcardPKI</skos:notation>
    <skos:prefLabel xml:lang="en">SAML2_SmartcardPKI</skos:prefLabel>
    <skos:definition>As specified in https://docs.oasis-open.org/security/saml/v2.0/saml-authn-context-2.0-os.pdf</skos:definition>
    <ns1:status rdf:resource="http://www.opengis.net/def/status/valid"/>
  </rdf:Description>
  <rdf:Description rdf:about="https://www.opengis.net/def/security/1.0/codelist/authentication/SAML2_PublicKeyXMLDigitalSignature">
    <rdf:type rdf:resource="http://www.w3.org/2004/02/skos/core#Concept"/>
    <rdfs:seeAlso rdf:resource="https://www.opengis.net/def/security/1.0/codelist/authentication/SAML2_PublicKeyXMLDigitalSignature?_view=alternates"/>
    <rdfs:seeAlso rdf:resource="http://schemas.opengis.net/security/1.0/codelist/authentication.xml"/>
    <skos:notation rdf:datatype="http://www.opengis.net/def/metamodel/URN">urn:oasis:names:tc:SAML:2.0:ac:classes:XMLDSig</skos:notation>
    <skos:prefLabel xml:lang="en">SAML2_PublicKeyXMLDigitalSignature</skos:prefLabel>
    <skos:definition>As specified in https://docs.oasis-open.org/security/saml/v2.0/saml-authn-context-2.0-os.pdf</skos:definition>
    <skos:inScheme rdf:resource="https://www.opengis.net/def/security/1.0/codelist/authentication"/>
    <ns1:status rdf:resource="http://www.opengis.net/def/status/valid"/>
  </rdf:Description>
  <rdf:Description rdf:about="https://www.opengis.net/def/security/1.0/codelist/authentication/SAML2_TimeSyncToken">
    <rdf:type rdf:resource="http://www.w3.org/2004/02/skos/core#Concept"/>
    <rdfs:seeAlso rdf:resource="https://www.opengis.net/def/security/1.0/codelist/authentication/SAML2_TimeSyncToken?_view=alternates"/>
    <rdfs:seeAlso rdf:resource="http://schemas.opengis.net/security/1.0/codelist/authentication.xml"/>
    <skos:notation rdf:datatype="http://www.opengis.net/def/metamodel/URN">urn:oasis:names:tc:SAML:2.0:ac:classes:TimeSyncToken</skos:notation>
    <skos:prefLabel xml:lang="en">SAML2_TimeSyncToken</skos:prefLabel>
    <skos:definition>As specified in https://docs.oasis-open.org/security/saml/v2.0/saml-authn-context-2.0-os.pdf</skos:definition>
    <skos:inScheme rdf:resource="https://www.opengis.net/def/security/1.0/codelist/authentication"/>
    <ns1:status rdf:resource="http://www.opengis.net/def/status/valid"/>
  </rdf:Description>
  <rdf:Description rdf:about="https://www.opengis.net/def/security/1.0/codelist/authentication/SAML2_InternetProtocolPassword">
    <skos:inScheme rdf:resource="https://www.opengis.net/def/security/1.0/codelist/authentication"/>
    <rdf:type rdf:resource="http://www.w3.org/2004/02/skos/core#Concept"/>
    <rdfs:seeAlso rdf:resource="https://www.opengis.net/def/security/1.0/codelist/authentication/SAML2_InternetProtocolPassword?_view=alternates"/>
    <rdfs:seeAlso rdf:resource="http://schemas.opengis.net/security/1.0/codelist/authentication.xml"/>
    <skos:notation rdf:datatype="http://www.opengis.net/def/metamodel/URN">urn:oasis:names:tc:SAML:2.0:ac:classes:InternetProtocolPassword</skos:notation>
    <skos:prefLabel xml:lang="en">SAML2_InternetProtocolPassword</skos:prefLabel>
    <skos:definition>As specified in https://docs.oasis-open.org/security/saml/v2.0/saml-authn-context-2.0-os.pdf</skos:definition>
    <ns1:status rdf:resource="http://www.opengis.net/def/status/valid"/>
  </rdf:Description>
  <rdf:Description rdf:about="https://www.opengis.net/def/security/1.0/codelist/authentication/SAML2_PreviousSession">
    <rdf:type rdf:resource="http://www.w3.org/2004/02/skos/core#Concept"/>
    <rdfs:seeAlso rdf:resource="https://www.opengis.net/def/security/1.0/codelist/authentication/SAML2_PreviousSession?_view=alternates"/>
    <rdfs:seeAlso rdf:resource="http://schemas.opengis.net/security/1.0/codelist/authentication.xml"/>
    <skos:notation rdf:datatype="http://www.opengis.net/def/metamodel/URN">urn:oasis:names:tc:SAML:2.0:ac:classes:PreviousSession</skos:notation>
    <skos:prefLabel xml:lang="en">SAML2_PreviousSession</skos:prefLabel>
    <skos:definition>As specified in https://docs.oasis-open.org/security/saml/v2.0/saml-authn-context-2.0-os.pdf</skos:definition>
    <skos:inScheme rdf:resource="https://www.opengis.net/def/security/1.0/codelist/authentication"/>
    <ns1:status rdf:resource="http://www.opengis.net/def/status/valid"/>
  </rdf:Description>
  <rdf:Description rdf:about="https://www.opengis.net/def/security/1.0/codelist/authentication/SAML2_InternetProtocol">
    <rdf:type rdf:resource="http://www.w3.org/2004/02/skos/core#Concept"/>
    <rdfs:seeAlso rdf:resource="https://www.opengis.net/def/security/1.0/codelist/authentication/SAML2_InternetProtocol?_view=alternates"/>
    <rdfs:seeAlso rdf:resource="http://schemas.opengis.net/security/1.0/codelist/authentication.xml"/>
    <skos:notation rdf:datatype="http://www.opengis.net/def/metamodel/URN">urn:oasis:names:tc:SAML:2.0:ac:classes:InternetProtocol</skos:notation>
    <skos:prefLabel xml:lang="en">SAML2_InternetProtocol</skos:prefLabel>
    <skos:definition>As specified in https://docs.oasis-open.org/security/saml/v2.0/saml-authn-context-2.0-os.pdf</skos:definition>
    <skos:inScheme rdf:resource="https://www.opengis.net/def/security/1.0/codelist/authentication"/>
    <ns1:status rdf:resource="http://www.opengis.net/def/status/valid"/>
  </rdf:Description>
  <rdf:Description rdf:about="https://www.opengis.net/def/security/1.0/codelist/authentication/SAML2_Smartcard">
    <rdf:type rdf:resource="http://www.w3.org/2004/02/skos/core#Concept"/>
    <rdfs:seeAlso rdf:resource="https://www.opengis.net/def/security/1.0/codelist/authentication/SAML2_Smartcard?_view=alternates"/>
    <rdfs:seeAlso rdf:resource="http://schemas.opengis.net/security/1.0/codelist/authentication.xml"/>
    <skos:notation rdf:datatype="http://www.opengis.net/def/metamodel/URN">urn:oasis:names:tc:SAML:2.0:ac:classes:Smartcard</skos:notation>
    <skos:prefLabel xml:lang="en">SAML2_Smartcard</skos:prefLabel>
    <skos:definition>As specified in https://docs.oasis-open.org/security/saml/v2.0/saml-authn-context-2.0-os.pdf</skos:definition>
    <skos:inScheme rdf:resource="https://www.opengis.net/def/security/1.0/codelist/authentication"/>
    <ns1:status rdf:resource="http://www.opengis.net/def/status/valid"/>
  </rdf:Description>
  <rdf:Description rdf:about="https://www.opengis.net/def/security/1.0/codelist/authentication/SAML2_TLSClient">
    <skos:inScheme rdf:resource="https://www.opengis.net/def/security/1.0/codelist/authentication"/>
    <rdf:type rdf:resource="http://www.w3.org/2004/02/skos/core#Concept"/>
    <rdfs:seeAlso rdf:resource="https://www.opengis.net/def/security/1.0/codelist/authentication/SAML2_TLSClient?_view=alternates"/>
    <rdfs:seeAlso rdf:resource="http://schemas.opengis.net/security/1.0/codelist/authentication.xml"/>
    <skos:notation rdf:datatype="http://www.opengis.net/def/metamodel/URN">urn:oasis:names:tc:SAML:2.0:ac:classes:TLSClient</skos:notation>
    <skos:prefLabel xml:lang="en">SAML2_TLSClient</skos:prefLabel>
    <skos:definition>As specified in https://docs.oasis-open.org/security/saml/v2.0/saml-authn-context-2.0-os.pdf</skos:definition>
    <ns1:status rdf:resource="http://www.opengis.net/def/status/valid"/>
  </rdf:Description>
  <rdf:Description rdf:about="https://www.opengis.net/def/security/">
    <skos:member rdf:resource="https://www.opengis.net/def/security/1.0/"/>
    <rdf:type rdf:resource="http://www.w3.org/2004/02/skos/core#Collection"/>
    <skos:prefLabel>OGC Web Services Security</skos:prefLabel>
    <dc:source>OGC 17-007</dc:source>
    <dcterms:created rdf:datatype="http://www.w3.org/2001/XMLSchema#date">2019-01-23</dcterms:created>
    <owl:sameAs rdf:resource="https://www.opengis.net/def/security"/>
    <skos:definition>OGC Web Services Security</skos:definition>
  </rdf:Description>
  <rdf:Description rdf:about="https://www.opengis.net/def/security/1.0/codelist/authentication/HTTP_BASIC">
    <skos:inScheme rdf:resource="https://www.opengis.net/def/security/1.0/codelist/authentication"/>
    <rdf:type rdf:resource="http://www.w3.org/2004/02/skos/core#Concept"/>
    <rdfs:seeAlso rdf:resource="https://www.opengis.net/def/security/1.0/codelist/authentication/HTTP_BASIC?_view=alternates"/>
    <rdfs:seeAlso rdf:resource="http://schemas.opengis.net/security/1.0/codelist/authentication.xml"/>
    <skos:notation rdf:datatype="http://www.opengis.net/def/metamodel/URN">urn:ogc:def:security:authentication:ietf:2617:Basic</skos:notation>
    <skos:prefLabel xml:lang="en">HTTP_BASIC</skos:prefLabel>
    <skos:definition>The "basic" authentication scheme is based on the model that the
				    client must authenticate itself with a user-ID and a password for
				    each realm.  The realm value should be considered an opaque string
				    which can only be compared for equality with other realms on that
				    server. The server will service the request only if it can validate
				    the user-ID and password for the protection space of the Request-URI.
				    There are no optional authentication parameters.</skos:definition>
    <ns1:status rdf:resource="http://www.opengis.net/def/status/valid"/>
  </rdf:Description>
  <rdf:Description rdf:about="https://www.opengis.net/def/security/1.0/codelist/authentication/HTTP_DIGEST">
    <rdf:type rdf:resource="http://www.w3.org/2004/02/skos/core#Concept"/>
    <rdfs:seeAlso rdf:resource="https://www.opengis.net/def/security/1.0/codelist/authentication/HTTP_DIGEST?_view=alternates"/>
    <rdfs:seeAlso rdf:resource="http://schemas.opengis.net/security/1.0/codelist/authentication.xml"/>
    <skos:notation rdf:datatype="http://www.opengis.net/def/metamodel/URN">urn:ogc:def:security:authentication:ietf:2617:Digest</skos:notation>
    <skos:prefLabel xml:lang="en">HTTP_DIGEST</skos:prefLabel>
    <skos:definition>
            Like Basic Access Authentication, the Digest scheme is based on a
		        simple challenge-response paradigm. The Digest scheme challenges
		        using a nonce value. A valid response contains a checksum (by
		        default, the MD5 checksum) of the username, the password, the given
		        nonce value, the HTTP method, and the requested URI. In this way, the
		        password is never sent in the clear. Just as with the Basic scheme,
		        the username and password must be prearranged in some fashion not
		        addressed by this document.</skos:definition>
    <skos:inScheme rdf:resource="https://www.opengis.net/def/security/1.0/codelist/authentication"/>
    <ns1:status rdf:resource="http://www.opengis.net/def/status/valid"/>
  </rdf:Description>
  <rdf:Description rdf:about="https://www.opengis.net/def/security/1.0/codelist/authentication/SAML2_PublicKeySPKI">
    <rdf:type rdf:resource="http://www.w3.org/2004/02/skos/core#Concept"/>
    <rdfs:seeAlso rdf:resource="https://www.opengis.net/def/security/1.0/codelist/authentication/SAML2_PublicKeySPKI?_view=alternates"/>
    <rdfs:seeAlso rdf:resource="http://schemas.opengis.net/security/1.0/codelist/authentication.xml"/>
    <skos:notation rdf:datatype="http://www.opengis.net/def/metamodel/URN">urn:oasis:names:tc:SAML:2.0:ac:classes:SPKI</skos:notation>
    <skos:prefLabel xml:lang="en">SAML2_PublicKeySPKI</skos:prefLabel>
    <skos:definition>As specified in https://docs.oasis-open.org/security/saml/v2.0/saml-authn-context-2.0-os.pdf</skos:definition>
    <skos:inScheme rdf:resource="https://www.opengis.net/def/security/1.0/codelist/authentication"/>
    <ns1:status rdf:resource="http://www.opengis.net/def/status/valid"/>
  </rdf:Description>
  <rdf:Description rdf:about="https://www.opengis.net/def/security/1.0/codelist/authentication/SAML2_Unspecified">
    <rdf:type rdf:resource="http://www.w3.org/2004/02/skos/core#Concept"/>
    <rdfs:seeAlso rdf:resource="https://www.opengis.net/def/security/1.0/codelist/authentication/SAML2_Unspecified?_view=alternates"/>
    <rdfs:seeAlso rdf:resource="http://schemas.opengis.net/security/1.0/codelist/authentication.xml"/>
    <skos:notation rdf:datatype="http://www.opengis.net/def/metamodel/URN">urn:oasis:names:tc:SAML:2.0:ac:classes:unspecified</skos:notation>
    <skos:prefLabel xml:lang="en">SAML2_Unspecified</skos:prefLabel>
    <skos:definition>As specified in https://docs.oasis-open.org/security/saml/v2.0/saml-authn-context-2.0-os.pdf</skos:definition>
    <skos:inScheme rdf:resource="https://www.opengis.net/def/security/1.0/codelist/authentication"/>
    <ns1:status rdf:resource="http://www.opengis.net/def/status/valid"/>
  </rdf:Description>
  <rdf:Description rdf:about="https://www.opengis.net/def/security/1.0/codelist/authentication/USERNAME_TOKEN">
    <rdf:type rdf:resource="http://www.w3.org/2004/02/skos/core#Concept"/>
    <rdfs:seeAlso rdf:resource="https://www.opengis.net/def/security/1.0/codelist/authentication/USERNAME_TOKEN?_view=alternates"/>
    <rdfs:seeAlso rdf:resource="http://schemas.opengis.net/security/1.0/codelist/authentication.xml"/>
    <skos:notation rdf:datatype="http://www.opengis.net/def/metamodel/URN">urn:ogc:def:security:authentication:wsse:username_token</skos:notation>
    <skos:prefLabel xml:lang="en">USERNAME_TOKEN</skos:prefLabel>
    <skos:definition>WSSE UsernameToken as specified in https://docs.oasis-open.org/wss/2004/01/oasis-200401-wss-username-token-profile-1.0.pdf</skos:definition>
    <skos:inScheme rdf:resource="https://www.opengis.net/def/security/1.0/codelist/authentication"/>
    <ns1:status rdf:resource="http://www.opengis.net/def/status/valid"/>
  </rdf:Description>
  <rdf:Description rdf:about="https://www.opengis.net/def/security">
    <rdf:type rdf:resource="http://www.w3.org/2004/02/skos/core#Concept"/>
    <ns1:collectionView rdf:resource="https://www.opengis.net/def/security/"/>
    <skos:prefLabel>OGC Web Services Security</skos:prefLabel>
    <skos:definition>OGC Web Services Security</skos:definition>
  </rdf:Description>
  <rdf:Description rdf:about="https://www.opengis.net/def/security/1.0">
    <rdf:type rdf:resource="http://www.w3.org/2004/02/skos/core#Concept"/>
    <ns1:collectionView rdf:resource="https://www.opengis.net/def/security/1.0/"/>
    <skos:prefLabel>OGC Web Services Security 1.0</skos:prefLabel>
    <skos:definition>OGC Web Services Security 1.0</skos:definition>
  </rdf:Description>
  <rdf:Description rdf:about="https://www.opengis.net/def/security/1.0/codelist/authentication/SAML2_TelephonyNomadic">
    <skos:inScheme rdf:resource="https://www.opengis.net/def/security/1.0/codelist/authentication"/>
    <rdf:type rdf:resource="http://www.w3.org/2004/02/skos/core#Concept"/>
    <rdfs:seeAlso rdf:resource="https://www.opengis.net/def/security/1.0/codelist/authentication/SAML2_TelephonyNomadic?_view=alternates"/>
    <rdfs:seeAlso rdf:resource="http://schemas.opengis.net/security/1.0/codelist/authentication.xml"/>
    <skos:notation rdf:datatype="http://www.opengis.net/def/metamodel/URN">urn:oasis:names:tc:SAML:2.0:ac:classes:NomadTelephony</skos:notation>
    <skos:prefLabel xml:lang="en">SAML2_TelephonyNomadic</skos:prefLabel>
    <skos:definition>As specified in https://docs.oasis-open.org/security/saml/v2.0/saml-authn-context-2.0-os.pdf</skos:definition>
    <ns1:status rdf:resource="http://www.opengis.net/def/status/valid"/>
  </rdf:Description>
  <rdf:Description rdf:about="http://www.opengis.net/def/entities/bodies/ogcna">
    <rdf:type rdf:resource="http://www.w3.org/2004/02/skos/core#Concept"/>
  </rdf:Description>
  <rdf:Description rdf:about="http://www.opengis.net/def/ogc/">
    <skos:member rdf:resource="https://www.opengis.net/def/security/"/>
  </rdf:Description>
</rdf:RDF>
