# baseURI: https://www.opengis.net/def/profile/skos/owl2skos
# imports: http://datashapes.org/dash
# imports: http://www.w3.org/2004/02/skos/core

@prefix dash: <http://datashapes.org/dash#> .
@prefix dcterms: <http://purl.org/dc/terms/> .
@prefix owl: <http://www.w3.org/2002/07/owl#> .
@prefix rdf: <http://www.w3.org/1999/02/22-rdf-syntax-ns#> .
@prefix rdfs: <http://www.w3.org/2000/01/rdf-schema#> .
@prefix sh: <http://www.w3.org/ns/shacl#> .
@prefix skos: <http://www.w3.org/2004/02/skos/core#> .
@prefix : <https://www.opengis.net/def/profile/skos/owl2skos#> .
@prefix xsd: <http://www.w3.org/2001/XMLSchema#> .

<https://www.opengis.net/def/profile/skos/basics>
  a owl:Ontology ;
  owl:imports <http://datashapes.org/dash> ;
  owl:imports <http://www.w3.org/2004/02/skos/core> ;
  dcterms:creator "Rob Atkinson" ;
  rdfs:comment "SHACL rules to entail a SKOS concept scheme preserving a declared rdfs:subClassOf heirarchy" ;
.

:ontology a sh:NodeShape;
  sh:rule :buildConceptScheme ;
        # skostopconcepts:rdfslabel> ;
  sh:targetClass owl:Ontology ;
.

:feature a sh:NodeShape;
  sh:rule :buildClass ;
        # skostopconcepts:rdfslabel> ;
  sh:targetClass owl:Class ;
.

:buildConceptScheme
  a sh:SPARQLRule ;
  rdfs:label "Build Concept Scheme" ;
  rdfs:comment "Also builds top level collections for classes and properties" ;
  sh:construct """PREFIX ogc: <http://www.opengis.net/def/metamodel/>
    PREFIX ft: <http://www.opengis.net/def/metamodel/featuretypes/>
    PREFIX prof: <http://www.w3.org/ns/dx/prof/>
	  prefix skos: <http://www.w3.org/2004/02/skos/core#>
      PREFIX afn: <http://jena.hpl.hp.com/ARQ/function#>
      prefix dct: <http://purl.org/dc/terms/>
      PREFIX rdfs: <http://www.w3.org/2000/01/rdf-schema#>
      CONSTRUCT {
    ?this a skos:ConceptScheme .
    ?this skos:prefLabel ?cslabel .
    ?this rdfs:comment "This object provides the metadata view of an application schema. Definitions are organised as a SKOS ConceptScheme and can be accessed via the collection view property."@en .
	?this a owl:Ontology .
	?this owl:imports <http://www.opengis.net/ont/geosparql> .
	?this skos:definition ?def .
	?this ft:propertyList ?pcollection .
	?this ft:ftList ?ftcollection .
    ?this ft:codelistList ?clcollection .
	?topcollection a skos:Collection .
    ?topcollection rdfs:comment "This is the collection viewpoint of this application schema, consisting of sub-collections of feature types, properties and codelists defined by the application schema."@en .
    ?topcollection skos:inScheme ?this .
    ?ftcollection a skos:Collection .
    ?ftcollection rdfs:label "Feature Types" .
    ?ftcollection rdfs:comment "All feature types declared in this Application Schema." .
    ?ftcollection skos:inScheme ?this .
	?pcollection a skos:Collection .
    ?pcollection rdfs:label "Feature Properties" .
    ?pcollection rdfs:comment "All properties declared in this Application Schema." .
    ?pcollection skos:inScheme ?this .
	?clcollection a skos:Collection .
    ?clcollection rdfs:label "Code Lists" .
    ?clcollection rdfs:comment "All Code Lists declared in this Application Schema" .
    ?clcollection skos:inScheme ?this .
	?topcollection skos:member ?ftcollection .
	?topcollection skos:member ?pcollection .
    ?topcollection skos:member ?clcollection .
	?ftcollection skos:member ?class .
	?class skos:inScheme ?this .
    ?pcollection skos:member ?property .
    ?property a skos:Concept.
    ?property skos:broader ?superprop .
    ?property skos:inScheme ?this .
}
WHERE {
     ?this a owl:Ontology FILTER ( ?this != <http://www.opengis.net/def/metamodel/featuretypes> )
     OPTIONAL { ?this rdfs:label ?label }
    OPTIONAL { ?this skos:prefLabel ?plabel }
    OPTIONAL { ?this dct:title ?title }
BIND ( COALESCE (?title,?plabel,?label,afn:localname(?this)) as ?cslabel )
	 OPTIONAL { ?this skos:definition ?def }
    OPTIONAL { ?this ogc:sourceGraph ?sourceGraph . }
    BIND ( COALESCE(?sourceGraph,?this) as ?g )
		BIND (URI(CONCAT(str(?g), "/")) AS ?topcollection) .
	BIND (URI(CONCAT(str(?g), "/FeatureTypes/")) AS ?ftcollection) .
	BIND (URI(CONCAT(str(?g), "/Properties/")) AS ?pcollection) .
	BIND (URI(CONCAT(str(?g), "/CodeLists/")) AS ?clcollection) .

      OPTIONAL { ?class a owl:Class  }

        OPTIONAL {
          { ?property a owl:ObjectProperty }
           UNION { ?property a owl:DatatypeProperty }
           UNION { ?property a rdf:Property }
           UNION { ?property rdfs:domain|rdfs:range ?anyClass }
          OPTIONAL { ?property rdfs:subPropertyOf ?superprop }

  }

}""" ;
.

:buildClass
  a sh:SPARQLRule ;
  rdfs:label "Build owl:Class as a Feature and properties" ;
  rdfs:comment "under construction.." ;
  sh:construct """
    PREFIX prof: <http://www.w3.org/ns/dx/prof/>
	  prefix skos: <http://www.w3.org/2004/02/skos/core#>
      PREFIX afn: <http://jena.hpl.hp.com/ARQ/function#>
      prefix dct: <http://purl.org/dc/terms/>
      PREFIX rdfs: <http://www.w3.org/2000/01/rdf-schema#>
      CONSTRUCT {
    ?this a skos:Concept;
       rdfs:comment "Entailed as SKOS Concept for Linked Data purposes." ;
       skos:definition ?bestclassdef ;
	   skos:broader ?parent ;
     .
        }
WHERE {
     ?this a owl:Class .

      OPTIONAL {
            ?this rdfs:subClassOf ?parent FILTER ( !isBlank(?parent) )
        } .

        OPTIONAL { ?this skos:definition ?cdef . }
        OPTIONAL { ?this dct:description ?cdesc . }
        OPTIONAL { ?this rdfs:comment ?ccomment . }
        BIND (COALESCE(?cdef,?cdesc,?ccomment) AS ?bestclassdef) .

}""" ;
.

