<?xml version="1.0" encoding="utf-8"?>
<rdf:RDF
   xmlns:dcterms="http://purl.org/dc/terms/"
   xmlns:ns1="http://www.opengis.net/def/metamodel/ogc-na/"
   xmlns:rdf="http://www.w3.org/1999/02/22-rdf-syntax-ns#"
   xmlns:rdfs="http://www.w3.org/2000/01/rdf-schema#"
   xmlns:skos="http://www.w3.org/2004/02/skos/core#"
>
  <rdf:Description rdf:about="http://www.opengis.net/def/timeseries/ProcessTypeCode">
    <rdf:type rdf:resource="http://www.opengis.net/def/metamodel/lid/lidset"/>
    <rdf:type rdf:resource="http://rdfs.org/ns/void#Dataset"/>
    <rdf:type rdf:resource="http://www.w3.org/2004/02/skos/core#ConceptScheme"/>
    <rdf:type rdf:resource="http://www.opengis.net/def/metamodel/lid/ConceptScheme"/>
    <rdfs:label xml:lang="en">TimeSeriesML - ProcessTypeCode</rdfs:label>
    <rdfs:seeAlso rdf:resource="http://www.opengis.net/def/docs/15-042r5"/>
    <ns1:collectionView rdf:resource="http://www.opengis.net/def/timeseries/ProcessTypeCode/"/>
    <skos:definition xml:lang="en">Terms from this codelist are used to indicate the type of process that was used in an observation.</skos:definition>
    <skos:prefLabel xml:lang="en">TimeSeriesML - ProcessTypeCode</skos:prefLabel>
    <dcterms:source rdf:resource="http://www.opengis.net/def/entities/bodies/ogcna"/>
  </rdf:Description>
  <rdf:Description rdf:about="http://www.opengis.net/def/timeseries/InterpolationCode/AverageSucc">
    <rdf:type rdf:resource="http://www.w3.org/2004/02/skos/core#Concept"/>
    <rdfs:label xml:lang="en">Average Succeeding</rdfs:label>
    <rdfs:seeAlso rdf:resource="http://www.opengis.net/def/docs/15-042r5"/>
    <skos:definition xml:lang="en">Value represents the average value over the following interval.    </skos:definition>
    <skos:inScheme rdf:resource="http://www.opengis.net/def/timeseries/InterpolationCode"/>
    <skos:prefLabel xml:lang="en">Average Succeeding</skos:prefLabel>
    <ns1:status rdf:resource="http://www.opengis.net/def/status/valid"/>
  </rdf:Description>
  <rdf:Description rdf:about="http://www.opengis.net/def/timeseries/DataQualityCode/Poor">
    <rdf:type rdf:resource="http://www.w3.org/2004/02/skos/core#Concept"/>
    <rdfs:label xml:lang="en">Poor</rdfs:label>
    <rdfs:seeAlso rdf:resource="http://www.opengis.net/def/docs/15-042r5"/>
    <skos:definition xml:lang="en">The data should be considered as low quality and may have been rejected.</skos:definition>
    <skos:inScheme rdf:resource="http://www.opengis.net/def/timeseries/DataQualityCode"/>
    <skos:prefLabel xml:lang="en">Poor</skos:prefLabel>
    <ns1:status rdf:resource="http://www.opengis.net/def/status/valid"/>
  </rdf:Description>
  <rdf:Description rdf:about="http://www.opengis.net/def/timeseries/InterpolationCode/ConstPrec">
    <rdf:type rdf:resource="http://www.w3.org/2004/02/skos/core#Concept"/>
    <rdfs:label xml:lang="en">Constant Preceding</rdfs:label>
    <rdfs:seeAlso rdf:resource="http://www.opengis.net/def/docs/15-042r5"/>
    <skos:definition xml:lang="en">Value is constant in the preceding interval.</skos:definition>
    <skos:inScheme rdf:resource="http://www.opengis.net/def/timeseries/InterpolationCode"/>
    <skos:prefLabel xml:lang="en">Constant Preceding</skos:prefLabel>
    <ns1:status rdf:resource="http://www.opengis.net/def/status/valid"/>
  </rdf:Description>
  <rdf:Description rdf:about="http://www.opengis.net/def/timeseriesType/timeseriesML/TimeseriesDomainRange/">
    <rdf:type rdf:resource="http://www.w3.org/2004/02/skos/core#Collection"/>
    <rdfs:label xml:lang="en">Concepts in TimeSeriesML - TimeseriesDomainRange</rdfs:label>
    <rdfs:seeAlso rdf:resource="http://www.opengis.net/def/docs/15-042r5"/>
    <skos:definition xml:lang="en">A tsml:type property is present on the TimeseriesDomainRange type to enable a soft-typing approach to this class. The values for this property should be taken from this list.</skos:definition>
    <skos:inScheme rdf:resource="http://www.opengis.net/def/timeseriesType/timeseriesML/TimeseriesDomainRange"/>
    <skos:member rdf:resource="http://www.opengis.net/def/timeseriesType/timeseriesML/1.2/Time/MeasurementTimeseriesDomainRange"/>
    <skos:member rdf:resource="http://www.opengis.net/def/timeseriesType/timeseriesML/1.2/Time/CategoricalTimeseriesDomainRange"/>
    <skos:prefLabel xml:lang="en">Concepts in TimeSeriesML - TimeseriesDomainRange</skos:prefLabel>
  </rdf:Description>
  <rdf:Description rdf:about="http://www.opengis.net/def/observationType/timeseriesML/1.0/CategoricalTimeseriesTVPObservation">
    <rdf:type rdf:resource="http://www.w3.org/2004/02/skos/core#Concept"/>
    <rdfs:label xml:lang="en">CategoricalTimeseriesTVPObservation</rdfs:label>
    <rdfs:seeAlso rdf:resource="http://www.opengis.net/def/docs/15-042r5"/>
    <skos:definition xml:lang="en">CategoricalTimeseriesTVPObservation</skos:definition>
    <skos:inScheme rdf:resource="http://www.opengis.net/def/observationType/timeseriesML"/>
    <skos:prefLabel xml:lang="en">CategoricalTimeseriesTVPObservation</skos:prefLabel>
    <ns1:status rdf:resource="http://www.opengis.net/def/status/valid"/>
  </rdf:Description>
  <rdf:Description rdf:about="http://www.opengis.net/def/timeseries/InterpolationCode/MinPrec">
    <rdf:type rdf:resource="http://www.w3.org/2004/02/skos/core#Concept"/>
    <rdfs:label xml:lang="en">Minimum Preceding</rdfs:label>
    <rdfs:seeAlso rdf:resource="http://www.opengis.net/def/docs/15-042r5"/>
    <skos:definition xml:lang="en">Value represents the minimum value that was measured during the preceding time interval.</skos:definition>
    <skos:inScheme rdf:resource="http://www.opengis.net/def/timeseries/InterpolationCode"/>
    <skos:prefLabel xml:lang="en">Minimum Preceding</skos:prefLabel>
    <ns1:status rdf:resource="http://www.opengis.net/def/status/valid"/>
  </rdf:Description>
  <rdf:Description rdf:about="http://www.opengis.net/def/observationType/timeseriesML/1.0/MeasurementTimeseriesTVPObservation">
    <rdf:type rdf:resource="http://www.w3.org/2004/02/skos/core#Concept"/>
    <rdfs:label xml:lang="en">MeasurementTimeseriesTVPObservation</rdfs:label>
    <rdfs:seeAlso rdf:resource="http://www.opengis.net/def/docs/15-042r5"/>
    <skos:definition xml:lang="en">MeasurementTimeseriesTVPObservation</skos:definition>
    <skos:inScheme rdf:resource="http://www.opengis.net/def/observationType/timeseriesML"/>
    <skos:prefLabel xml:lang="en">MeasurementTimeseriesTVPObservation</skos:prefLabel>
    <ns1:status rdf:resource="http://www.opengis.net/def/status/valid"/>
  </rdf:Description>
  <rdf:Description rdf:about="http://www.opengis.net/def/timeseries/ProcessTypeCode/ManualMethod">
    <rdf:type rdf:resource="http://www.w3.org/2004/02/skos/core#Concept"/>
    <rdfs:label xml:lang="en">Manual Method</rdfs:label>
    <rdfs:seeAlso rdf:resource="http://www.opengis.net/def/docs/15-042r5"/>
    <skos:definition xml:lang="en">Timeseries data is collected manually</skos:definition>
    <skos:inScheme rdf:resource="http://www.opengis.net/def/timeseries/ProcessTypeCode"/>
    <skos:narrower rdf:resource="http://www.opengis.net/def/waterml/2.0/process-type/manual-method"/>
    <skos:narrower rdf:resource="http://www.opengis.net/def/waterml/2.0/processType/ManualMethod"/>
    <skos:prefLabel xml:lang="en">Manual Method</skos:prefLabel>
    <ns1:status rdf:resource="http://www.opengis.net/def/status/valid"/>
  </rdf:Description>
  <rdf:Description rdf:about="http://www.opengis.net/def/timeseries/DataQualityCode/Estimate">
    <rdf:type rdf:resource="http://www.w3.org/2004/02/skos/core#Concept"/>
    <rdfs:label xml:lang="en">Estimate</rdfs:label>
    <rdfs:seeAlso rdf:resource="http://www.opengis.net/def/docs/15-042r5"/>
    <skos:definition xml:lang="en">The data is an estimate only, not a direct measurement.</skos:definition>
    <skos:inScheme rdf:resource="http://www.opengis.net/def/timeseries/DataQualityCode"/>
    <skos:prefLabel xml:lang="en">Estimate</skos:prefLabel>
    <ns1:status rdf:resource="http://www.opengis.net/def/status/valid"/>
  </rdf:Description>
  <rdf:Description rdf:about="http://www.opengis.net/def/observationType/timeseriesML">
    <rdf:type rdf:resource="http://www.opengis.net/def/metamodel/lid/lidset"/>
    <rdf:type rdf:resource="http://rdfs.org/ns/void#Dataset"/>
    <rdf:type rdf:resource="http://www.w3.org/2004/02/skos/core#ConceptScheme"/>
    <rdf:type rdf:resource="http://www.opengis.net/def/metamodel/lid/ConceptScheme"/>
    <rdfs:label xml:lang="en">TimeSeriesML - observationType</rdfs:label>
    <rdfs:seeAlso rdf:resource="http://www.opengis.net/def/docs/15-042r5"/>
    <ns1:collectionView rdf:resource="http://www.opengis.net/def/observationType/timeseriesML/"/>
    <skos:definition xml:lang="en">In accordance with OMXML, the specialization of the OM_Observation result type is provided through schematron restriction. The om:type element may be used to specify the type of OM_Observation that is being encoded. This shall be done using the OGC Name URI for the corresponding type from this list.</skos:definition>
    <skos:prefLabel xml:lang="en">TimeSeriesML - observationType</skos:prefLabel>
    <dcterms:source rdf:resource="http://www.opengis.net/def/entities/bodies/ogcna"/>
  </rdf:Description>
  <rdf:Description rdf:about="http://www.opengis.net/def/timeseries/DataQualityCode">
    <rdf:type rdf:resource="http://www.opengis.net/def/metamodel/lid/lidset"/>
    <rdf:type rdf:resource="http://rdfs.org/ns/void#Dataset"/>
    <rdf:type rdf:resource="http://www.w3.org/2004/02/skos/core#ConceptScheme"/>
    <rdf:type rdf:resource="http://www.opengis.net/def/metamodel/lid/ConceptScheme"/>
    <rdfs:label xml:lang="en">TimeSeriesML - DataQualityCode</rdfs:label>
    <rdfs:seeAlso rdf:resource="http://www.opengis.net/def/docs/15-042r5"/>
    <ns1:collectionView rdf:resource="http://www.opengis.net/def/timeseries/DataQualityCode/"/>
    <skos:definition xml:lang="en">Terms in this codelist are used to indicate the quality of individual data points.</skos:definition>
    <skos:prefLabel xml:lang="en">TimeSeriesML - DataQualityCode</skos:prefLabel>
    <dcterms:source rdf:resource="http://www.opengis.net/def/entities/bodies/ogcna"/>
  </rdf:Description>
  <rdf:Description rdf:about="http://www.opengis.net/def/timeseries/InterpolationCode/">
    <rdf:type rdf:resource="http://www.w3.org/2004/02/skos/core#Collection"/>
    <rdfs:label xml:lang="en">Concepts in TimeSeriesML - InterpolationCode</rdfs:label>
    <rdfs:seeAlso rdf:resource="http://www.opengis.net/def/docs/15-042r5"/>
    <skos:definition xml:lang="en">Terms in this codelist are used to indicate how data should be interpolated between neighboring points in a timeseries.</skos:definition>
    <skos:inScheme rdf:resource="http://www.opengis.net/def/timeseries/InterpolationCode"/>
    <skos:member rdf:resource="http://www.opengis.net/def/timeseries/InterpolationCode/AveragePrec"/>
    <skos:member rdf:resource="http://www.opengis.net/def/timeseries/InterpolationCode/MaxPrec"/>
    <skos:member rdf:resource="http://www.opengis.net/def/timeseries/InterpolationCode/TotalSucc"/>
    <skos:member rdf:resource="http://www.opengis.net/def/timeseries/InterpolationCode/InstantTotal"/>
    <skos:member rdf:resource="http://www.opengis.net/def/timeseries/InterpolationCode/Discontinuous"/>
    <skos:member rdf:resource="http://www.opengis.net/def/timeseries/InterpolationCode/MinSucc"/>
    <skos:member rdf:resource="http://www.opengis.net/def/timeseries/InterpolationCode/ConstPrec"/>
    <skos:member rdf:resource="http://www.opengis.net/def/timeseries/InterpolationCode/Continuous"/>
    <skos:member rdf:resource="http://www.opengis.net/def/timeseries/InterpolationCode/AverageSucc"/>
    <skos:member rdf:resource="http://www.opengis.net/def/timeseries/InterpolationCode/PrecTotal"/>
    <skos:member rdf:resource="http://www.opengis.net/def/timeseries/InterpolationCode/MaxSucc"/>
    <skos:member rdf:resource="http://www.opengis.net/def/timeseries/InterpolationCode/MinPrec"/>
    <skos:member rdf:resource="http://www.opengis.net/def/timeseries/InterpolationCode/ConstSucc"/>
    <skos:prefLabel xml:lang="en">Concepts in TimeSeriesML - InterpolationCode</skos:prefLabel>
  </rdf:Description>
  <rdf:Description rdf:about="http://www.opengis.net/def/timeseries/ProcessTypeCode/Sensor">
    <rdf:type rdf:resource="http://www.w3.org/2004/02/skos/core#Concept"/>
    <rdfs:label xml:lang="en">Sensor</rdfs:label>
    <rdfs:seeAlso rdf:resource="http://www.opengis.net/def/docs/15-042r5"/>
    <skos:definition xml:lang="en">Timeseries data is collected from an automated sensor</skos:definition>
    <skos:inScheme rdf:resource="http://www.opengis.net/def/timeseries/ProcessTypeCode"/>
    <skos:narrower rdf:resource="http://www.opengis.net/def/waterml/2.0/processType/Sensor"/>
    <skos:narrower rdf:resource="http://www.opengis.net/def/waterml/2.0/process-type/sensor"/>
    <skos:prefLabel xml:lang="en">Sensor</skos:prefLabel>
    <ns1:status rdf:resource="http://www.opengis.net/def/status/valid"/>
  </rdf:Description>
  <rdf:Description rdf:about="http://www.opengis.net/def/timeseriesType/timeseriesML/TimeseriesDomainRange">
    <rdf:type rdf:resource="http://www.opengis.net/def/metamodel/lid/lidset"/>
    <rdf:type rdf:resource="http://rdfs.org/ns/void#Dataset"/>
    <rdf:type rdf:resource="http://www.w3.org/2004/02/skos/core#ConceptScheme"/>
    <rdf:type rdf:resource="http://www.opengis.net/def/metamodel/lid/ConceptScheme"/>
    <rdfs:label xml:lang="en">TimeSeriesML - TimeseriesDomainRange</rdfs:label>
    <rdfs:seeAlso rdf:resource="http://www.opengis.net/def/docs/15-042r5"/>
    <ns1:collectionView rdf:resource="http://www.opengis.net/def/timeseriesType/timeseriesML/TimeseriesDomainRange/"/>
    <skos:definition xml:lang="en">A tsml:type property is present on the TimeseriesDomainRange type to enable a soft-typing approach to this class. The values for this property should be taken from this list.</skos:definition>
    <skos:prefLabel xml:lang="en">TimeSeriesML - TimeseriesDomainRange</skos:prefLabel>
    <dcterms:source rdf:resource="http://www.opengis.net/def/entities/bodies/ogcna"/>
  </rdf:Description>
  <rdf:Description rdf:about="http://www.opengis.net/def/timeseriesType/timeseriesML/1.2/Time/CategoricalTimeseriesDomainRange">
    <rdf:type rdf:resource="http://www.w3.org/2004/02/skos/core#Concept"/>
    <rdfs:label xml:lang="en">CategoricalTimeseriesDomainRangeTimeseries</rdfs:label>
    <rdfs:seeAlso rdf:resource="http://www.opengis.net/def/docs/15-042r5"/>
    <skos:definition xml:lang="en">CategoricalTimeseriesDomainRangeTimeseries</skos:definition>
    <skos:inScheme rdf:resource="http://www.opengis.net/def/timeseriesType/timeseriesML"/>
    <skos:prefLabel xml:lang="en">CategoricalTimeseriesDomainRangeTimeseries</skos:prefLabel>
    <ns1:status rdf:resource="http://www.opengis.net/def/status/valid"/>
  </rdf:Description>
  <rdf:Description rdf:about="http://www.opengis.net/def/timeseries/InterpolationCode/TotalSucc">
    <rdf:type rdf:resource="http://www.w3.org/2004/02/skos/core#Concept"/>
    <rdfs:label xml:lang="en">Total Succeeding</rdfs:label>
    <rdfs:seeAlso rdf:resource="http://www.opengis.net/def/docs/15-042r5"/>
    <skos:definition xml:lang="en">Value represents the average value over the following interval.</skos:definition>
    <skos:inScheme rdf:resource="http://www.opengis.net/def/timeseries/InterpolationCode"/>
    <skos:prefLabel xml:lang="en">Total Succeeding</skos:prefLabel>
    <ns1:status rdf:resource="http://www.opengis.net/def/status/valid"/>
  </rdf:Description>
  <rdf:Description rdf:about="http://www.opengis.net/def/observationType/timeseriesML/1.0/MeasurementTimeseriesDomainRangeObservation">
    <rdf:type rdf:resource="http://www.w3.org/2004/02/skos/core#Concept"/>
    <rdfs:label xml:lang="en">MeasurementTimeseriesDomainRangeObservation</rdfs:label>
    <rdfs:seeAlso rdf:resource="http://www.opengis.net/def/docs/15-042r5"/>
    <skos:definition xml:lang="en">MeasurementTimeseriesDomainRangeObservation</skos:definition>
    <skos:inScheme rdf:resource="http://www.opengis.net/def/observationType/timeseriesML"/>
    <skos:prefLabel xml:lang="en">MeasurementTimeseriesDomainRangeObservation</skos:prefLabel>
    <ns1:status rdf:resource="http://www.opengis.net/def/status/valid"/>
  </rdf:Description>
  <rdf:Description rdf:about="http://www.opengis.net/def/timeseries/ProcessTypeCode/Algorithm">
    <rdf:type rdf:resource="http://www.w3.org/2004/02/skos/core#Concept"/>
    <rdfs:label xml:lang="en">Algorithm</rdfs:label>
    <rdfs:seeAlso rdf:resource="http://www.opengis.net/def/docs/15-042r5"/>
    <skos:definition xml:lang="en">Timeseries data is generated by applying an algorithm to input data</skos:definition>
    <skos:inScheme rdf:resource="http://www.opengis.net/def/timeseries/ProcessTypeCode"/>
    <skos:narrower rdf:resource="http://www.opengis.net/def/waterml/2.0/processType/Algorithm"/>
    <skos:narrower rdf:resource="http://www.opengis.net/def/waterml/2.0/process-type/algorithm"/>
    <skos:prefLabel xml:lang="en">Algorithm</skos:prefLabel>
    <ns1:status rdf:resource="http://www.opengis.net/def/status/valid"/>
  </rdf:Description>
  <rdf:Description rdf:about="http://www.opengis.net/def/timeseries/InterpolationCode/PrecTotal">
    <rdf:type rdf:resource="http://www.w3.org/2004/02/skos/core#Concept"/>
    <rdfs:label xml:lang="en">Preceding Total</rdfs:label>
    <rdfs:seeAlso rdf:resource="http://www.opengis.net/def/docs/15-042r5"/>
    <skos:definition xml:lang="en">Value represents the total of measurements taken within the previous time interval.</skos:definition>
    <skos:inScheme rdf:resource="http://www.opengis.net/def/timeseries/InterpolationCode"/>
    <skos:prefLabel xml:lang="en">Preceding Total</skos:prefLabel>
    <ns1:status rdf:resource="http://www.opengis.net/def/status/valid"/>
  </rdf:Description>
  <rdf:Description rdf:about="http://www.opengis.net/def/timeseries/InterpolationCode/MaxSucc">
    <rdf:type rdf:resource="http://www.w3.org/2004/02/skos/core#Concept"/>
    <rdfs:label xml:lang="en">Maximum Succeeding</rdfs:label>
    <rdfs:seeAlso rdf:resource="http://www.opengis.net/def/docs/15-042r5"/>
    <skos:definition xml:lang="en">Value represents the maximum value for the following interval.</skos:definition>
    <skos:inScheme rdf:resource="http://www.opengis.net/def/timeseries/InterpolationCode"/>
    <skos:prefLabel xml:lang="en">Maximum Succeeding</skos:prefLabel>
    <ns1:status rdf:resource="http://www.opengis.net/def/status/valid"/>
  </rdf:Description>
  <rdf:Description rdf:about="http://www.opengis.net/def/timeseries/DataQualityCode/">
    <rdf:type rdf:resource="http://www.w3.org/2004/02/skos/core#Collection"/>
    <rdfs:label xml:lang="en">Concepts in TimeSeriesML - DataQualityCode</rdfs:label>
    <rdfs:seeAlso rdf:resource="http://www.opengis.net/def/docs/15-042r5"/>
    <skos:definition xml:lang="en">Terms in this codelist are used to indicate the quality of individual data points.</skos:definition>
    <skos:inScheme rdf:resource="http://www.opengis.net/def/timeseries/DataQualityCode"/>
    <skos:member rdf:resource="http://www.opengis.net/def/timeseries/DataQualityCode/Missing"/>
    <skos:member rdf:resource="http://www.opengis.net/def/timeseries/DataQualityCode/Poor"/>
    <skos:member rdf:resource="http://www.opengis.net/def/timeseries/DataQualityCode/Good"/>
    <skos:member rdf:resource="http://www.opengis.net/def/timeseries/DataQualityCode/Unchecked"/>
    <skos:member rdf:resource="http://www.opengis.net/def/timeseries/DataQualityCode/Suspect"/>
    <skos:member rdf:resource="http://www.opengis.net/def/timeseries/DataQualityCode/Estimate"/>
    <skos:prefLabel xml:lang="en">Concepts in TimeSeriesML - DataQualityCode</skos:prefLabel>
  </rdf:Description>
  <rdf:Description rdf:about="http://www.opengis.net/def/observationType/timeseriesML/">
    <rdf:type rdf:resource="http://www.w3.org/2004/02/skos/core#Collection"/>
    <rdfs:label xml:lang="en">Concepts in TimeSeriesML - observationType</rdfs:label>
    <rdfs:seeAlso rdf:resource="http://www.opengis.net/def/docs/15-042r5"/>
    <skos:definition xml:lang="en">Terms in this codelist are used to indicate how data should be interpolated between neighboring points in a timeseries.</skos:definition>
    <skos:inScheme rdf:resource="http://www.opengis.net/def/observationType/timeseriesML"/>
    <skos:member rdf:resource="http://www.opengis.net/def/observationType/timeseriesML/1.0/CategoricalTimeseriesTVPObservation"/>
    <skos:member rdf:resource="http://www.opengis.net/def/observationType/timeseriesML/1.0/MeasurementTimeseriesDomainRangeObservation"/>
    <skos:member rdf:resource="http://www.opengis.net/def/observationType/timeseriesML/1.0/CategoricalTimeseriesDomainRangeObservation"/>
    <skos:member rdf:resource="http://www.opengis.net/def/observationType/timeseriesML/1.0/MeasurementTimeseriesTVPObservation"/>
    <skos:prefLabel xml:lang="en">Concepts in TimeSeriesML - observationType</skos:prefLabel>
  </rdf:Description>
  <rdf:Description rdf:about="http://www.opengis.net/def/timeseries/InterpolationCode/Continuous">
    <rdf:type rdf:resource="http://www.w3.org/2004/02/skos/core#Concept"/>
    <rdfs:label xml:lang="en">Continuous</rdfs:label>
    <rdfs:seeAlso rdf:resource="http://www.opengis.net/def/docs/15-042r5"/>
    <skos:definition xml:lang="en">A continuous timeseries indicates the observation result is the value of a property at the indicated instant in time. The points are essentially connected and interpolation may occur between points in order to estimate the value of the property between points. The appropriate time spacing between successive points to minimize interpolation errors is related to rate of change (with respect to time) of the property.</skos:definition>
    <skos:inScheme rdf:resource="http://www.opengis.net/def/timeseries/InterpolationCode"/>
    <skos:prefLabel xml:lang="en">Continuous</skos:prefLabel>
    <ns1:status rdf:resource="http://www.opengis.net/def/status/valid"/>
  </rdf:Description>
  <rdf:Description rdf:about="http://www.opengis.net/def/timeseries/ProcessTypeCode/Unknown">
    <rdf:type rdf:resource="http://www.w3.org/2004/02/skos/core#Concept"/>
    <rdfs:label xml:lang="en">Unknown</rdfs:label>
    <rdfs:seeAlso rdf:resource="http://www.opengis.net/def/docs/15-042r5"/>
    <skos:definition xml:lang="en">Timeseries is collected or generated by an unknown process</skos:definition>
    <skos:inScheme rdf:resource="http://www.opengis.net/def/timeseries/ProcessTypeCode"/>
    <skos:narrower rdf:resource="http://www.opengis.net/def/waterml/2.0/processType/Unknown"/>
    <skos:narrower rdf:resource="http://www.opengis.net/def/waterml/2.0/process-type/unknown"/>
    <skos:prefLabel xml:lang="en">Unknown</skos:prefLabel>
    <ns1:status rdf:resource="http://www.opengis.net/def/status/valid"/>
  </rdf:Description>
  <rdf:Description rdf:about="http://www.opengis.net/def/observationType/timeseriesML/1.0/CategoricalTimeseriesDomainRangeObservation">
    <rdf:type rdf:resource="http://www.w3.org/2004/02/skos/core#Concept"/>
    <rdfs:label xml:lang="en">CategoricalTimeseriesDomainRangeObservation</rdfs:label>
    <rdfs:seeAlso rdf:resource="http://www.opengis.net/def/docs/15-042r5"/>
    <skos:definition xml:lang="en">CategoricalTimeseriesDomainRangeObservation</skos:definition>
    <skos:inScheme rdf:resource="http://www.opengis.net/def/observationType/timeseriesML"/>
    <skos:prefLabel xml:lang="en">CategoricalTimeseriesDomainRangeObservation</skos:prefLabel>
    <ns1:status rdf:resource="http://www.opengis.net/def/status/valid"/>
  </rdf:Description>
  <rdf:Description rdf:about="http://www.opengis.net/def/waterml/2.0/process-type/manual-method">
    <skos:broader rdf:resource="http://www.opengis.net/def/timeseries/ProcessTypeCode/ManualMethod"/>
  </rdf:Description>
  <rdf:Description rdf:about="http://www.opengis.net/def/timeseries/DataQualityCode/Unchecked">
    <rdf:type rdf:resource="http://www.w3.org/2004/02/skos/core#Concept"/>
    <rdfs:label xml:lang="en">Unchecked</rdfs:label>
    <rdfs:seeAlso rdf:resource="http://www.opengis.net/def/docs/15-042r5"/>
    <skos:definition xml:lang="en">The data has not been checked by any qualitative method.</skos:definition>
    <skos:inScheme rdf:resource="http://www.opengis.net/def/timeseries/DataQualityCode"/>
    <skos:prefLabel xml:lang="en">Unchecked</skos:prefLabel>
    <ns1:status rdf:resource="http://www.opengis.net/def/status/valid"/>
  </rdf:Description>
  <rdf:Description rdf:about="http://www.opengis.net/def/timeseries/InterpolationCode/MaxPrec">
    <rdf:type rdf:resource="http://www.w3.org/2004/02/skos/core#Concept"/>
    <rdfs:label xml:lang="en">Maximum Preceding</rdfs:label>
    <rdfs:seeAlso rdf:resource="http://www.opengis.net/def/docs/15-042r5"/>
    <skos:definition xml:lang="en">Value represents the maximum value that was measured during the preceding time interval.</skos:definition>
    <skos:inScheme rdf:resource="http://www.opengis.net/def/timeseries/InterpolationCode"/>
    <skos:prefLabel xml:lang="en">Maximum Preceding</skos:prefLabel>
    <ns1:status rdf:resource="http://www.opengis.net/def/status/valid"/>
  </rdf:Description>
  <rdf:Description rdf:about="http://www.opengis.net/def/timeseries/InterpolationCode">
    <rdf:type rdf:resource="http://www.opengis.net/def/metamodel/lid/lidset"/>
    <rdf:type rdf:resource="http://rdfs.org/ns/void#Dataset"/>
    <rdf:type rdf:resource="http://www.w3.org/2004/02/skos/core#ConceptScheme"/>
    <rdf:type rdf:resource="http://www.opengis.net/def/metamodel/lid/ConceptScheme"/>
    <rdfs:label xml:lang="en">TimeSeriesML - InterpolationCode</rdfs:label>
    <rdfs:seeAlso rdf:resource="http://www.opengis.net/def/docs/15-042r5"/>
    <ns1:collectionView rdf:resource="http://www.opengis.net/def/timeseries/InterpolationCode/"/>
    <skos:definition xml:lang="en">Terms in this codelist are used to indicate how data should be interpolated between neighboring points in a timeseries.</skos:definition>
    <skos:prefLabel xml:lang="en">TimeSeriesML - InterpolationCode</skos:prefLabel>
    <dcterms:source rdf:resource="http://www.opengis.net/def/entities/bodies/ogcna"/>
  </rdf:Description>
  <rdf:Description rdf:about="http://www.opengis.net/def/timeseries/InterpolationCode/MinSucc">
    <rdf:type rdf:resource="http://www.w3.org/2004/02/skos/core#Concept"/>
    <rdfs:label xml:lang="en">Minimum Succeeding</rdfs:label>
    <rdfs:seeAlso rdf:resource="http://www.opengis.net/def/docs/15-042r5"/>
    <skos:definition xml:lang="en">Value represents the minimum value for the following interval.</skos:definition>
    <skos:inScheme rdf:resource="http://www.opengis.net/def/timeseries/InterpolationCode"/>
    <skos:prefLabel xml:lang="en">Minimum Succeeding</skos:prefLabel>
    <ns1:status rdf:resource="http://www.opengis.net/def/status/valid"/>
  </rdf:Description>
  <rdf:Description rdf:about="http://www.opengis.net/def/timeseries/ProcessTypeCode/Simulation">
    <rdf:type rdf:resource="http://www.w3.org/2004/02/skos/core#Concept"/>
    <rdfs:label xml:lang="en">Simulation</rdfs:label>
    <rdfs:seeAlso rdf:resource="http://www.opengis.net/def/docs/15-042r5"/>
    <skos:definition xml:lang="en">Timeseries is generated from a simulation</skos:definition>
    <skos:inScheme rdf:resource="http://www.opengis.net/def/timeseries/ProcessTypeCode"/>
    <skos:narrower rdf:resource="http://www.opengis.net/def/waterml/2.0/processType/Simulation"/>
    <skos:narrower rdf:resource="http://www.opengis.net/def/waterml/2.0/process-type/simulation"/>
    <skos:prefLabel xml:lang="en">Simulation</skos:prefLabel>
    <ns1:status rdf:resource="http://www.opengis.net/def/status/valid"/>
  </rdf:Description>
  <rdf:Description rdf:about="http://www.opengis.net/def/waterml/2.0/processType/Algorithm">
    <skos:broader rdf:resource="http://www.opengis.net/def/timeseries/ProcessTypeCode/Algorithm"/>
  </rdf:Description>
  <rdf:Description rdf:about="http://www.opengis.net/def/timeseries/ProcessTypeCode/">
    <rdf:type rdf:resource="http://www.w3.org/2004/02/skos/core#Collection"/>
    <rdfs:label xml:lang="en">Concepts in TimeSeriesML - ProcessTypeCode</rdfs:label>
    <rdfs:seeAlso rdf:resource="http://www.opengis.net/def/docs/15-042r5"/>
    <skos:definition xml:lang="en">Terms from this codelist are used to indicate the type of process that was used in an observation.</skos:definition>
    <skos:inScheme rdf:resource="http://www.opengis.net/def/timeseries/ProcessTypeCode"/>
    <skos:member rdf:resource="http://www.opengis.net/def/timeseries/ProcessTypeCode/ManualMethod"/>
    <skos:member rdf:resource="http://www.opengis.net/def/timeseries/ProcessTypeCode/Sensor"/>
    <skos:member rdf:resource="http://www.opengis.net/def/timeseries/ProcessTypeCode/Unknown"/>
    <skos:member rdf:resource="http://www.opengis.net/def/timeseries/ProcessTypeCode/Algorithm"/>
    <skos:member rdf:resource="http://www.opengis.net/def/timeseries/ProcessTypeCode/Simulation"/>
    <skos:prefLabel xml:lang="en">Concepts in TimeSeriesML - ProcessTypeCode</skos:prefLabel>
  </rdf:Description>
  <rdf:Description rdf:about="http://www.opengis.net/def/timeseries/InterpolationCode/Discontinuous">
    <rdf:type rdf:resource="http://www.w3.org/2004/02/skos/core#Concept"/>
    <rdfs:label xml:lang="en">Discontinuous</rdfs:label>
    <rdfs:seeAlso rdf:resource="http://www.opengis.net/def/docs/15-042r5"/>
    <skos:definition xml:lang="en">The sampling of the property occurs such that it is not possible to regard the series as continuous. The time between samples is too large to classify the measurements as continuous. Example: An infrequent water sample measuring pH.</skos:definition>
    <skos:inScheme rdf:resource="http://www.opengis.net/def/timeseries/InterpolationCode"/>
    <skos:prefLabel xml:lang="en">Discontinuous</skos:prefLabel>
    <ns1:status rdf:resource="http://www.opengis.net/def/status/valid"/>
  </rdf:Description>
  <rdf:Description rdf:about="http://www.opengis.net/def/timeseries/DataQualityCode/Suspect">
    <rdf:type rdf:resource="http://www.w3.org/2004/02/skos/core#Concept"/>
    <rdfs:label xml:lang="en">Suspect</rdfs:label>
    <rdfs:seeAlso rdf:resource="http://www.opengis.net/def/docs/15-042r5"/>
    <skos:definition xml:lang="en">The data should be treated as suspect.</skos:definition>
    <skos:inScheme rdf:resource="http://www.opengis.net/def/timeseries/DataQualityCode"/>
    <skos:prefLabel xml:lang="en">Suspect</skos:prefLabel>
    <ns1:status rdf:resource="http://www.opengis.net/def/status/valid"/>
  </rdf:Description>
  <rdf:Description rdf:about="http://www.opengis.net/def/timeseries/InterpolationCode/ConstSucc">
    <rdf:type rdf:resource="http://www.w3.org/2004/02/skos/core#Concept"/>
    <rdfs:label xml:lang="en">Constant Succeeding</rdfs:label>
    <rdfs:seeAlso rdf:resource="http://www.opengis.net/def/docs/15-042r5"/>
    <skos:definition xml:lang="en">Value is constant in the succeeding interval.</skos:definition>
    <skos:inScheme rdf:resource="http://www.opengis.net/def/timeseries/InterpolationCode"/>
    <skos:prefLabel xml:lang="en">Constant Succeeding</skos:prefLabel>
    <ns1:status rdf:resource="http://www.opengis.net/def/status/valid"/>
  </rdf:Description>
  <rdf:Description rdf:about="http://www.opengis.net/def/waterml/2.0/processType/ManualMethod">
    <skos:broader rdf:resource="http://www.opengis.net/def/timeseries/ProcessTypeCode/ManualMethod"/>
  </rdf:Description>
  <rdf:Description rdf:about="http://www.opengis.net/def/waterml/2.0/process-type/simulation">
    <skos:broader rdf:resource="http://www.opengis.net/def/timeseries/ProcessTypeCode/Simulation"/>
  </rdf:Description>
  <rdf:Description rdf:about="http://www.opengis.net/def/timeseriesType/timeseriesML/1.2/Time/MeasurementTimeseriesDomainRange">
    <rdf:type rdf:resource="http://www.w3.org/2004/02/skos/core#Concept"/>
    <rdfs:label xml:lang="en">MeasurementTimeseriesDomainRangeTimeseries</rdfs:label>
    <rdfs:seeAlso rdf:resource="http://www.opengis.net/def/docs/15-042r5"/>
    <skos:definition xml:lang="en">MeasurementTimeseriesDomainRangeTimeseries</skos:definition>
    <skos:inScheme rdf:resource="http://www.opengis.net/def/timeseriesType/timeseriesML"/>
    <skos:prefLabel xml:lang="en">MeasurementTimeseriesDomainRangeTimeseries</skos:prefLabel>
    <ns1:status rdf:resource="http://www.opengis.net/def/status/valid"/>
  </rdf:Description>
  <rdf:Description rdf:about="http://www.opengis.net/def/timeseries/DataQualityCode/Good">
    <rdf:type rdf:resource="http://www.w3.org/2004/02/skos/core#Concept"/>
    <rdfs:label xml:lang="en">Good</rdfs:label>
    <rdfs:seeAlso rdf:resource="http://www.opengis.net/def/docs/15-042r5"/>
    <skos:definition xml:lang="en">The data has been examined and represents a reliable measurement.</skos:definition>
    <skos:inScheme rdf:resource="http://www.opengis.net/def/timeseries/DataQualityCode"/>
    <skos:prefLabel xml:lang="en">Good</skos:prefLabel>
    <ns1:status rdf:resource="http://www.opengis.net/def/status/valid"/>
  </rdf:Description>
  <rdf:Description rdf:about="http://www.opengis.net/def/timeseries/DataQualityCode/Missing">
    <rdf:type rdf:resource="http://www.w3.org/2004/02/skos/core#Concept"/>
    <rdfs:label xml:lang="en">Missing</rdfs:label>
    <rdfs:seeAlso rdf:resource="http://www.opengis.net/def/docs/15-042r5"/>
    <skos:definition xml:lang="en">The data is missing.</skos:definition>
    <skos:inScheme rdf:resource="http://www.opengis.net/def/timeseries/DataQualityCode"/>
    <skos:prefLabel xml:lang="en">Missing</skos:prefLabel>
    <ns1:status rdf:resource="http://www.opengis.net/def/status/valid"/>
  </rdf:Description>
  <rdf:Description rdf:about="http://www.opengis.net/def/waterml/2.0/process-type/algorithm">
    <skos:broader rdf:resource="http://www.opengis.net/def/timeseries/ProcessTypeCode/Algorithm"/>
  </rdf:Description>
  <rdf:Description rdf:about="http://www.opengis.net/def/timeseries/InterpolationCode/AveragePrec">
    <rdf:type rdf:resource="http://www.w3.org/2004/02/skos/core#Concept"/>
    <rdfs:label xml:lang="en">Average Preceding</rdfs:label>
    <rdfs:seeAlso rdf:resource="http://www.opengis.net/def/docs/15-042r5"/>
    <skos:definition xml:lang="en">Value represents the average value over the preceding interval.    </skos:definition>
    <skos:inScheme rdf:resource="http://www.opengis.net/def/timeseries/InterpolationCode"/>
    <skos:prefLabel xml:lang="en">Average Preceding</skos:prefLabel>
    <ns1:status rdf:resource="http://www.opengis.net/def/status/valid"/>
  </rdf:Description>
  <rdf:Description rdf:about="http://www.opengis.net/def/waterml/2.0/processType/Unknown">
    <skos:broader rdf:resource="http://www.opengis.net/def/timeseries/ProcessTypeCode/Unknown"/>
  </rdf:Description>
  <rdf:Description rdf:about="http://www.opengis.net/def/timeseries/InterpolationCode/InstantTotal">
    <rdf:type rdf:resource="http://www.w3.org/2004/02/skos/core#Concept"/>
    <rdfs:label xml:lang="en">Instant Total</rdfs:label>
    <rdfs:seeAlso rdf:resource="http://www.opengis.net/def/docs/15-042r5"/>
    <skos:definition xml:lang="en">Value represents a total attributed to a specific time instant. This is normally generated from an event based measuring device. Example: An individual tip of a tipping bucket rain gauge.</skos:definition>
    <skos:inScheme rdf:resource="http://www.opengis.net/def/timeseries/InterpolationCode"/>
    <skos:prefLabel xml:lang="en">Instant Total</skos:prefLabel>
    <ns1:status rdf:resource="http://www.opengis.net/def/status/valid"/>
  </rdf:Description>
  <rdf:Description rdf:about="http://www.opengis.net/def/waterml/2.0/process-type/sensor">
    <skos:broader rdf:resource="http://www.opengis.net/def/timeseries/ProcessTypeCode/Sensor"/>
  </rdf:Description>
  <rdf:Description rdf:about="http://www.opengis.net/def/waterml/2.0/processType/Simulation">
    <skos:broader rdf:resource="http://www.opengis.net/def/timeseries/ProcessTypeCode/Simulation"/>
  </rdf:Description>
  <rdf:Description rdf:about="http://www.opengis.net/def/waterml/2.0/process-type/unknown">
    <skos:broader rdf:resource="http://www.opengis.net/def/timeseries/ProcessTypeCode/Unknown"/>
  </rdf:Description>
  <rdf:Description rdf:about="http://www.opengis.net/def/waterml/2.0/processType/Sensor">
    <skos:broader rdf:resource="http://www.opengis.net/def/timeseries/ProcessTypeCode/Sensor"/>
  </rdf:Description>
  <rdf:Description rdf:about="http://www.opengis.net/def/entities/bodies/ogcna">
    <rdf:type rdf:resource="http://www.w3.org/2004/02/skos/core#Concept"/>
  </rdf:Description>
</rdf:RDF>
