@prefix dcterms: <http://purl.org/dc/terms/> .
@prefix ns1: <http://www.opengis.net/def/metamodel/ogc-na/> .
@prefix rdfs: <http://www.w3.org/2000/01/rdf-schema#> .
@prefix skos: <http://www.w3.org/2004/02/skos/core#> .
@prefix void: <http://rdfs.org/ns/void#> .

<http://www.opengis.net/def/observationType/timeseriesML/> a skos:Collection ;
    rdfs:label "Concepts in TimeSeriesML - observationType"@en ;
    rdfs:seeAlso <http://www.opengis.net/def/docs/15-042r5> ;
    skos:definition "Terms in this codelist are used to indicate how data should be interpolated between neighboring points in a timeseries."@en ;
    skos:inScheme <http://www.opengis.net/def/observationType/timeseriesML> ;
    skos:member <http://www.opengis.net/def/observationType/timeseriesML/1.0/CategoricalTimeseriesDomainRangeObservation>,
        <http://www.opengis.net/def/observationType/timeseriesML/1.0/CategoricalTimeseriesTVPObservation>,
        <http://www.opengis.net/def/observationType/timeseriesML/1.0/MeasurementTimeseriesDomainRangeObservation>,
        <http://www.opengis.net/def/observationType/timeseriesML/1.0/MeasurementTimeseriesTVPObservation> ;
    skos:prefLabel "Concepts in TimeSeriesML - observationType"@en .

<http://www.opengis.net/def/observationType/timeseriesML/1.0/CategoricalTimeseriesDomainRangeObservation> a skos:Concept ;
    rdfs:label "CategoricalTimeseriesDomainRangeObservation"@en ;
    ns1:status <http://www.opengis.net/def/status/valid> ;
    rdfs:seeAlso <http://www.opengis.net/def/docs/15-042r5> ;
    skos:definition "CategoricalTimeseriesDomainRangeObservation"@en ;
    skos:inScheme <http://www.opengis.net/def/observationType/timeseriesML> ;
    skos:prefLabel "CategoricalTimeseriesDomainRangeObservation"@en .

<http://www.opengis.net/def/observationType/timeseriesML/1.0/CategoricalTimeseriesTVPObservation> a skos:Concept ;
    rdfs:label "CategoricalTimeseriesTVPObservation"@en ;
    ns1:status <http://www.opengis.net/def/status/valid> ;
    rdfs:seeAlso <http://www.opengis.net/def/docs/15-042r5> ;
    skos:definition "CategoricalTimeseriesTVPObservation"@en ;
    skos:inScheme <http://www.opengis.net/def/observationType/timeseriesML> ;
    skos:prefLabel "CategoricalTimeseriesTVPObservation"@en .

<http://www.opengis.net/def/observationType/timeseriesML/1.0/MeasurementTimeseriesDomainRangeObservation> a skos:Concept ;
    rdfs:label "MeasurementTimeseriesDomainRangeObservation"@en ;
    ns1:status <http://www.opengis.net/def/status/valid> ;
    rdfs:seeAlso <http://www.opengis.net/def/docs/15-042r5> ;
    skos:definition "MeasurementTimeseriesDomainRangeObservation"@en ;
    skos:inScheme <http://www.opengis.net/def/observationType/timeseriesML> ;
    skos:prefLabel "MeasurementTimeseriesDomainRangeObservation"@en .

<http://www.opengis.net/def/observationType/timeseriesML/1.0/MeasurementTimeseriesTVPObservation> a skos:Concept ;
    rdfs:label "MeasurementTimeseriesTVPObservation"@en ;
    ns1:status <http://www.opengis.net/def/status/valid> ;
    rdfs:seeAlso <http://www.opengis.net/def/docs/15-042r5> ;
    skos:definition "MeasurementTimeseriesTVPObservation"@en ;
    skos:inScheme <http://www.opengis.net/def/observationType/timeseriesML> ;
    skos:prefLabel "MeasurementTimeseriesTVPObservation"@en .

<http://www.opengis.net/def/timeseries/DataQualityCode/> a skos:Collection ;
    rdfs:label "Concepts in TimeSeriesML - DataQualityCode"@en ;
    rdfs:seeAlso <http://www.opengis.net/def/docs/15-042r5> ;
    skos:definition "Terms in this codelist are used to indicate the quality of individual data points."@en ;
    skos:inScheme <http://www.opengis.net/def/timeseries/DataQualityCode> ;
    skos:member <http://www.opengis.net/def/timeseries/DataQualityCode/Estimate>,
        <http://www.opengis.net/def/timeseries/DataQualityCode/Good>,
        <http://www.opengis.net/def/timeseries/DataQualityCode/Missing>,
        <http://www.opengis.net/def/timeseries/DataQualityCode/Poor>,
        <http://www.opengis.net/def/timeseries/DataQualityCode/Suspect>,
        <http://www.opengis.net/def/timeseries/DataQualityCode/Unchecked> ;
    skos:prefLabel "Concepts in TimeSeriesML - DataQualityCode"@en .

<http://www.opengis.net/def/timeseries/DataQualityCode/Estimate> a skos:Concept ;
    rdfs:label "Estimate"@en ;
    ns1:status <http://www.opengis.net/def/status/valid> ;
    rdfs:seeAlso <http://www.opengis.net/def/docs/15-042r5> ;
    skos:definition "The data is an estimate only, not a direct measurement."@en ;
    skos:inScheme <http://www.opengis.net/def/timeseries/DataQualityCode> ;
    skos:prefLabel "Estimate"@en .

<http://www.opengis.net/def/timeseries/DataQualityCode/Good> a skos:Concept ;
    rdfs:label "Good"@en ;
    ns1:status <http://www.opengis.net/def/status/valid> ;
    rdfs:seeAlso <http://www.opengis.net/def/docs/15-042r5> ;
    skos:definition "The data has been examined and represents a reliable measurement."@en ;
    skos:inScheme <http://www.opengis.net/def/timeseries/DataQualityCode> ;
    skos:prefLabel "Good"@en .

<http://www.opengis.net/def/timeseries/DataQualityCode/Missing> a skos:Concept ;
    rdfs:label "Missing"@en ;
    ns1:status <http://www.opengis.net/def/status/valid> ;
    rdfs:seeAlso <http://www.opengis.net/def/docs/15-042r5> ;
    skos:definition "The data is missing."@en ;
    skos:inScheme <http://www.opengis.net/def/timeseries/DataQualityCode> ;
    skos:prefLabel "Missing"@en .

<http://www.opengis.net/def/timeseries/DataQualityCode/Poor> a skos:Concept ;
    rdfs:label "Poor"@en ;
    ns1:status <http://www.opengis.net/def/status/valid> ;
    rdfs:seeAlso <http://www.opengis.net/def/docs/15-042r5> ;
    skos:definition "The data should be considered as low quality and may have been rejected."@en ;
    skos:inScheme <http://www.opengis.net/def/timeseries/DataQualityCode> ;
    skos:prefLabel "Poor"@en .

<http://www.opengis.net/def/timeseries/DataQualityCode/Suspect> a skos:Concept ;
    rdfs:label "Suspect"@en ;
    ns1:status <http://www.opengis.net/def/status/valid> ;
    rdfs:seeAlso <http://www.opengis.net/def/docs/15-042r5> ;
    skos:definition "The data should be treated as suspect."@en ;
    skos:inScheme <http://www.opengis.net/def/timeseries/DataQualityCode> ;
    skos:prefLabel "Suspect"@en .

<http://www.opengis.net/def/timeseries/DataQualityCode/Unchecked> a skos:Concept ;
    rdfs:label "Unchecked"@en ;
    ns1:status <http://www.opengis.net/def/status/valid> ;
    rdfs:seeAlso <http://www.opengis.net/def/docs/15-042r5> ;
    skos:definition "The data has not been checked by any qualitative method."@en ;
    skos:inScheme <http://www.opengis.net/def/timeseries/DataQualityCode> ;
    skos:prefLabel "Unchecked"@en .

<http://www.opengis.net/def/timeseries/InterpolationCode/> a skos:Collection ;
    rdfs:label "Concepts in TimeSeriesML - InterpolationCode"@en ;
    rdfs:seeAlso <http://www.opengis.net/def/docs/15-042r5> ;
    skos:definition "Terms in this codelist are used to indicate how data should be interpolated between neighboring points in a timeseries."@en ;
    skos:inScheme <http://www.opengis.net/def/timeseries/InterpolationCode> ;
    skos:member <http://www.opengis.net/def/timeseries/InterpolationCode/AveragePrec>,
        <http://www.opengis.net/def/timeseries/InterpolationCode/AverageSucc>,
        <http://www.opengis.net/def/timeseries/InterpolationCode/ConstPrec>,
        <http://www.opengis.net/def/timeseries/InterpolationCode/ConstSucc>,
        <http://www.opengis.net/def/timeseries/InterpolationCode/Continuous>,
        <http://www.opengis.net/def/timeseries/InterpolationCode/Discontinuous>,
        <http://www.opengis.net/def/timeseries/InterpolationCode/InstantTotal>,
        <http://www.opengis.net/def/timeseries/InterpolationCode/MaxPrec>,
        <http://www.opengis.net/def/timeseries/InterpolationCode/MaxSucc>,
        <http://www.opengis.net/def/timeseries/InterpolationCode/MinPrec>,
        <http://www.opengis.net/def/timeseries/InterpolationCode/MinSucc>,
        <http://www.opengis.net/def/timeseries/InterpolationCode/PrecTotal>,
        <http://www.opengis.net/def/timeseries/InterpolationCode/TotalSucc> ;
    skos:prefLabel "Concepts in TimeSeriesML - InterpolationCode"@en .

<http://www.opengis.net/def/timeseries/InterpolationCode/AveragePrec> a skos:Concept ;
    rdfs:label "Average Preceding"@en ;
    ns1:status <http://www.opengis.net/def/status/valid> ;
    rdfs:seeAlso <http://www.opengis.net/def/docs/15-042r5> ;
    skos:definition "Value represents the average value over the preceding interval.    "@en ;
    skos:inScheme <http://www.opengis.net/def/timeseries/InterpolationCode> ;
    skos:prefLabel "Average Preceding"@en .

<http://www.opengis.net/def/timeseries/InterpolationCode/AverageSucc> a skos:Concept ;
    rdfs:label "Average Succeeding"@en ;
    ns1:status <http://www.opengis.net/def/status/valid> ;
    rdfs:seeAlso <http://www.opengis.net/def/docs/15-042r5> ;
    skos:definition "Value represents the average value over the following interval.    "@en ;
    skos:inScheme <http://www.opengis.net/def/timeseries/InterpolationCode> ;
    skos:prefLabel "Average Succeeding"@en .

<http://www.opengis.net/def/timeseries/InterpolationCode/ConstPrec> a skos:Concept ;
    rdfs:label "Constant Preceding"@en ;
    ns1:status <http://www.opengis.net/def/status/valid> ;
    rdfs:seeAlso <http://www.opengis.net/def/docs/15-042r5> ;
    skos:definition "Value is constant in the preceding interval."@en ;
    skos:inScheme <http://www.opengis.net/def/timeseries/InterpolationCode> ;
    skos:prefLabel "Constant Preceding"@en .

<http://www.opengis.net/def/timeseries/InterpolationCode/ConstSucc> a skos:Concept ;
    rdfs:label "Constant Succeeding"@en ;
    ns1:status <http://www.opengis.net/def/status/valid> ;
    rdfs:seeAlso <http://www.opengis.net/def/docs/15-042r5> ;
    skos:definition "Value is constant in the succeeding interval."@en ;
    skos:inScheme <http://www.opengis.net/def/timeseries/InterpolationCode> ;
    skos:prefLabel "Constant Succeeding"@en .

<http://www.opengis.net/def/timeseries/InterpolationCode/Continuous> a skos:Concept ;
    rdfs:label "Continuous"@en ;
    ns1:status <http://www.opengis.net/def/status/valid> ;
    rdfs:seeAlso <http://www.opengis.net/def/docs/15-042r5> ;
    skos:definition "A continuous timeseries indicates the observation result is the value of a property at the indicated instant in time. The points are essentially connected and interpolation may occur between points in order to estimate the value of the property between points. The appropriate time spacing between successive points to minimize interpolation errors is related to rate of change (with respect to time) of the property."@en ;
    skos:inScheme <http://www.opengis.net/def/timeseries/InterpolationCode> ;
    skos:prefLabel "Continuous"@en .

<http://www.opengis.net/def/timeseries/InterpolationCode/Discontinuous> a skos:Concept ;
    rdfs:label "Discontinuous"@en ;
    ns1:status <http://www.opengis.net/def/status/valid> ;
    rdfs:seeAlso <http://www.opengis.net/def/docs/15-042r5> ;
    skos:definition "The sampling of the property occurs such that it is not possible to regard the series as continuous. The time between samples is too large to classify the measurements as continuous. Example: An infrequent water sample measuring pH."@en ;
    skos:inScheme <http://www.opengis.net/def/timeseries/InterpolationCode> ;
    skos:prefLabel "Discontinuous"@en .

<http://www.opengis.net/def/timeseries/InterpolationCode/InstantTotal> a skos:Concept ;
    rdfs:label "Instant Total"@en ;
    ns1:status <http://www.opengis.net/def/status/valid> ;
    rdfs:seeAlso <http://www.opengis.net/def/docs/15-042r5> ;
    skos:definition "Value represents a total attributed to a specific time instant. This is normally generated from an event based measuring device. Example: An individual tip of a tipping bucket rain gauge."@en ;
    skos:inScheme <http://www.opengis.net/def/timeseries/InterpolationCode> ;
    skos:prefLabel "Instant Total"@en .

<http://www.opengis.net/def/timeseries/InterpolationCode/MaxPrec> a skos:Concept ;
    rdfs:label "Maximum Preceding"@en ;
    ns1:status <http://www.opengis.net/def/status/valid> ;
    rdfs:seeAlso <http://www.opengis.net/def/docs/15-042r5> ;
    skos:definition "Value represents the maximum value that was measured during the preceding time interval."@en ;
    skos:inScheme <http://www.opengis.net/def/timeseries/InterpolationCode> ;
    skos:prefLabel "Maximum Preceding"@en .

<http://www.opengis.net/def/timeseries/InterpolationCode/MaxSucc> a skos:Concept ;
    rdfs:label "Maximum Succeeding"@en ;
    ns1:status <http://www.opengis.net/def/status/valid> ;
    rdfs:seeAlso <http://www.opengis.net/def/docs/15-042r5> ;
    skos:definition "Value represents the maximum value for the following interval."@en ;
    skos:inScheme <http://www.opengis.net/def/timeseries/InterpolationCode> ;
    skos:prefLabel "Maximum Succeeding"@en .

<http://www.opengis.net/def/timeseries/InterpolationCode/MinPrec> a skos:Concept ;
    rdfs:label "Minimum Preceding"@en ;
    ns1:status <http://www.opengis.net/def/status/valid> ;
    rdfs:seeAlso <http://www.opengis.net/def/docs/15-042r5> ;
    skos:definition "Value represents the minimum value that was measured during the preceding time interval."@en ;
    skos:inScheme <http://www.opengis.net/def/timeseries/InterpolationCode> ;
    skos:prefLabel "Minimum Preceding"@en .

<http://www.opengis.net/def/timeseries/InterpolationCode/MinSucc> a skos:Concept ;
    rdfs:label "Minimum Succeeding"@en ;
    ns1:status <http://www.opengis.net/def/status/valid> ;
    rdfs:seeAlso <http://www.opengis.net/def/docs/15-042r5> ;
    skos:definition "Value represents the minimum value for the following interval."@en ;
    skos:inScheme <http://www.opengis.net/def/timeseries/InterpolationCode> ;
    skos:prefLabel "Minimum Succeeding"@en .

<http://www.opengis.net/def/timeseries/InterpolationCode/PrecTotal> a skos:Concept ;
    rdfs:label "Preceding Total"@en ;
    ns1:status <http://www.opengis.net/def/status/valid> ;
    rdfs:seeAlso <http://www.opengis.net/def/docs/15-042r5> ;
    skos:definition "Value represents the total of measurements taken within the previous time interval."@en ;
    skos:inScheme <http://www.opengis.net/def/timeseries/InterpolationCode> ;
    skos:prefLabel "Preceding Total"@en .

<http://www.opengis.net/def/timeseries/InterpolationCode/TotalSucc> a skos:Concept ;
    rdfs:label "Total Succeeding"@en ;
    ns1:status <http://www.opengis.net/def/status/valid> ;
    rdfs:seeAlso <http://www.opengis.net/def/docs/15-042r5> ;
    skos:definition "Value represents the average value over the following interval."@en ;
    skos:inScheme <http://www.opengis.net/def/timeseries/InterpolationCode> ;
    skos:prefLabel "Total Succeeding"@en .

<http://www.opengis.net/def/timeseries/ProcessTypeCode/> a skos:Collection ;
    rdfs:label "Concepts in TimeSeriesML - ProcessTypeCode"@en ;
    rdfs:seeAlso <http://www.opengis.net/def/docs/15-042r5> ;
    skos:definition "Terms from this codelist are used to indicate the type of process that was used in an observation."@en ;
    skos:inScheme <http://www.opengis.net/def/timeseries/ProcessTypeCode> ;
    skos:member <http://www.opengis.net/def/timeseries/ProcessTypeCode/Algorithm>,
        <http://www.opengis.net/def/timeseries/ProcessTypeCode/ManualMethod>,
        <http://www.opengis.net/def/timeseries/ProcessTypeCode/Sensor>,
        <http://www.opengis.net/def/timeseries/ProcessTypeCode/Simulation>,
        <http://www.opengis.net/def/timeseries/ProcessTypeCode/Unknown> ;
    skos:prefLabel "Concepts in TimeSeriesML - ProcessTypeCode"@en .

<http://www.opengis.net/def/timeseriesType/timeseriesML/1.2/Time/CategoricalTimeseriesDomainRange> a skos:Concept ;
    rdfs:label "CategoricalTimeseriesDomainRangeTimeseries"@en ;
    ns1:status <http://www.opengis.net/def/status/valid> ;
    rdfs:seeAlso <http://www.opengis.net/def/docs/15-042r5> ;
    skos:definition "CategoricalTimeseriesDomainRangeTimeseries"@en ;
    skos:inScheme <http://www.opengis.net/def/timeseriesType/timeseriesML> ;
    skos:prefLabel "CategoricalTimeseriesDomainRangeTimeseries"@en .

<http://www.opengis.net/def/timeseriesType/timeseriesML/1.2/Time/MeasurementTimeseriesDomainRange> a skos:Concept ;
    rdfs:label "MeasurementTimeseriesDomainRangeTimeseries"@en ;
    ns1:status <http://www.opengis.net/def/status/valid> ;
    rdfs:seeAlso <http://www.opengis.net/def/docs/15-042r5> ;
    skos:definition "MeasurementTimeseriesDomainRangeTimeseries"@en ;
    skos:inScheme <http://www.opengis.net/def/timeseriesType/timeseriesML> ;
    skos:prefLabel "MeasurementTimeseriesDomainRangeTimeseries"@en .

<http://www.opengis.net/def/timeseriesType/timeseriesML/TimeseriesDomainRange> a void:Dataset,
        <http://www.opengis.net/def/metamodel/lid/ConceptScheme>,
        <http://www.opengis.net/def/metamodel/lid/lidset>,
        skos:ConceptScheme ;
    rdfs:label "TimeSeriesML - TimeseriesDomainRange"@en ;
    dcterms:source <http://www.opengis.net/def/entities/bodies/ogcna> ;
    ns1:collectionView <http://www.opengis.net/def/timeseriesType/timeseriesML/TimeseriesDomainRange/> ;
    rdfs:seeAlso <http://www.opengis.net/def/docs/15-042r5> ;
    skos:definition "A tsml:type property is present on the TimeseriesDomainRange type to enable a soft-typing approach to this class. The values for this property should be taken from this list."@en ;
    skos:prefLabel "TimeSeriesML - TimeseriesDomainRange"@en .

<http://www.opengis.net/def/timeseriesType/timeseriesML/TimeseriesDomainRange/> a skos:Collection ;
    rdfs:label "Concepts in TimeSeriesML - TimeseriesDomainRange"@en ;
    rdfs:seeAlso <http://www.opengis.net/def/docs/15-042r5> ;
    skos:definition "A tsml:type property is present on the TimeseriesDomainRange type to enable a soft-typing approach to this class. The values for this property should be taken from this list."@en ;
    skos:inScheme <http://www.opengis.net/def/timeseriesType/timeseriesML/TimeseriesDomainRange> ;
    skos:member <http://www.opengis.net/def/timeseriesType/timeseriesML/1.2/Time/CategoricalTimeseriesDomainRange>,
        <http://www.opengis.net/def/timeseriesType/timeseriesML/1.2/Time/MeasurementTimeseriesDomainRange> ;
    skos:prefLabel "Concepts in TimeSeriesML - TimeseriesDomainRange"@en .

<http://www.opengis.net/def/waterml/2.0/process-type/algorithm> skos:broader <http://www.opengis.net/def/timeseries/ProcessTypeCode/Algorithm> .

<http://www.opengis.net/def/waterml/2.0/process-type/manual-method> skos:broader <http://www.opengis.net/def/timeseries/ProcessTypeCode/ManualMethod> .

<http://www.opengis.net/def/waterml/2.0/process-type/sensor> skos:broader <http://www.opengis.net/def/timeseries/ProcessTypeCode/Sensor> .

<http://www.opengis.net/def/waterml/2.0/process-type/simulation> skos:broader <http://www.opengis.net/def/timeseries/ProcessTypeCode/Simulation> .

<http://www.opengis.net/def/waterml/2.0/process-type/unknown> skos:broader <http://www.opengis.net/def/timeseries/ProcessTypeCode/Unknown> .

<http://www.opengis.net/def/waterml/2.0/processType/Algorithm> skos:broader <http://www.opengis.net/def/timeseries/ProcessTypeCode/Algorithm> .

<http://www.opengis.net/def/waterml/2.0/processType/ManualMethod> skos:broader <http://www.opengis.net/def/timeseries/ProcessTypeCode/ManualMethod> .

<http://www.opengis.net/def/waterml/2.0/processType/Sensor> skos:broader <http://www.opengis.net/def/timeseries/ProcessTypeCode/Sensor> .

<http://www.opengis.net/def/waterml/2.0/processType/Simulation> skos:broader <http://www.opengis.net/def/timeseries/ProcessTypeCode/Simulation> .

<http://www.opengis.net/def/waterml/2.0/processType/Unknown> skos:broader <http://www.opengis.net/def/timeseries/ProcessTypeCode/Unknown> .

<http://www.opengis.net/def/timeseries/ProcessTypeCode/Algorithm> a skos:Concept ;
    rdfs:label "Algorithm"@en ;
    ns1:status <http://www.opengis.net/def/status/valid> ;
    rdfs:seeAlso <http://www.opengis.net/def/docs/15-042r5> ;
    skos:definition "Timeseries data is generated by applying an algorithm to input data"@en ;
    skos:inScheme <http://www.opengis.net/def/timeseries/ProcessTypeCode> ;
    skos:narrower <http://www.opengis.net/def/waterml/2.0/process-type/algorithm>,
        <http://www.opengis.net/def/waterml/2.0/processType/Algorithm> ;
    skos:prefLabel "Algorithm"@en .

<http://www.opengis.net/def/timeseries/ProcessTypeCode/ManualMethod> a skos:Concept ;
    rdfs:label "Manual Method"@en ;
    ns1:status <http://www.opengis.net/def/status/valid> ;
    rdfs:seeAlso <http://www.opengis.net/def/docs/15-042r5> ;
    skos:definition "Timeseries data is collected manually"@en ;
    skos:inScheme <http://www.opengis.net/def/timeseries/ProcessTypeCode> ;
    skos:narrower <http://www.opengis.net/def/waterml/2.0/process-type/manual-method>,
        <http://www.opengis.net/def/waterml/2.0/processType/ManualMethod> ;
    skos:prefLabel "Manual Method"@en .

<http://www.opengis.net/def/timeseries/ProcessTypeCode/Sensor> a skos:Concept ;
    rdfs:label "Sensor"@en ;
    ns1:status <http://www.opengis.net/def/status/valid> ;
    rdfs:seeAlso <http://www.opengis.net/def/docs/15-042r5> ;
    skos:definition "Timeseries data is collected from an automated sensor"@en ;
    skos:inScheme <http://www.opengis.net/def/timeseries/ProcessTypeCode> ;
    skos:narrower <http://www.opengis.net/def/waterml/2.0/process-type/sensor>,
        <http://www.opengis.net/def/waterml/2.0/processType/Sensor> ;
    skos:prefLabel "Sensor"@en .

<http://www.opengis.net/def/timeseries/ProcessTypeCode/Simulation> a skos:Concept ;
    rdfs:label "Simulation"@en ;
    ns1:status <http://www.opengis.net/def/status/valid> ;
    rdfs:seeAlso <http://www.opengis.net/def/docs/15-042r5> ;
    skos:definition "Timeseries is generated from a simulation"@en ;
    skos:inScheme <http://www.opengis.net/def/timeseries/ProcessTypeCode> ;
    skos:narrower <http://www.opengis.net/def/waterml/2.0/process-type/simulation>,
        <http://www.opengis.net/def/waterml/2.0/processType/Simulation> ;
    skos:prefLabel "Simulation"@en .

<http://www.opengis.net/def/timeseries/ProcessTypeCode/Unknown> a skos:Concept ;
    rdfs:label "Unknown"@en ;
    ns1:status <http://www.opengis.net/def/status/valid> ;
    rdfs:seeAlso <http://www.opengis.net/def/docs/15-042r5> ;
    skos:definition "Timeseries is collected or generated by an unknown process"@en ;
    skos:inScheme <http://www.opengis.net/def/timeseries/ProcessTypeCode> ;
    skos:narrower <http://www.opengis.net/def/waterml/2.0/process-type/unknown>,
        <http://www.opengis.net/def/waterml/2.0/processType/Unknown> ;
    skos:prefLabel "Unknown"@en .

<http://www.opengis.net/def/entities/bodies/ogcna> a skos:Concept .

<http://www.opengis.net/def/observationType/timeseriesML> a void:Dataset,
        <http://www.opengis.net/def/metamodel/lid/ConceptScheme>,
        <http://www.opengis.net/def/metamodel/lid/lidset>,
        skos:ConceptScheme ;
    rdfs:label "TimeSeriesML - observationType"@en ;
    dcterms:source <http://www.opengis.net/def/entities/bodies/ogcna> ;
    ns1:collectionView <http://www.opengis.net/def/observationType/timeseriesML/> ;
    rdfs:seeAlso <http://www.opengis.net/def/docs/15-042r5> ;
    skos:definition "In accordance with OMXML, the specialization of the OM_Observation result type is provided through schematron restriction. The om:type element may be used to specify the type of OM_Observation that is being encoded. This shall be done using the OGC Name URI for the corresponding type from this list."@en ;
    skos:prefLabel "TimeSeriesML - observationType"@en .

<http://www.opengis.net/def/timeseries/ProcessTypeCode> a void:Dataset,
        <http://www.opengis.net/def/metamodel/lid/ConceptScheme>,
        <http://www.opengis.net/def/metamodel/lid/lidset>,
        skos:ConceptScheme ;
    rdfs:label "TimeSeriesML - ProcessTypeCode"@en ;
    dcterms:source <http://www.opengis.net/def/entities/bodies/ogcna> ;
    ns1:collectionView <http://www.opengis.net/def/timeseries/ProcessTypeCode/> ;
    rdfs:seeAlso <http://www.opengis.net/def/docs/15-042r5> ;
    skos:definition "Terms from this codelist are used to indicate the type of process that was used in an observation."@en ;
    skos:prefLabel "TimeSeriesML - ProcessTypeCode"@en .

<http://www.opengis.net/def/timeseries/DataQualityCode> a void:Dataset,
        <http://www.opengis.net/def/metamodel/lid/ConceptScheme>,
        <http://www.opengis.net/def/metamodel/lid/lidset>,
        skos:ConceptScheme ;
    rdfs:label "TimeSeriesML - DataQualityCode"@en ;
    dcterms:source <http://www.opengis.net/def/entities/bodies/ogcna> ;
    ns1:collectionView <http://www.opengis.net/def/timeseries/DataQualityCode/> ;
    rdfs:seeAlso <http://www.opengis.net/def/docs/15-042r5> ;
    skos:definition "Terms in this codelist are used to indicate the quality of individual data points."@en ;
    skos:prefLabel "TimeSeriesML - DataQualityCode"@en .

<http://www.opengis.net/def/timeseries/InterpolationCode> a void:Dataset,
        <http://www.opengis.net/def/metamodel/lid/ConceptScheme>,
        <http://www.opengis.net/def/metamodel/lid/lidset>,
        skos:ConceptScheme ;
    rdfs:label "TimeSeriesML - InterpolationCode"@en ;
    dcterms:source <http://www.opengis.net/def/entities/bodies/ogcna> ;
    ns1:collectionView <http://www.opengis.net/def/timeseries/InterpolationCode/> ;
    rdfs:seeAlso <http://www.opengis.net/def/docs/15-042r5> ;
    skos:definition "Terms in this codelist are used to indicate how data should be interpolated between neighboring points in a timeseries."@en ;
    skos:prefLabel "TimeSeriesML - InterpolationCode"@en .

